Hybrid/PPermutLib.v
@@ -1,0 +1,553 @@
+Require Import Setoid.
+Require Export LibTactics.
+Require Export Shared.
+Require Export PermutLib.
+
+Open Scope permut_scope.
+
+Inductive PPermut: list Context_LF -> list Context_LF -> Prop :=
+| PPermut_nil: PPermut nil nil
+| PPermut_skip: forall G G' w Gamma Gamma',
+    Gamma *=* Gamma' ->
+    PPermut G G' ->
+    PPermut ((w, Gamma)::G) ((w,Gamma')::G')
+| PPermut_swap: forall G w w' Gamma0 Gamma0' Gamma1 Gamma1',
+    Gamma0 *=* Gamma1 ->
+    Gamma0' *=* Gamma1' ->
+    PPermut ((w, Gamma0) :: (w', Gamma0') :: G)
+                ((w', Gamma1') :: (w, Gamma1) :: G)
+| PPermut_trans: forall G G' G'',
+    PPermut G G' -> PPermut G' G'' -> PPermut G G''.
+Hint Resolve PPermut_nil PPermut_skip PPermut_swap.
+Hint Constructors PPermut : ppermut_rew.
+
+Notation "G ~=~ G'" := (PPermut G G') (at level 70) : permut_scope.
+
+Lemma PPermut_reflexive:
+  Reflexive PPermut.
+unfold Reflexive; intros;
+induction x; [ | destruct a]; eauto.
+Qed.
+
+Lemma PPermut_symmetric:
+  Symmetric PPermut.
+unfold Symmetric; intros;
+induction H; eauto with ppermut_rew.
+  apply PPermut_trans with (G':=(w, Gamma')::G); eauto with ppermut_rew;
+  apply PPermut_skip;
+  [ apply permut_sym |
+    apply PPermut_reflexive];
+  auto.
+  apply PPermut_swap; apply permut_sym; assumption.
+Qed.
+
+Lemma PPermut_transitive:
+  Transitive PPermut.
+exact PPermut_trans.
+Qed.
+Hint Resolve PPermut_reflexive PPermut_symmetric.
+
+Theorem PPermut'oid: Setoid_Theory _ PPermut.
+  split.
+  exact PPermut_reflexive.
+  exact PPermut_symmetric.
+  exact PPermut_transitive.
+Qed.
+
+Add Setoid (list Context_LF) PPermut PPermut'oid as PPermutoid.
+
+Add Morphism (@cons Context_LF) : PPermut_cons.
+intro y; destruct y; auto.
+Qed.
+Hint Resolve PPermut_cons.
+
+Lemma PPermut_app_tail:
+forall G G' G0,
+  G ~=~ G' ->
+  G ++ G0 ~=~ G' ++ G0.
+intros; induction H; simpl; rew_app; auto;
+econstructor; eauto.
+Qed.
+
+Lemma PPermut_app_head:
+forall G0 G G',
+  G ~=~ G' ->
+  G0 ++ G ~=~ G0 ++ G'.
+intros; induction G0; simpl; rew_app; auto.
+Qed.
+Hint Resolve PPermut_app_tail PPermut_app_head.
+
+Add Morphism (@append Context_LF) : PPermut_app.
+intros; induction H; simpl in *; rew_app; auto.
+transitivity ((w, Gamma0) :: (w', Gamma0') :: G ++ y0); auto.
+transitivity (G' ++ y0); auto.
+Qed.
+Hint Resolve PPermut_app.
+
+Theorem PPermut_app_comm:
+forall G1 G2,
+  G1 ++ G2 ~=~ G2 ++ G1.
+induction G1; intros; simpl; rew_app;
+[ auto |
+ induction G2]; simpl in *;
+[ rewrite app_nil_r; auto |
+  destruct a; destruct a0];
+transitivity ((v,l) :: (v0, l0) :: G2 ++ G1);
+[ constructor; auto; apply IHG1 |
+  transitivity ((v0, l0) :: (v, l) :: G2 ++ G1); auto];
+rew_app; constructor; auto;
+transitivity ((v,l) :: G1 ++ G2); auto.
+Qed.
+Hint Resolve PPermut_app_comm.
+
+
+(*** Automation **)
+(* Based on permutation tactics from tlc's LibListSorted *)
+
+Lemma PPermut_get_1 : forall l1 l2,
+  PPermut (l1 ++ l2) (l1 ++ l2).
+auto.
+Qed.
+
+Lemma PPermut_get_2 : forall l1 l2 l3,
+  PPermut (l1 ++ l2 ++ l3) (l2 ++ l1 ++ l3).
+intros;
+assert (l1 ++ l2 ~=~ l2 ++ l1) as H by auto;
+transitivity ((l1 ++ l2) ++ l3); [ | rewrite H ]; rew_app; auto.
+Qed.
+
+Lemma PPermut_get_3 : forall l1 l2 l3 l4,
+  PPermut (l1 ++ l2 ++ l3 ++ l4) (l2 ++ l3 ++ l1 ++ l4).
+intros;
+do 2 rewrite <- (@app_assoc _ l2); eapply PPermut_get_2.
+Qed.
+
+Lemma PPermut_get_4 : forall l1 l2 l3 l4 l5,
+  PPermut (l1 ++ l2 ++ l3 ++ l4 ++ l5)
+         (l2 ++ l3 ++ l4 ++ l1 ++ l5).
+intros;
+do 2 rewrite <- (@app_assoc _ l2); eapply PPermut_get_3.
+Qed.
+
+Lemma PPermut_get_5 : forall l1 l2 l3 l4 l5 l6,
+  PPermut (l1 ++ l2 ++ l3 ++ l4 ++ l5 ++ l6)
+         (l2 ++ l3 ++ l4 ++ l5 ++ l1 ++ l6).
+intros;
+do 2 rewrite <- (@app_assoc _ l2); eapply PPermut_get_4.
+Qed.
+
+Lemma PPermut_get_6 : forall l1 l2 l3 l4 l5 l6 l7,
+  PPermut (l1 ++ l2 ++ l3 ++ l4 ++ l5 ++ l6 ++ l7)
+         (l2 ++ l3 ++ l4 ++ l5 ++ l6 ++ l1 ++ l7).
+intros;
+do 2 rewrite <- (@app_assoc _ l2); eapply PPermut_get_5.
+Qed.
+
+Lemma PPermut_tactic_setup : forall l1 l2,
+  PPermut (nil ++ l1 ++ nil) (l2 ++ nil) -> PPermut l1 l2.
+intros; rew_app in *; auto.
+Qed.
+
+Lemma PPermut_tactic_keep : forall l1 l2 l3 l4,
+  PPermut ((l1 ++ l2) ++ l3) l4 ->
+  PPermut (l1 ++ (l2 ++ l3)) l4.
+intros; rew_app in *; auto.
+Qed.
+
+Lemma PPermut_tactic_simpl : forall l1 l2 l3 l4,
+  PPermut (l1 ++ l3) l4 ->
+  PPermut (l1 ++ (l2 ++ l3)) (l2 ++ l4).
+intros; rewrite <- H; apply PPermut_get_2.
+Qed.
+
+Lemma PPermut_tactic_trans : forall l1 l2 l3,
+  PPermut l3 l2 -> PPermut l1 l3 -> PPermut l1 l2.
+intros; eauto with ppermut_rew.
+Qed.
+
+Hint Rewrite app_assoc app_nil_l app_nil_r : ppermut_rew.
+
+Ltac PPermut_lemma_get n :=
+  match nat_from_number n with
+  | 1 => constr:(PPermut_get_1)
+  | 2 => constr:(PPermut_get_2)
+  | 3 => constr:(PPermut_get_3)
+  | 4 => constr:(PPermut_get_4)
+  | 5 => constr:(PPermut_get_5)
+  end.
+
+Ltac PPermut_isolate_cons :=
+  do 20 try (* todo : repeat *)
+    match goal with |- context [?x::?l] =>
+      match l with
+      | nil => fail 1
+      | _ => rewrite <- (@app_cons_one _ x l)
+      end
+    end.
+
+Ltac PPermut_simpl_prepare :=
+   autorewrite with ppermut_rew;
+   PPermut_isolate_cons;
+   autorewrite with ppermut_rew;
+   apply PPermut_tactic_setup;
+   repeat rewrite app_assoc.
+
+Ltac PPermut_index_of l lcontainer :=
+  match constr:(lcontainer) with
+  | l ++ _ => constr:(1)
+  | _ ++ l ++ _ => constr:(2)
+  | _ ++ _ ++ l ++ _ => constr:(3)
+  | _ ++ _ ++ _ ++ l ++ _ => constr:(4)
+  | _ ++ _ ++ _ ++ _ ++ l ++ _ => constr:(5)
+  | _ ++ _ ++ _ ++ _ ++ _ ++ l ++ _ => constr:(6)
+  | _ => constr:(0) (* not found *)
+  end.
+
+Ltac PPermut_simpl_once :=
+  match goal with
+  | |- PPermut (_ ++ nil) _ => fail 1
+  | |- PPermut (_ ++ (?l ++ _)) ?l' =>
+     match PPermut_index_of l l' with
+     | 0 => apply PPermut_tactic_keep
+     | ?n => let F := PPermut_lemma_get n in
+            eapply PPermut_tactic_trans;
+            [ apply F
+            | apply PPermut_tactic_simpl ]
+     end
+  end.
+
+Ltac PPermut_simpl :=
+  PPermut_simpl_prepare;
+  repeat PPermut_simpl_once;
+  autorewrite with ppermut_rew;
+  try apply PPermut_reflexive;
+  auto.
+
+
+(*** Other lemmas ***)
+(* Note:
+   Some are covered by PPermut_simpl tactic, but we want to use them in auto! *)
+
+Lemma PPermut_Mem:
+forall G G' w X,
+  G ~=~ G' ->
+  Mem (w, X) G ->
+  exists X', X' *=* X /\ Mem (w, X') G'.
+intros; generalize dependent X; induction H; intros.
+rewrite Mem_nil_eq in H0; contradiction.
+rewrite Mem_cons_eq in H1; destruct H1.
+inversion H1; subst; exists Gamma'; split; [ symmetry | apply Mem_here]; auto.
+apply IHPPermut in H1; destruct H1 as (Gamma''); exists Gamma'';
+destruct H1; split; auto; rewrite Mem_cons_eq; right; auto.
+repeat rewrite Mem_cons_eq in H1; destruct H1.
+inversion H1; subst; exists Gamma1; split; [ symmetry | rewrite Mem_cons_eq];
+auto; right; apply Mem_here.
+destruct H1.
+inversion H1; subst; exists Gamma1'; split; [ symmetry | rewrite Mem_cons_eq];
+auto.
+exists X; split; auto; repeat rewrite Mem_cons_eq; right; right; auto.
+apply IHPPermut1 in H1; destruct H1 as (X'); destruct H1.
+apply IHPPermut2 in H2; destruct H2 as (X''); destruct H2;
+exists X''; split; auto; transitivity X'; auto.
+Qed.
+
+Lemma PPermut_nil_impl:
+forall L,
+  nil ~=~ L -> L = nil.
+intros; remember (@nil Context_LF) as L' in H;
+induction H; intros;
+discriminate || auto.
+Qed.
+
+Lemma PPermut_nil_contr:
+forall L a,
+  ~ (PPermut nil (a::L)).
+induction L; intros; intro;
+apply PPermut_nil_impl in H; discriminate.
+Qed.
+
+Hint Resolve PPermut_nil_impl PPermut_nil_contr.
+
+(* Based on Sorting/Permutation/Permutation_ind_bis *)
+Theorem PPermut_ind_bis :
+ forall P : list Context_LF -> list Context_LF -> Prop,
+   P nil nil ->
+   (forall w x y l l', l ~=~ l' -> P l l' ->
+     x *=* y -> P ((w,x) :: l) ((w,y) :: l')) ->
+   (forall w w' x x' y y' l l', l ~=~ l' -> P l l' -> x *=* x' -> y *=* y' ->
+     P ((w', y) :: (w, x) :: l) ((w, x') :: (w', y') :: l')) ->
+   (forall l l' l'', l ~=~ l' -> P l l' -> l' ~=~ l'' -> P l' l'' -> P l l'') ->
+   forall l l', l ~=~ l' -> P l l'.
+Proof.
+  intros P Hnil Hskip Hswap Htrans;
+  intros; induction H; auto.
+  apply Htrans with ((w', Gamma0')::(w, Gamma0)::G); auto.
+    apply Hswap; auto; induction G; auto; destruct a; apply Hskip; auto.
+    apply Hskip; auto; apply Hskip; auto; induction G; auto;
+    destruct a; apply Hskip; auto.
+  eauto.
+Qed.
+
+Lemma PPermut_app_rev:
+forall G G' H H' w a a',
+  a *=* a' ->
+  G & (w, a) ++ G' ~=~ H & (w, a') ++ H' ->
+  G ++ G' ~=~ H ++ H'.
+Proof.
+  set (P l l' :=
+         forall w a a' l1 l2 l3 l4, a *=* a' ->
+         l=l1 & (w, a) ++ l2 -> l'=l3 & (w, a') ++l4 -> (l1++l2) ~=~ (l3++l4)).
+  cut (forall l l', l ~=~ l' -> P l l').
+  intros; apply (H _ _ H2 w a a'); auto.
+  intros; apply (PPermut_ind_bis P); unfold P; clear P;
+    try clear H l l'; simpl; auto.
+  (* nil *)
+  intros; destruct l1; simpl in *; discriminate.
+  (* skip *)
+  intros w x y l l' H IH; intros.
+  destruct l1; destruct l3; rew_app in *;
+  inversion H2; inversion H3; subst; auto.
+    rewrite H; PPermut_simpl; constructor; [transitivity a |] ; auto;
+      symmetry; auto.
+    rewrite <- H; PPermut_simpl; constructor; auto; transitivity a';
+      [ | symmetry]; auto.
+  constructor; auto.
+  apply (IH w0 a a' l1 l2 l3 l4); rew_app; auto.
+  (* swap *)
+  intros w w' x x' y y' l l' Hp IH; intros.
+  destruct l1; destruct l2; rew_app in *; subst;
+  inversion H2; subst; auto; try rewrite Hp; rew_app;
+  PPermut_simpl; destruct l3; destruct l4; rew_app in *; subst;
+  inversion H3; subst; auto.
+    constructor; auto; transitivity a'; auto; transitivity a; auto;
+    symmetry; auto.
+    constructor; auto; destruct l3; rew_app in *; inversion H6; subst; auto;
+      PPermut_simpl; constructor; auto; transitivity a; auto; symmetry; auto.
+    constructor; auto; destruct l3; rew_app in *; inversion H6; subst; auto;
+      PPermut_simpl; constructor; auto; transitivity a; auto; symmetry; auto.
+    constructor; auto; destruct l1; rew_app in *; inversion H6; subst; auto;
+      PPermut_simpl; rewrite <- Hp; PPermut_simpl; constructor; auto;
+      transitivity a'; auto; symmetry; auto.
+  destruct l1; destruct l3; rew_app in *; inversion H6; inversion H7; subst;
+    auto.
+      constructor; auto; transitivity a'; auto; transitivity a; auto;
+        symmetry; auto.
+       apply PPermut_nil_impl in Hp; destruct l3; rew_app in *; discriminate.
+       symmetry in Hp; apply PPermut_nil_impl in Hp; destruct l1; rew_app in *;
+         discriminate.
+       transitivity ((w', y') :: (w, x') :: l1).
+         constructor; [ | constructor]; auto.
+         PPermut_simpl.
+       replace l1 with (l1 ++ nil) by (rew_app; auto);
+       replace l3 with (l3 ++ nil) by (rew_app; auto);
+       apply IH with (w:=w0) (a0:=a) (a'0:=a'); auto;
+         rew_app; auto.
+  destruct l1; destruct l3; rew_app in *; inversion H6; inversion H7; subst;
+    auto.
+       apply PPermut_nil_impl in Hp; discriminate.
+       apply PPermut_nil_impl in Hp; destruct l3; rew_app in *; discriminate.
+       rewrite <- Hp; PPermut_simpl; transitivity ((w,x)::(w0,y)::nil);
+         PPermut_simpl; constructor; auto; constructor; auto; transitivity a';
+         auto; symmetry; auto.
+       transitivity ((w',y')::(w,x')::l1); auto; PPermut_simpl; rew_app;
+       replace l1 with (l1 ++ nil) by (rew_app; auto);
+       apply IH with (w:=w0) (a0:=a) (a'0:=a'); auto;
+         rew_app; auto.
+  constructor; auto; rewrite <- Hp; symmetry; destruct l1; rew_app in *;
+    inversion H6; subst; auto; PPermut_simpl; constructor; auto;
+    transitivity a'; auto; symmetry; auto.
+  destruct l3; rew_app in *; inversion H7; subst.
+    symmetry in Hp; apply PPermut_nil_impl in Hp; subst; inversion H6; subst;
+      destruct l1; rew_app in *; inversion H6; subst; destruct l1; rew_app in *;
+      discriminate.
+    transitivity ((w', y') ::l1 ++ p0 :: l2); PPermut_simpl; rew_app.
+    destruct l1; rew_app in *; inversion H6; subst.
+      rewrite Hp; PPermut_simpl; constructor; auto; transitivity a; auto;
+      symmetry; auto.
+      constructor; auto; replace l3 with (l3 ++ nil) by (rew_app; auto);
+      apply IH with (w:=w0) (a0:=a) (a'0:=a'); auto; rew_app; auto.
+  clear H2 H3. destruct l1; destruct l3; rew_app in *; inversion H6;
+  inversion H7; subst.
+    constructor; auto; transitivity a; auto; transitivity a'; auto;
+    symmetry; auto.
+    transitivity ((w', y'):: p0 :: l2).
+      constructor; auto.
+      PPermut_simpl. clear H6 H7. rew_app; rewrite Hp; PPermut_simpl;
+      constructor; auto; transitivity a; auto; symmetry; auto.
+    transitivity ((w, x)::p1::l4).
+      PPermut_simpl; rew_app; rewrite <- Hp; PPermut_simpl; constructor;
+        auto; transitivity a'; auto; symmetry; auto.
+      constructor; auto.
+    transitivity ((w', y') :: (w, x') :: l1 ++ p0 :: l2).
+      constructor; auto; constructor; auto.
+      PPermut_simpl. clear H7 H6. rew_app.
+    apply IH with (w:=w0) (a0:=a) (a'0:=a'); rew_app; auto.
+  (* trans *)
+  intros. destruct (PPermut_Mem l l' w a) as (a'', (H6a, H6b)); auto.
+    subst; rewrite Mem_app_or_eq; left; rewrite Mem_app_or_eq; right;
+      apply Mem_here.
+  destruct (Mem_split Context_LF l' (w, a'')) as (l'1, (l'2, H6)); auto.
+  transitivity (l'1 ++ l'2).
+    apply H0 with (w:=w) (a:=a) (a':=a''); [ symmetry | | ]; auto.
+    apply H2 with (w:=w) (a:=a'') (a':=a').
+      transitivity a; auto; symmetry; auto.
+      auto.
+      auto.
+Qed.
+
+Lemma PPermut_last_rev_simpl:
+forall G G' a,
+  G & a ~=~ G' & a ->
+  G ~=~ G'.
+intros. replace G with (G ++ nil);
+replace G' with (G'++nil).
+destruct a; eapply PPermut_app_rev; rew_app; eauto.
+rew_app; auto.
+rew_app; auto.
+rew_app; auto.
+Qed.
+
+Lemma PPermut_last_rev:
+forall G G' w Gamma Gamma',
+  Gamma *=* Gamma' ->
+  G & (w, Gamma) ~=~ G' & (w, Gamma') ->
+  G ~=~ G'.
+intros;
+assert (G & (w, Gamma) ~=~ G' & (w, Gamma)) by eauto with ppermut_rew;
+apply PPermut_last_rev_simpl with (a:=(w, Gamma)); auto.
+Qed.
+
+Lemma PPermut_split_head:
+forall G G' w Gamma,
+  (w, Gamma) :: G ~=~ G' ->
+  exists Gamma' hd tl,
+    Gamma *=* Gamma' /\ G' = hd & (w, Gamma') ++ tl.
+intros.
+apply PPermut_Mem with (w:=w) (X:=Gamma) in H.
+destruct H as (Gamma'); destruct H.
+exists Gamma'.
+assert (exists hd, exists tl, G' = hd & (w, Gamma') ++ tl) by
+  (eapply Mem_split; auto).
+destruct H1 as (hd, (tl, H1));
+exists hd; exists tl; split; [symmetry | ]; auto.
+apply Mem_here.
+Qed.
+
+Lemma PPermut_split_neq:
+forall G G' w w' Gamma Gamma',
+  G & (w, Gamma) ~=~ G' & (w', Gamma') ->
+  ~Gamma *=* Gamma' \/ w <> w' ->
+  exists Gamma0, exists GH, exists GT,
+    Gamma0 *=* Gamma' /\
+    G = GH & (w', Gamma0) ++ GT.
+intros.
+assert ((w, Gamma) ::G  ~=~ (G' & (w', Gamma'))) by
+  (transitivity (G & (w,Gamma)); auto; PPermut_simpl).
+assert ((w, Gamma) :: G ~=~ (w', Gamma') :: G') by
+  (transitivity (G' & (w', Gamma')); auto; PPermut_simpl).
+symmetry in H2;
+apply PPermut_split_head in H2; destruct H2 as (Gamma'',(GH, (GT, (Ha, Hb)))).
+destruct GH; rew_app in *.
+inversion Hb; subst; destruct H0; elim H0; symmetry; auto.
+destruct p; inversion Hb; subst.
+exists Gamma''; exists GH; exists GT; split;
+[symmetry | rew_app]; auto.
+Qed.
+
+Lemma PPermut_swap2:
+forall C C' G,
+  C :: G & C' ~=~ G & C & C'.
+intros; PPermut_simpl.
+Qed.
+Hint Resolve PPermut_swap2.
+
+Lemma PPermut_middle_last:
+forall G G' C,
+  G ++ G' & C ~=~ G ++ C :: G'.
+intros; PPermut_simpl.
+Qed.
+Hint Resolve PPermut_middle_last.
+
+Lemma PPermut_specialized1:
+forall G G' C C',
+  G ++ C :: G' & C' ~=~ G ++ G' ++ C' :: C :: nil.
+intros; PPermut_simpl.
+Qed.
+
+Lemma PPermut_specialized2:
+forall GH GT G Gamma Gamma' Gamma'',
+  GH ++ Gamma :: GT & Gamma' ~=~ G & Gamma ->
+  GH ++ GT ++ Gamma'' :: Gamma' :: nil ~=~ G & Gamma''.
+intros; PPermut_simpl;
+apply PPermut_last_rev_simpl with (a:=Gamma);
+rewrite <- H; PPermut_simpl.
+Qed.
+
+Lemma PPermut_specialized3:
+forall G G' C C',
+  G ++ G' ++ C :: C' :: nil ~=~ G ++ C :: G' & C'.
+intros; PPermut_simpl.
+Qed.
+
+Lemma PPermut_specialized4:
+forall G GH GT Gamma Gamma0 Gamma'0,
+  GH ++ Gamma :: GT & Gamma'0 ~=~ G & Gamma ->
+  G ++ Gamma0 :: Gamma :: nil ~=~ GH ++ GT ++ Gamma0 :: Gamma'0 :: Gamma :: nil.
+intros; PPermut_simpl;
+apply PPermut_last_rev_simpl with (a:=Gamma); rewrite <- H;
+PPermut_simpl.
+Qed.
+
+Lemma PPermut_specialized5:
+forall G G' C C' C'',
+  G ++ C :: G' ++ C' :: C'' :: nil ~=~ (G ++ G' ++ C' :: C'' :: nil) & C.
+intros; PPermut_simpl.
+Qed.
+
+Lemma PPermut_specialized6:
+forall GH GT C0 C'' C'0,
+  GH ++ GT ++ C'0 :: C'' :: C0 :: nil ~=~ GH ++ GT ++ C0 :: C'0 :: C'' :: nil.
+intros; PPermut_simpl.
+Qed.
+
+Lemma PPermut_swap_inner:
+forall G G' C C',
+  C :: G ++ C' :: G' ~=~ C' :: G ++ G' & C.
+intros; PPermut_simpl.
+Qed.
+
+Lemma PPermut_swap_inner2:
+forall G G' C C',
+  C :: G ++ G' & C' ~=~ C' :: G ++ G' & C.
+intros; PPermut_simpl.
+Qed.
+
+Lemma PPermut_swap3:
+forall C C' G,
+  C :: G & C' ~=~ C' :: G & C.
+intros; PPermut_simpl.
+Qed.
+
+Lemma PPermut_swap4:
+forall C G' G,
+  G ++ G' & C ~=~ G & C ++ G'.
+intros; PPermut_simpl.
+Qed.
+
+Hint Resolve PPermut_swap_inner.
+Hint Resolve PPermut_swap_inner2.
+Hint Resolve PPermut_swap3 PPermut_swap4.
+
+Hint Resolve PPermut_specialized2 : ppermut_rew.
+Hint Resolve PPermut_specialized1
+             PPermut_specialized3 PPermut_specialized4
+             PPermut_specialized5 PPermut_specialized6.
+
+Lemma permut_PPermut:
+forall G G', G *=* G' -> G ~=~ G'.
+intros. induction H; auto.
+transitivity y; auto.
+inversion H. PPermut_simpl.
+Qed.
+
+Close Scope permut_scope.
