Hybrid/Semantics.v
@@ -1,0 +1,2156 @@
+Require Import LFSubstitution.
+Require Import Setoid.
+Require Import LibList.
+Require Import PermutLib.
+Require Import PPermutLib.
+Require Import OkLib.
+Require Import EmptyEquivLib.
+
+Open Scope label_free_is5_scope.
+Open Scope is5_scope.
+Open Scope permut_scope.
+
+(* Notation for term typing *)
+Global Reserved Notation " G '|=' Ctx '|-' M ':::' A " (at level 70).
+
+
+(*** Definitions ::: Statics ***)
+
+
+(*
+   For each full context (that is, context and background), we require
+   that the variables - both for terms and worlds - are unique.
+*)
+Inductive types_LF: Background_LF -> Context_LF -> te_LF -> ty -> Prop :=
+
+| t_hyp_LF: forall A G w (Gamma: list (prod var ty)) v
+  (Ok_Bg: ok_Bg ((w, Gamma) :: G))
+  (HT: Mem (v, A) Gamma),
+  G |= (w, Gamma) |- hyp_LF (fte v) ::: A
+
+| t_lam_LF: forall L A B G w Gamma M
+  (Ok_Bg: ok_Bg ((w, Gamma) :: G))
+  (HT: forall v', v' \notin L ->
+    G |= (w, (v', A) :: Gamma) |- M ^t^ (hyp_LF (fte v')) ::: B),
+  G |= (w, Gamma) |- (lam_LF A M) ::: A ---> B
+
+| t_appl_LF: forall A B G w Gamma M N
+  (Ok_Bg: ok_Bg ((w, Gamma) :: G))
+  (HT1: G |= (w, Gamma) |- M ::: A ---> B)
+  (HT2: G |= (w, Gamma) |- N ::: A),
+  G |= (w, Gamma) |- (appl_LF M N) ::: B
+
+| t_box_LF: forall L A G w Gamma M
+  (Ok_Bg: ok_Bg (G & (w, Gamma)))
+  (HT: forall w', w' \notin L ->
+    G & (w, Gamma) |= (w', nil) |- M ^w^ (fwo w') ::: A),
+  G |= (w, Gamma) |- box_LF M ::: [*] A
+
+| t_unbox_LF: forall A G w Gamma M
+  (Ok_Bg: ok_Bg ((w, Gamma) :: G))
+  (HT: G |= (w, Gamma) |- M ::: [*] A),
+  G |= (w, Gamma) |- unbox_fetch_LF (fwo w) M ::: A
+
+| t_unbox_fetch_LF: forall A G w Gamma w' Gamma' M
+  (Ok_Bg: ok_Bg ((w, Gamma) :: G & (w', Gamma')))
+  (HT: (G & (w', Gamma')) |= (w, Gamma) |- M ::: [*] A),
+  forall G', (G & (w, Gamma)) ~=~ G' ->
+    G' |= (w', Gamma') |- unbox_fetch_LF (fwo w) M ::: A
+
+| t_here_LF: forall A G w Gamma M
+  (Ok_Bg: ok_Bg ((w, Gamma) :: G))
+  (HT: G |= (w, Gamma) |- M ::: A),
+  G |= (w, Gamma) |- get_here_LF (fwo w) M ::: <*> A
+
+| t_get_here_LF: forall A G w Gamma w' Gamma' M
+  (Ok_Bg: ok_Bg ((w, Gamma) :: G & (w', Gamma')))
+  (HT: G & (w', Gamma') |= (w, Gamma) |- M ::: A),
+  forall G', (G & (w, Gamma)) ~=~ G' ->
+    G' |= (w', Gamma') |- get_here_LF (fwo w) M ::: <*> A
+
+| t_letdia_LF: forall L_w L_t A B G w Gamma M N
+  (Ok_Bg: ok_Bg ((w, Gamma) :: G))
+  (HT1: G |= (w, Gamma) |- M ::: <*> A)
+  (HT2: forall v', v' \notin L_t -> forall w', w' \notin L_w ->
+    (w', (v', A) :: nil) :: G |=
+      (w, Gamma) |- (N ^w^ (fwo w')) ^t^ (hyp_LF (fte v')) ::: B),
+  G |= (w, Gamma) |- letdia_get_LF (fwo w) M N ::: B
+
+| t_letdia_get_LF: forall L_w L_t A B G w (Gamma: list (prod var ty)) Ctx' M N
+  (Ok_Bg: ok_Bg ((w, Gamma) :: G & Ctx'))
+  (HT1: G & Ctx' |= (w, Gamma) |- M ::: <*> A)
+  (HT2: forall v', v' \notin L_t -> forall w', w' \notin L_w ->
+    (w', ((v', A) :: nil)) :: G & (w, Gamma) |=
+      Ctx' |- (N ^w^ (fwo w')) ^t^ (hyp_LF (fte v')) ::: B),
+  forall G0, (G & (w, Gamma)) ~=~ G0 ->
+    G0 |= Ctx' |- letdia_get_LF (fwo w) M N ::: B
+
+where " G '|=' Ctx '|-' M ':::' A " := (types_LF G Ctx M A)
+  : label_free_is5_scope.
+
+
+(*** Definitions ::: Dynamics ***)
+
+
+Inductive value_LF: te_LF -> Prop :=
+| val_lam_LF: forall A M, value_LF (lam_LF A M)
+| val_box_LF: forall M, value_LF (box_LF M)
+| val_get_here_LF: forall M Ctx, value_LF M -> value_LF (get_here_LF Ctx M)
+.
+
+
+Global Reserved Notation " M |-> N " (at level 70).
+
+(*
+   In order to define a step of reduction we require that certain terms
+   are locally closed.
+*)
+Inductive step_LF: (te_LF * vwo) -> (te_LF * vwo) -> Prop :=
+| red_appl_lam_LF: forall ctx M A N,
+  lc_w_LF M ->
+  lc_t_n_LF 1 M -> (* or (forall x, x \notin L -> lc_t_LF (M ^t^ (fte x))) -> *)
+  lc_w_LF N -> lc_t_LF N ->
+  (appl_LF (lam_LF A M) N, ctx) |-> ( M ^t^ N , ctx)
+
+| red_unbox_fetch_box_LF: forall ctx ctx' M,
+   lc_w_n_LF 1 M -> (* or
+     (forall x, x \notin L -> lc_w_LF (M ^w^ (fwo x))) -> *)
+  lc_t_LF M ->
+  (unbox_fetch_LF ctx' (box_LF M), ctx) |-> (M ^w^ ctx, ctx)
+
+| red_letdia_get_get_here_LF: forall ctx ctx' ctx'' M N,
+  lc_w_LF M -> lc_t_LF M ->
+  lc_w_n_LF 1 N -> (* or
+     (forall x, x \notin L_w -> lc_w_LF (N ^w^ (fwo x))) -> *)
+  lc_t_n_LF 1 N -> (* or
+     (forall x, x \notin L_t -> lc_t_LF (N ^t^ (fte x))) -> *)
+  (letdia_get_LF ctx' (get_here_LF ctx'' M) N, ctx) |->
+    ((N ^w^ ctx'') ^t^ M, ctx)
+
+| red_appl_LF: forall ctx M N M'
+  (HT: (M, ctx) |-> (M', ctx)),
+  lc_w_LF M -> lc_t_LF M ->
+  lc_w_LF N -> lc_t_LF N ->
+  (appl_LF M N, ctx) |-> (appl_LF M' N, ctx)
+
+| red_unbox_fetch_LF: forall ctx' M M' ctx
+  (HT: (M, ctx') |-> (M', ctx')),
+  lc_w_LF M -> lc_t_LF M ->
+  (unbox_fetch_LF ctx' M, ctx) |-> (unbox_fetch_LF ctx' M', ctx)
+
+| red_get_here_LF: forall ctx ctx' M M'
+  (HT: (M, ctx) |-> (M', ctx)),
+  lc_w_LF M -> lc_t_LF M ->
+  (get_here_LF ctx M, ctx') |-> (get_here_LF ctx M', ctx')
+
+| red_letdia_get_LF: forall ctx ctx' M N M'
+  (HT: (M, ctx) |-> (M', ctx)),
+  lc_w_LF M -> lc_t_LF M ->
+  lc_w_n_LF 1 N -> (* or
+     (forall x, x \notin L_w -> lc_w_LF (N ^w^ (fwo x))) -> *)
+  lc_t_n_LF 1 N -> (* or
+     (forall x, x \notin L_t -> lc_t_LF (N ^t^ (fte x))) -> *)
+  (letdia_get_LF ctx M N, ctx') |-> (letdia_get_LF ctx M' N, ctx')
+
+where " M |-> N " := (step_LF M N ) : label_free_is5_scope.
+
+Inductive steps_LF : te_LF * vwo -> te_LF * vwo -> Prop :=
+| single_step_LF: forall M M' w, (M, w) |-> (M', w) -> steps_LF (M, w) (M', w)
+| multi_step_LF: forall M M' M'' w,
+  (M, w) |-> (M', w) -> steps_LF (M', w) (M'', w)
+  -> steps_LF (M, w) (M'', w)
+.
+
+
+(*** Properties ***)
+
+
+(*
+   Properties of background and context:
+   * Background is defined up to ~=~ relation
+   * Context is defined up to *=* relation
+   * Weakening rules for
+     * Background
+     * Specific element of background
+     * Main context
+*)
+
+(* Proof: simple induction on typing rules *)
+Lemma BackgroundSubsetImpl:
+forall G G' Ctx M A
+  (HT: G |= Ctx |- M ::: A)
+  (HSubst: exists GT, (G++GT) ~=~ G')
+  (H_ok: ok_Bg (Ctx :: G')),
+  G' |= Ctx |- M ::: A.
+intros;
+generalize dependent G';
+induction HT; intros.
+(* hyp *)
+constructor; auto.
+(* lam *)
+apply t_lam_LF with (L:=L \u used_t_vars ((w, Gamma)::G'));
+[assumption | intros; eapply H; auto].
+(* appl *)
+econstructor; auto.
+(* box *)
+destruct HSubst as [GT];
+apply t_box_LF with (L:=L \u used_w_vars (G' & (w, Gamma))); intros;
+[ apply ok_Bg_cons_last |
+  apply H; [ | exists GT | ] ]; auto; try PPermut_simpl;
+eapply ok_Bg_fresh_wo;
+[ apply ok_Bg_cons_last |
+  rewrite notin_union in H1; destruct H1]; auto.
+(* unbox *)
+constructor; auto.
+(* unbox_fetch *)
+destruct HSubst as [GT];
+apply t_unbox_fetch_LF with (Gamma:=Gamma) (G:=G++GT).
+apply ok_Bg_ppermut with (G:=(w', Gamma')::G'0);
+  [rewrite <- H0; rewrite <- H; rew_app | ]; auto.
+apply IHHT; [exists GT | ]; auto; try PPermut_simpl.
+apply ok_Bg_ppermut with (G:=(w', Gamma')::G'0); auto.
+rewrite <- H0; rewrite <- H; rew_app; auto.
+transitivity (G' ++ GT); PPermut_simpl; auto.
+(* here *)
+constructor; auto.
+(* get_here *)
+destruct HSubst as [GT];
+apply t_get_here_LF with (Gamma:=Gamma) (G:=G++GT).
+apply ok_Bg_ppermut with (G:=(w', Gamma')::G'0);
+  [rewrite <- H0; rewrite <- H; rew_app | ]; auto.
+apply IHHT; [exists GT | ]; auto; try PPermut_simpl;
+  apply ok_Bg_ppermut with (G:=(w', Gamma')::G'0); auto;
+  rewrite <- H0; rewrite <- H; rew_app; auto.
+rewrite <- H0; rewrite <- H; rew_app; auto.
+(* letdia *)
+apply t_letdia_LF with (A:=A) (L_t:=L_t \u used_t_vars ((w, Gamma) :: G'))
+  (L_w:=L_w \u used_w_vars ((w, Gamma)::G'));
+[  | | intros; apply H]; auto;
+destruct HSubst as [GT];
+[ exists GT; rew_app; auto |
+  rewrite notin_union in *; destruct H1; destruct H0];
+apply ok_Bg_ppermut with (G:= (w', (v', A) :: nil ) :: (w, Gamma) :: G');
+[ | apply ok_Bg_fresh_wo_te]; auto.
+(* letdia_get *)
+destruct HSubst as [GT];
+apply t_letdia_get_LF with (A:=A) (Gamma:=Gamma) (G:=G++GT)
+                           (L_t:=L_t \u used_t_vars (Ctx'::G'))
+                           (L_w:=L_w \u used_w_vars (Ctx'::G')).
+apply ok_Bg_ppermut with (G:=Ctx' :: G');
+  [rewrite <- H1; rewrite <- H0; rew_app | ]; auto.
+apply IHHT.
+  exists GT; rew_app; auto.
+  apply ok_Bg_ppermut with (G:=Ctx' :: G');
+  [ rewrite <- H1; rewrite <- H0; rew_app | ]; auto.
+  intros; apply H; auto.
+  exists GT; rew_app; auto.
+  apply ok_Bg_ppermut with (G:=(w', (v', A) :: nil) :: Ctx' :: G'); auto;
+  rewrite <- H1; rewrite <- H0;
+  assert ((G & (w, Gamma) ++ GT)  ~=~ (G ++ GT) & (w, Gamma))
+    by (symmetry; rew_app; auto);
+  rewrite H4; destruct Ctx'; auto.
+rewrite <- H1; rewrite <- H0; rew_app; auto.
+Qed.
+
+
+(*
+   Proof: using BackgroundSubsetImpl with some tweaks to remove ok_Bg from
+   assumptions.
+*)
+Lemma PPermut_bg:
+forall G Gamma w M A,
+  G |= (w, Gamma) |- M ::: A ->
+    forall G',
+      G ~=~ G' ->
+      G' |= (w, Gamma) |- M ::: A.
+intros; apply BackgroundSubsetImpl with (G:=G);
+[ | exists (@nil Context_LF) | ]; rew_app; auto;
+inversion H; subst;
+try (apply ok_Bg_ppermut with (G:=(w, Gamma) :: G); auto);
+apply ok_Bg_cons_last; auto;
+rewrite <- H6 || rewrite <- H1;
+apply ok_Bg_ppermut with (G:=(w0, Gamma0) :: G0 & (w, Gamma)); eauto.
+Qed.
+
+
+(*
+   Adding types_LF as morphism for PPermut will allow us to simply rewrite
+   PPermutations of backgrounds.
+*)
+Add Morphism types_LF : PPermut_types.
+split; intros; destruct y0;
+[ apply PPermut_bg with (G:=x) |
+  apply PPermut_bg with (G:=y) ]; auto.
+Qed.
+
+
+(* Proof: Simple induction on typing rules *)
+Lemma ContextPermutImpl:
+forall G Gamma Gamma' w M A
+  (HPerm: Gamma *=* Gamma')
+  (HT: G |= (w, Gamma) |- M ::: A),
+  G |= (w, Gamma') |- M ::: A.
+intros; generalize dependent Gamma';
+remember (w, Gamma) as Ctx; generalize dependent Gamma;
+induction HT;
+intros; simpl in *; try (inversion HeqCtx; subst).
+(* hyp *)
+constructor;
+[ eapply ok_Bg_permut |
+  eapply Mem_permut]; eauto.
+(* lam *)
+econstructor; [ eapply ok_Bg_permut | ]; eauto.
+(* appl *)
+econstructor; [ eapply ok_Bg_permut | | ]; eauto.
+(* box *)
+econstructor; [ eapply ok_Bg_permut_last | intros]; eauto;
+assert (G & (w, Gamma') ~=~ G & (w, Gamma0)) by auto;
+rewrite H1; apply HT; eauto.
+(* unbox *)
+econstructor; [ eapply ok_Bg_permut | ]; eauto.
+(* unbox_fetch *)
+apply t_unbox_fetch_LF with (G:=G) (Gamma:=Gamma); auto.
+apply ok_Bg_ppermut with (G:=(w0, Gamma) :: G & (w, Gamma0)); auto.
+assert (G & (w, Gamma'0) ~=~ (G & (w, Gamma0))) as H0 by auto;
+rewrite H0; auto.
+(* here *)
+econstructor; [ eapply ok_Bg_permut | ]; eauto.
+(* get_here *)
+apply t_get_here_LF with (G:=G) (Gamma:=Gamma); auto.
+apply ok_Bg_ppermut with (G:=(w0, Gamma) :: G & (w, Gamma0)); auto.
+assert (G & (w, Gamma'0) ~=~ (G & (w, Gamma0))) as H1 by auto;
+rewrite H1; auto.
+(* letdia *)
+econstructor; [ eapply ok_Bg_permut | | ]; eauto.
+(* letdia_get *)
+apply t_letdia_get_LF with (L_w:=L_w) (L_t:=L_t) (A:=A) (Gamma:=Gamma) (G:=G).
+apply ok_Bg_ppermut with (G:=(w0, Gamma) :: G & (w, Gamma0)); auto.
+assert (G & (w, Gamma') ~=~ (G & (w, Gamma0))) as H2 by auto;
+rewrite H2; auto.
+intros; eapply H; eauto.
+auto.
+Qed.
+
+
+(* Weakening lemmas *)
+
+Lemma GlobalWeakening:
+forall G G' Ctx Ctx' M A
+  (HT: G ++ G' |= Ctx |- M ::: A)
+  (H_ok: ok_Bg (Ctx :: G & Ctx' ++ G')),
+  G & Ctx' ++ G' |= Ctx |- M ::: A.
+intros; rew_app;
+apply BackgroundSubsetImpl with (G:=G++G'); auto;
+[ exists (Ctx'::nil); rew_app; symmetry |
+  rew_app in *]; auto.
+Qed.
+
+(*
+Proof: induction on typing
+  * we need to be carefull when switching contexts - it's important to know
+  if the context we're switching to is the one we intend to extend
+  * if it is the case, it implies certain equivalences between pairs of
+  backgrounds, which then help to use the induction hypothesis
+  * otherwise we have to deconstruct background in order to extract the context
+  that we want to switch
+*)
+Lemma Weakening_general:
+  forall G w Gamma M A
+  (HT: G |= (w, Gamma) |- M ::: A),
+  (forall G' w' Delta Delta',
+    G ~=~ (G' & (w', Delta)) ->
+    ok_Bg ((w, Gamma) :: G' & (w', Delta ++ Delta')) ->
+    G' & (w', Delta ++ Delta') |= (w, Gamma) |- M ::: A) /\
+  (forall Gamma',
+    ok_Bg ((w, Gamma ++ Gamma') :: G) ->
+    G |= (w, Gamma ++ Gamma') |- M ::: A).
+intros;
+remember (w, Gamma) as Ctx;
+generalize dependent Gamma;
+generalize dependent w;
+induction HT; split;
+intros; subst; simpl;
+try (inversion HeqCtx; subst).
+(* hyp *)
+constructor; auto.
+constructor; auto; rewrite Mem_app_or_eq; left; assumption.
+(* lam *)
+apply t_lam_LF with
+  (L:=L \u used_t_vars ((w0, Gamma0) :: G' & (w', Delta ++ Delta')));
+[ | intros; eapply H]; auto.
+apply t_lam_LF with (L:=L \u used_t_vars ((w0, Gamma0++Gamma')::G));
+[ | intros; eapply H with (v':=v')  (w:=w0) (Gamma:=(v' ,A)::Gamma0)]; auto;
+rew_app; auto.
+(* appl *)
+econstructor; [ | eapply IHHT1| eapply IHHT2]; eauto.
+econstructor; [ | eapply IHHT1| eapply IHHT2]; eauto.
+(* box *)
+apply t_box_LF with
+  (L:=L \u used_w_vars (G' & (w0, Gamma0) & (w', Delta ++ Delta')));
+intros;
+assert (G' & (w', Delta ++ Delta') & (w0, Gamma0) ~=~
+        G' & (w0, Gamma0) & (w', Delta ++ Delta')) by (rew_app; auto);
+[ apply ok_Bg_ppermut with (G:=(w0, Gamma0) :: G' & (w', Delta ++ Delta')) |
+  rewrite H3]; auto; try PPermut_simpl;
+apply H with (w:=w'0) (Gamma:=nil);
+[ | | rewrite H0 | rewrite H0 in Ok_Bg]; auto; try PPermut_simpl.
+apply ok_Bg_fresh_wo; auto;
+apply ok_Bg_ppermut with
+  (G:=((w0, Gamma0) :: G' & (w', Delta ++ Delta')));
+auto.
+apply t_box_LF with (L:=L \u used_w_vars (G & (w0, Gamma0++Gamma')));
+[ apply ok_Bg_ppermut with (G:= (w0, Gamma0++Gamma') :: G) |
+  intros; eapply H]; auto; try PPermut_simpl;
+apply ok_Bg_fresh_wo; auto;
+apply ok_Bg_ppermut with (G:=(w0, Gamma0++Gamma')::G); auto; PPermut_simpl.
+(* unbox *)
+constructor; [ | eapply IHHT]; eauto.
+constructor; [ | eapply IHHT]; eauto.
+(* unbox_fetch 1 *)
+destruct (permut_context_LF_dec (w'0, Delta) (w, Gamma)) as [Eq|Neq];
+simpl in *.
+(* = *)
+destruct Eq; subst;
+assert (G ~=~ G'0) by
+   (apply PPermut_last_rev with (Gamma := Gamma) (Gamma':= Delta) (w:=w);
+    [ apply permut_sym |
+      transitivity G' ]; auto);
+assert ((w0, Gamma0) :: G'0 & (w, Delta ++ Delta') ~=~
+        (w, Gamma ++ Delta') :: G & (w0, Gamma0)) by
+  (rewrite H3;
+   transitivity ((w, Delta ++ Delta') :: G'0 & (w0, Gamma0));
+     [ transitivity ((w0, Gamma0) :: (w, Delta ++ Delta') :: G'0) | ]; auto;
+       transitivity ((w, Delta ++ Delta') :: (w0, Gamma0) :: G'0);
+       auto; PPermut_simpl);
+apply t_unbox_fetch_LF with (G:=G) (Gamma:=Gamma++Delta');
+[rewrite <- H4 | apply IHHT | rewrite H3]; auto; rewrite <- H4; auto.
+(* <> *)
+assert (exists Gamma', exists G0, exists G1,
+  Gamma' *=* Gamma /\ G'0 = G0 & (w, Gamma') ++ G1) as H2 by
+  ( apply PPermut_split_neq with (G':=G) (w:=w'0) (Gamma := Delta);
+    [ symmetry; transitivity G' | ]; auto);
+destruct H2 as (Gamma', (GH, (GT, (H2a, H2b)))); subst;
+apply t_unbox_fetch_LF with
+  (Gamma:=Gamma) (G:=GH ++ GT & (w'0, Delta ++ Delta')).
+apply ok_Bg_ppermut with
+  (G := (w0, Gamma0) :: (GH & (w, Gamma) ++ GT) & (w'0, Delta ++ Delta')); auto.
+rew_app; PPermut_simpl.
+assert ((w0, Gamma0) :: (GH & (w, Gamma) ++ GT) & (w'0, Delta ++ Delta') ~=~
+       ((w0, Gamma0) :: (GH & (w, Gamma') ++ GT) & (w'0, Delta ++ Delta')))
+  by PPermut_simpl.
+rewrite H2; auto.
+apply PPermut_bg with (G:= (GH ++ GT & (w0, Gamma0)) & (w'0, Delta ++ Delta')).
+  apply IHHT with (w1:=w) (Gamma1:=Gamma) (G':=GH ++ GT & (w0, Gamma0));
+  assert (G ~=~ GH ++ GT & (w'0, Delta)) by
+  ( apply PPermut_last_rev_simpl with (a:=(w, Gamma)); auto; transitivity G';
+     [ | rewrite H0]; auto; PPermut_simpl);
+  auto; try PPermut_simpl.
+  apply ok_Bg_ppermut with (G:= (w0, Gamma0) :: GH ++ (w, Gamma) :: GT &
+     (w'0, Delta ++ Delta')); auto; try PPermut_simpl.
+  assert ((w0, Gamma0) :: GH ++ (w, Gamma) :: GT & (w'0, Delta ++ Delta') ~=~
+       ((w0, Gamma0) :: (GH & (w, Gamma') ++ GT) & (w'0, Delta ++ Delta')))
+  by PPermut_simpl.
+  rewrite H3; auto.
+  transitivity (((w0, Gamma0) :: GH ++ GT) &
+    (w'0, Delta++Delta')); [rew_app | ]; auto; PPermut_simpl.
+  transitivity (((w, Gamma) :: GH ++ GT ) &
+    (w'0, Delta ++ Delta')); [ | rew_app]; auto; PPermut_simpl.
+(* unbox_fetch 2 *)
+apply t_unbox_fetch_LF with (G:=G) (Gamma:=Gamma);
+rewrite <- H in H0; [ | apply IHHT with (w1:=w) (Gamma1:=Gamma) |]; auto.
+(* here *)
+constructor; [ | apply IHHT with (w:=w0)(Gamma:=Gamma0)]; auto.
+constructor; [ | apply IHHT]; auto.
+(* get_here 1 *)
+destruct (permut_context_LF_dec (w'0, Delta) (w, Gamma)) as [Eq|Neq];
+simpl in *.
+(* = *)
+destruct Eq; subst;
+assert (G ~=~ G'0) by
+   (apply PPermut_last_rev with (Gamma := Gamma) (Gamma':= Delta) (w:=w);
+    [ apply permut_sym |
+      transitivity G' ]; auto);
+assert ((w0, Gamma0) :: G'0 & (w, Delta ++ Delta') ~=~
+        (w, Gamma ++ Delta') :: G & (w0, Gamma0)) by
+  (rewrite H3;
+   transitivity ((w, Delta ++ Delta') :: G'0 & (w0, Gamma0));
+     [ transitivity ((w0, Gamma0) :: (w, Delta ++ Delta') :: G'0) | ]; auto;
+       transitivity ((w, Delta ++ Delta') :: (w0, Gamma0) :: G'0);
+       auto; PPermut_simpl);
+apply t_get_here_LF with (G:=G) (Gamma:=Gamma++Delta');
+[rewrite <- H4 | apply IHHT | rewrite H3]; auto; rewrite <- H4; auto.
+(* <> *)
+assert (exists Gamma', exists G0, exists G1,
+  Gamma' *=* Gamma /\ G'0 = G0 & (w, Gamma') ++ G1) as H2 by
+  ( apply PPermut_split_neq with (G':=G) (w:=w'0) (Gamma := Delta);
+    [ symmetry; transitivity G' | ]; auto);
+destruct H2 as (Gamma', (GH, (GT, (H2a, H2b)))); subst;
+apply t_get_here_LF with
+  (Gamma:=Gamma) (G:=GH ++ GT & (w'0, Delta ++ Delta')).
+apply ok_Bg_ppermut with
+  (G := (w0, Gamma0) :: (GH & (w, Gamma) ++ GT) & (w'0, Delta ++ Delta')); auto.
+rew_app; PPermut_simpl.
+assert ((w0, Gamma0) :: (GH & (w, Gamma) ++ GT) & (w'0, Delta ++ Delta') ~=~
+       ((w0, Gamma0) :: (GH & (w, Gamma') ++ GT) & (w'0, Delta ++ Delta')))
+  by PPermut_simpl.
+rewrite H2; auto.
+apply PPermut_bg with (G:= (GH ++ GT & (w0, Gamma0)) & (w'0, Delta ++ Delta')).
+  apply IHHT with (w1:=w) (Gamma1:=Gamma) (G':=GH ++ GT & (w0, Gamma0));
+  assert (G ~=~ GH ++ GT & (w'0, Delta)) by
+  ( apply PPermut_last_rev_simpl with (a:=(w, Gamma)); auto; transitivity G';
+     [ | rewrite H0]; auto; PPermut_simpl);
+  auto; try PPermut_simpl.
+  apply ok_Bg_ppermut with (G:= (w0, Gamma0) :: GH ++ (w, Gamma) :: GT &
+     (w'0, Delta ++ Delta')); auto; try PPermut_simpl.
+  assert ((w0, Gamma0) :: GH ++ (w, Gamma) :: GT & (w'0, Delta ++ Delta') ~=~
+       ((w0, Gamma0) :: (GH & (w, Gamma') ++ GT) & (w'0, Delta ++ Delta')))
+  by PPermut_simpl.
+  rewrite H3; auto.
+  transitivity (((w0, Gamma0) :: GH ++ GT) &
+    (w'0, Delta++Delta')); [rew_app | ]; auto; PPermut_simpl.
+  transitivity (((w, Gamma) :: GH ++ GT ) &
+    (w'0, Delta ++ Delta')); [ | rew_app]; auto; PPermut_simpl.
+(* get_here 2 *)
+apply t_get_here_LF with (G:=G) (Gamma:=Gamma);
+rewrite <- H in H0; [ | apply IHHT with (w1:=w) (Gamma1:=Gamma) |]; auto.
+(* letdia *)
+apply t_letdia_LF with (A:=A)
+  (L_w:=L_w \u used_w_vars((w0, Gamma0) :: G' & (w', Delta ++ Delta')))
+  (L_t:=L_t \u used_t_vars ((w0, Gamma0) :: G' & (w', Delta ++ Delta')));
+[ | apply IHHT with (w:=w0) (Gamma:=Gamma0) | ]; auto;
+intros; destruct H with (v':=v') (w':=w'0) (w:=w0) (Gamma:=Gamma0); auto;
+replace ((w'0, (v', A) :: nil) :: G' & (w', Delta ++ Delta')) with
+   (((w'0, (v', A) :: nil) :: G') & (w', Delta ++ Delta')) by
+   (rew_app; reflexivity);
+apply H4; rew_app; auto;
+apply ok_Bg_ppermut with
+  (G:=(w'0, (v', A) :: nil) :: (w0, Gamma0) :: G' & (w', Delta ++ Delta'));
+auto.
+eapply t_letdia_LF with (A:=A)
+  (L_t := L_t \u used_t_vars ((w0, Gamma0 ++ Gamma') :: G))
+  (L_w := L_w \u used_w_vars ((w0, Gamma0 ++ Gamma') :: G));
+[ | apply IHHT | ]; auto;
+intros; eapply H; auto;
+apply ok_Bg_ppermut with
+  (G:=(w', (v', A) :: nil) :: (w0, Gamma0 ++ Gamma') :: G);
+auto.
+(* letdia_get 1 *)
+destruct (permut_context_LF_dec (w', Delta) (w, Gamma)) as [Eq | Neq];
+simpl in *.
+(* = *)
+destruct Eq; subst;
+assert (G ~=~ G') by
+  (apply PPermut_last_rev with (w:=w) (Gamma:=Gamma) (Gamma':=Delta);
+   [apply permut_sym | transitivity G0]; auto);
+apply t_letdia_get_LF with (Gamma:=Gamma++Delta') (G:=G) (A:=A)
+  (L_w:=L_w \u used_w_vars ((w0, Gamma0) :: G' & (w, Gamma ++ Delta')))
+  (L_t:=L_t \u used_t_vars ((w0, Gamma0) :: G & (w, Gamma ++ Delta'))).
+apply ok_Bg_ppermut with (G:=(w0, Gamma0) :: G' & (w, Delta ++ Delta'));
+[rewrite <- H4 | auto];
+transitivity ((w, Delta ++ Delta') :: G & (w0, Gamma0)); auto.
+apply IHHT; auto;
+apply ok_Bg_ppermut with (G:=(w0, Gamma0) :: G' & (w, Delta ++ Delta'));
+[rewrite <- H4 | auto];
+transitivity ((w, Delta ++ Delta') :: G & (w0, Gamma0)); auto.
+intros; destruct H with (v':=v') (w':=w') (w1:=w0) (Gamma1:=Gamma0); eauto;
+replace ( (w', (v', A) :: nil) :: G & (w, Gamma ++ Delta') ) with
+  (( (w', (v', A) :: nil) :: G) & (w, Gamma ++ Delta')) by
+  (rew_app; reflexivity);
+eapply H7; auto;
+apply ok_Bg_ppermut with
+  (G:=(w', (v', A) :: nil ) :: (w0, Gamma0) :: G & (w, Gamma ++ Delta'));
+[ rew_app | rewrite H4]; auto;
+apply ok_Bg_fresh_wo_te;
+[ apply ok_Bg_ppermut with (G:=(w0, Gamma0) :: G' & (w, Delta ++ Delta')) | | ];
+auto.
+rewrite notin_union in *; destruct H5; auto;
+rewrite <- H4; auto.
+rewrite <- H4; auto.
+(* <> *)
+assert (exists Gamma', exists G0, exists G1,
+  Gamma' *=* Gamma /\ G' = G0 & (w, Gamma') ++ G1) by
+  ( apply PPermut_split_neq with (G':=G) (w:=w') (Gamma := Delta);
+    [ symmetry; transitivity G0 | ]; auto).
+destruct H3 as (Gamma', (GH, (GT, (H3a, H3b)))); subst;
+assert ((w0, Gamma0) :: (GH & (w, Gamma') ++ GT) & (w', Delta ++ Delta') ~=~
+  (w0, Gamma0) :: (GH & (w, Gamma) ++ GT) & (w', Delta ++ Delta'))
+by PPermut_simpl;
+assert (G ~=~ GH ++ GT & (w', Delta)) by
+  ( apply PPermut_last_rev_simpl with (a:=(w, Gamma));
+    transitivity G0; auto; rewrite H1; PPermut_simpl);
+apply t_letdia_get_LF with
+  (Gamma:=Gamma) (G:=GH ++ GT & (w', Delta ++ Delta'))
+  (L_w:=L_w \u used_w_vars ((w0, Gamma0) :: (GH & (w, Gamma) ++ GT) &
+    (w', Delta ++ Delta')))
+  (L_t:=L_t \u used_t_vars ((w0, Gamma0) :: (GH & (w, Gamma) ++ GT) &
+    (w', Delta ++ Delta')))(A:=A).
+apply ok_Bg_ppermut with
+  (G:=(w0, Gamma0) :: (GH & (w, Gamma') ++ GT) & (w', Delta ++ Delta'));
+rew_app in *; auto; try PPermut_simpl.
+apply PPermut_bg with (G:= (GH ++ GT & (w0, Gamma0)) & (w', Delta ++ Delta'));
+[ | rew_app]; auto;
+apply IHHT with (w1:=w) (Gamma1:=Gamma); auto;
+[ rewrite H4 | ]; rew_app; auto;
+rew_app; apply ok_Bg_ppermut with
+  (G:=(w0, Gamma0) :: (GH & (w, Gamma') ++ GT) & (w', Delta ++ Delta')); auto;
+rew_app; try PPermut_simpl.
+intros; destruct H with (v':=v')(w':=w'0) (w1:=w0) (Gamma1:=Gamma0); auto;
+apply PPermut_bg with
+  (G:=((w'0, (v', A)::nil) :: GH++GT & (w, Gamma)) & (w', Delta ++ Delta'));
+[ | rew_app]; auto;
+apply H7; rew_app; [constructor | ]; auto;
+[ rewrite H4; rew_app; auto | ];
+apply ok_Bg_ppermut with
+  (G:= ((w'0, (v', A) :: nil) ::(w0, Gamma0) :: GH & (w, Gamma') ++ GT) &
+    (w', Delta ++ Delta')); rew_app; auto;
+[ transitivity (((w'0, (v', A) :: nil) ::(w0, Gamma0) :: GH ++GT & (w, Gamma))
+  & (w', Delta ++ Delta')); rew_app |
+ rew_app in *; apply ok_Bg_fresh_wo_te]; auto; try PPermut_simpl.
+rewrite H3; auto.
+rewrite H3; auto.
+rew_app; PPermut_simpl.
+(* letdia_get 2 *)
+apply t_letdia_get_LF with (G:=G) (Gamma:=Gamma) (A:=A)
+  (L_w:=L_w \u used_w_vars (((w0, Gamma0 ++ Gamma') :: G & (w, Gamma))))
+  (L_t:=L_t \u used_t_vars ((w0, Gamma0 ++ Gamma') :: G & (w, Gamma))).
+rewrite <- H0 in H1; apply ok_Bg_ppermut with
+  (G:=(w0, Gamma0 ++ Gamma') :: G & (w, Gamma)); auto.
+apply IHHT with (w1:=w) (Gamma1:=Gamma); auto.
+rewrite <- H0 in H1; apply ok_Bg_ppermut with
+  (G:=(w0, Gamma0 ++ Gamma') :: G & (w, Gamma)); auto.
+intros; destruct H with (v':=v')(w':=w') (w1:=w0)(Gamma1:=Gamma0); auto;
+apply H5; apply ok_Bg_ppermut with
+  (G:= (w', (v', A)::nil) :: (w0, Gamma0 ++ Gamma') :: G & (w, Gamma));
+[ | apply ok_Bg_fresh_wo_te ]; auto; rewrite H0; auto.
+assumption.
+Qed.
+
+Lemma WeakeningBackgroundElem:
+forall G G' w Delta Delta' Ctx M A
+  (H_ok: ok_Bg (Ctx :: G & (w, Delta ++ Delta') ++ G'))
+  (HT: G & (w, Delta) ++ G' |= Ctx |- M ::: A),
+  G & (w, Delta ++ Delta') ++ G' |= Ctx |- M ::: A.
+intros;
+assert ( G & (w, Delta ++ Delta') ++ G' ~=~ (G++G') & (w, Delta ++ Delta'))
+  by (rew_app; auto);
+rewrite H;
+destruct Ctx; eapply Weakening_general; auto.
+rew_app; assert (G ++ G' & (w, Delta) ~=~ G & (w, Delta) ++ G') by auto;
+rewrite H0; assumption.
+apply ok_Bg_ppermut with (G:=(v, l) :: G & (w, Delta ++ Delta') ++ G'); auto.
+Qed.
+
+Lemma Weakening:
+forall G w Gamma Gamma' M A
+  (H_ok: ok_Bg ((w,Gamma++Gamma')::G))
+  (HT: G |= (w, Gamma) |- M ::: A),
+  G |= (w, Gamma ++ Gamma') |- M ::: A.
+intros;
+eapply Weakening_general; eassumption.
+Qed.
+
+(*
+   When we can prove something in empty context and background, then we
+   can also do it in any "full" version of this context & background
+*)
+Lemma types_weakened:
+forall G G' w Gamma M A
+  (Ok: ok_Bg ((w, Gamma)::G ++ G'))
+  (HT: emptyEquiv G ++ G' |= (w, nil) |- M ::: A),
+  G ++ G'|= (w, Gamma) |- M ::: A.
+induction G; intros; simpl in *; rew_app in *; auto.
+apply Weakening with (Gamma':=Gamma) in HT; rew_app in *; auto.
+destruct a; rew_app in *.
+assert ((v,l) :: G ++ G' ~=~ G ++ (v,l)::G') by PPermut_simpl;
+rewrite H; apply IHG.
+rewrite <- H; auto.
+assert (emptyEquiv G ++ (v, l) :: G' ~=~ emptyEquiv G & (v, nil ++ l) ++ G')
+  by PPermut_simpl; rewrite H0; eapply WeakeningBackgroundElem.
+rew_app.
+apply ok_Bg_empty_first in Ok.
+assert ((w, nil) :: (v, l) :: G ++ G' ~=~ ((w, nil) :: G) ++ (v, l) :: G') by
+  PPermut_simpl; rewrite H1 in Ok;
+eapply emptyEquiv_ok_Bg_part in Ok; simpl in *; rew_app in *; auto.
+assert (emptyEquiv G & (v, nil) ++ G' ~=~  (v, nil) :: emptyEquiv G ++ G') by
+  PPermut_simpl; rewrite H1; auto.
+Qed.
+
+
+(* Type preservation under various types of substitution *)
+
+
+(*
+Proof: induction on typing
+  * for hypothesis case we simply use weakening
+  * for cases where we change worlds, we have to find the element, for
+  which the substitution is defined - in other words, the context, from
+  which the variable to substitute comes from; there are always two
+  options: either it is the marked element or we have to do a manual
+  split in order to find it
+*)
+Lemma subst_t_preserv_types:
+forall G w Gamma B M N v A
+  (H_lc_t: lc_t_LF M)
+  (H_lc_w: lc_w_LF M)
+  (HT: G |= (w, Gamma) |- N ::: B),
+  (* "inner" substitution *)
+  ( forall Gamma0,
+    permut Gamma ((v, A) :: Gamma0) ->
+    emptyEquiv G |= (w, nil) |- M ::: A ->
+    G |= (w, Gamma0) |- [M // fte v] N ::: B)
+  /\
+  (* "outer" substitution *)
+  ( forall G0 G' G'' w' Gamma',
+    G ~=~ (G0 & (w', (v,A)::Gamma')) ->
+    G' ~=~ (G0 & (w, Gamma)) ->
+    G'' ~=~ (G0 & (w', Gamma')) ->
+    emptyEquiv G' |= (w', nil) |- M ::: A ->
+    G'' |= (w, Gamma) |- [M // fte v] N ::: B).
+intros;
+remember (w, Gamma) as Ctx;
+generalize dependent v;
+generalize dependent A;
+generalize dependent M;
+generalize dependent w;
+generalize dependent Gamma;
+induction HT; split; intros;
+inversion HeqCtx; subst;
+simpl in *.
+
+(* hyp *)
+case_if.
+inversion H1; subst;
+assert (A = A0) by (eapply ok_Bg_Mem_eq; eauto);
+subst; replace G with (G ++ nil) by (rew_app; auto);
+apply types_weakened;
+[eapply ok_Bg_permut_first_tail with (C:=Gamma0) | ]; rew_app; eauto.
+constructor;
+[ apply ok_Bg_permut_first_tail with (C:=Gamma0) (x:=v0) (A:=A0) |
+  apply Mem_permut with (l' := (v0, A0) :: Gamma1) in HT]; eauto.
+rewrite Mem_cons_eq in HT; destruct HT; auto;
+inversion H2; subst; elim H1; reflexivity.
+
+case_if.
+inversion H3; subst;
+eapply ok_Bg_Mem_contradict in Ok_Bg;
+contradiction || eauto.
+constructor; auto;
+apply ok_Bg_ppermut with (G:=((w0, Gamma0)::G0) & (w', Gamma'));
+[ rewrite H1 |
+  eapply ok_Bg_permut_no_last; rewrite H in Ok_Bg; rew_app]; eauto.
+
+(* lam *)
+apply t_lam_LF with (L:=L \u \{v});
+[ apply ok_Bg_permut_first_tail with (C:=Gamma0) (x:=v) (A:=A0) |
+  intros]; auto;
+rewrite notin_union in H2; rewrite notin_singleton in H2; destruct H2;
+unfold open_t in *;
+rewrite <- subst_t_comm; auto;
+eapply H; auto;
+permut_simpl || rew_app; eauto.
+
+apply t_lam_LF with (L:=L \u \{v});
+[ apply ok_Bg_ppermut with (G:=((w0, Gamma0)::G0) & (w', Gamma'));
+  [ rewrite H2 |
+    rewrite H0 in Ok_Bg; rew_app] |
+  intros]; eauto with ok_bg_rew;
+rewrite notin_union in H4; rewrite notin_singleton in H4; destruct H4;
+unfold open_t in *;
+rewrite <- subst_t_comm; auto;
+eapply H with (G0:=G0) (w':=w'); eauto;
+assert (emptyEquiv G' ~=~ emptyEquiv (G0 ++ nil & (w0, (v', A) :: Gamma0))) as E
+ by (rewrite H1; rew_app; eapply emptyEquiv_last_change; auto);
+rew_app in *; rewrite <- E; auto.
+
+(* appl *)
+econstructor;  [ | eapply IHHT1 | eapply IHHT2];
+try apply ok_Bg_permut_first_tail with (C:=Gamma0) (x:=v) (A:=A0); eauto.
+
+econstructor;
+[ apply ok_Bg_ppermut with (G:=((w0, Gamma0)::G0) & (w', Gamma'));
+  [rewrite H1 | rewrite H in Ok_Bg] |
+  eapply IHHT1 |
+  eapply IHHT2]; eauto;
+apply ok_Bg_permut_no_last_spec in Ok_Bg; rew_app; auto.
+
+(* box *)
+apply t_box_LF with (L:=L \u used_w_vars (emptyEquiv G & (w0, nil)));
+[ apply ok_Bg_permut_no_last with (v:=v) (A:=A0);
+  eapply ok_Bg_permut_last |
+  intros; unfold open_w]; eauto;
+rewrite <- subst_order_irrelevant_bound;
+[ eapply H; eauto |
+  repeat rewrite emptyEquiv_rewrite];
+simpl; rew_app; auto;
+apply BackgroundSubsetImpl with (G:=emptyEquiv G); auto;
+[ exists ((w', (@nil (prod var ty))) :: nil); rew_app; auto |
+  assert ((w0, nil) :: emptyEquiv G & (w', nil) ~=~
+    (w', nil) :: emptyEquiv G & (w0, nil)) by auto];
+rew_app; rewrite emptyEquiv_rewrite_last; simpl; auto;
+rewrite H3;
+apply ok_Bg_fresh_wo; auto;
+apply emptyEquiv_ok_Bg in Ok_Bg;
+rewrite emptyEquiv_rewrite in Ok_Bg;
+simpl in *; auto.
+
+apply t_box_LF with
+  (L:=L \u used_w_vars(emptyEquiv G0 ++ (w', nil) :: (w0, nil) :: nil));
+[ rewrite H2; rewrite H0 in Ok_Bg |
+  intros; unfold open_w; rewrite <- subst_order_irrelevant_bound];
+eauto with ok_bg_rew;
+eapply H with (G'' := G'' & (w0, Gamma0)) (G0:=G0 & (w0, Gamma0)) (w'0:=w')
+  (Gamma':=Gamma') (A0:=A0); auto;
+repeat rewrite emptyEquiv_rewrite;
+simpl; rew_app; try PPermut_simpl;
+apply BackgroundSubsetImpl with (G:=emptyEquiv G0 & (w0, nil));
+[ rewrite H1 in H3; rewrite emptyEquiv_rewrite in H3 |
+  exists ((w'0, (@nil (var * ty)))::nil); rew_app |
+  apply emptyEquiv_ok_Bg in Ok_Bg; rewrite H0 in Ok_Bg]; auto;
+repeat rewrite emptyEquiv_rewrite in Ok_Bg;
+simpl in *; rew_app in *;
+apply ok_Bg_ppermut with
+  (G:=(w'0, nil) :: emptyEquiv G0 ++ (w', nil) :: (w0, nil) :: nil);
+[eauto with ppermut_rew | apply ok_Bg_fresh_wo ]; auto.
+
+(* unbox *)
+econstructor; [ | eapply IHHT];
+try apply ok_Bg_permut_first_tail with (C:=Gamma0) (x:=v) (A:=A0); eauto.
+
+econstructor;
+[ rewrite H1; rewrite H in Ok_Bg |
+  eapply IHHT]; eauto with ok_bg_rew.
+
+(* unbox_fetch *)
+apply t_unbox_fetch_LF with (G:=G) (Gamma:=Gamma); auto;
+[ apply ok_Bg_permut_no_last_spec with (v:=v) (A:=A0);
+  apply ok_Bg_ppermut with (G:= (w, Gamma) :: G & (w0, Gamma0)) |
+  eapply IHHT; eauto; rewrite <- H in H1; rew_app]; auto.
+
+destruct (eq_var_dec w w'0).
+(* = *)
+subst;
+assert (G ~=~ G0 /\ Gamma *=* (v, A0) :: Gamma'0) as HP by
+  (apply ok_Bg_impl_ppermut with (w:=w'0);
+   [eauto with ok_bg_rew | transitivity G'; auto]);
+destruct HP;
+apply t_unbox_fetch_LF with (G:=G) (Gamma:=Gamma'0);
+eauto with ok_bg_rew;
+specialize IHHT with (Gamma1:=Gamma) (w:=w'0);
+destruct IHHT with (M0:=M0) (A0:=A0) (v:=v); auto;
+[ apply H6; auto; rewrite H1 in H3; rewrite H4 |
+  rewrite H4; symmetry]; auto.
+(* <> *)
+assert (exists Gamma', exists GH, exists GT,
+  Gamma' *=* (v, A0)::Gamma'0 /\ G = GH & (w'0, Gamma') ++ GT) as HP by
+  (apply PPermut_split_neq with (w:=w) (Gamma:=Gamma) (G':=G0);
+    auto; transitivity G'; auto).
+destruct HP as (Gamma', (GH, (GT, (HPa, HPb)))).
+assert (GH & (w'0, Gamma') ++ GT ~=~ GH & (w'0, (v, A0)::Gamma'0) ++ GT)
+  by PPermut_simpl;
+apply t_unbox_fetch_LF with (G:=GH ++ GT & (w'0, Gamma'0)) (Gamma:=Gamma).
+subst;
+apply ok_Bg_ppermut with
+  (G:= (((w, Gamma) :: (GH & (w0, Gamma0) ++ GT)) & (w'0, Gamma'0)));
+[rew_app | ]; auto;
+apply ok_Bg_permut_no_last_spec with (v:=v)(A:=A0).
+apply ok_Bg_ppermut with
+  (G:=(w, Gamma):: (GH & (w'0, Gamma') ++ GT) & (w0, Gamma0));
+rew_app in *; auto; PPermut_simpl.
+eapply IHHT with (w1:=w) (Gamma1:=Gamma) (w':=w'0) (Gamma':=Gamma'0)
+                 (G0:=GH ++ GT & (w0, Gamma0)); rew_app; auto; subst;
+rew_app; auto;
+rewrite H1 in H3;
+assert (GH ++ (w, Gamma) :: GT ~=~ G0) by
+  (apply PPermut_last_rev_simpl with (a:=(w'0, (v, A0) :: Gamma'0));
+  rew_app in *; rewrite <- H0; rewrite <- H; auto; PPermut_simpl).
+PPermut_simpl; eauto.
+assert (GH ++ (w, Gamma) :: GT & (w0, Gamma0) ~=~ G0 & (w0,Gamma0)) by
+  (rewrite <- H5; rew_app; auto; PPermut_simpl);
+rewrite H6; auto.
+subst; rewrite H2; PPermut_simpl.
+apply PPermut_last_rev with (w:=w'0) (Gamma:=Gamma') (Gamma':=(v,A0)::Gamma'0);
+[ | symmetry]; auto; transitivity G'; auto; rewrite <- H; PPermut_simpl.
+
+(* here *)
+econstructor; [ | eapply IHHT];
+try apply ok_Bg_permut_first_tail with (C:=Gamma0) (x:=v) (A:=A0); eauto.
+
+econstructor;
+[ rewrite H1; rewrite H in Ok_Bg |
+  eapply IHHT]; eauto with ok_bg_rew.
+
+(* get_here *)
+apply t_get_here_LF with (G:=G) (Gamma:=Gamma); auto;
+[ apply ok_Bg_permut_no_last_spec with (v:=v) (A:=A0);
+  apply ok_Bg_ppermut with (G:= (w, Gamma) :: G & (w0, Gamma0)) |
+  eapply IHHT; eauto; rewrite <- H in H1; rew_app]; auto.
+
+destruct (eq_var_dec w w'0).
+(* = *)
+subst;
+assert (G ~=~ G0 /\ Gamma *=* (v, A0) :: Gamma'0) as HP by
+  (apply ok_Bg_impl_ppermut with (w:=w'0);
+   [eauto with ok_bg_rew | transitivity G'; auto]);
+destruct HP;
+apply t_get_here_LF with (G:=G) (Gamma:=Gamma'0);
+eauto with ok_bg_rew;
+specialize IHHT with (Gamma1:=Gamma) (w:=w'0);
+destruct IHHT with (M0:=M0) (A0:=A0) (v:=v); auto;
+[ apply H6; auto; rewrite H1 in H3; rewrite H4 |
+  rewrite H4; symmetry]; auto.
+(* <> *)
+assert (exists Gamma', exists GH, exists GT,
+  Gamma' *=* (v, A0)::Gamma'0 /\ G = GH & (w'0, Gamma') ++ GT) as HP by
+  (apply PPermut_split_neq with (w:=w) (Gamma:=Gamma) (G':=G0);
+    eauto; transitivity G'; auto).
+destruct HP as (Gamma', (GH, (GT, (HPa, HPb)))).
+assert (GH & (w'0, Gamma') ++ GT ~=~ GH & (w'0, (v, A0)::Gamma'0) ++ GT)
+  by PPermut_simpl;
+apply t_get_here_LF with (G:=GH ++ GT & (w'0, Gamma'0)) (Gamma:=Gamma).
+subst;
+apply ok_Bg_ppermut with
+  (G:= (((w, Gamma) :: (GH & (w0, Gamma0) ++ GT)) & (w'0, Gamma'0)));
+[rew_app | ]; auto;
+apply ok_Bg_permut_no_last_spec with (v:=v)(A:=A0).
+apply ok_Bg_ppermut with
+  (G:=(w, Gamma):: (GH & (w'0, Gamma') ++ GT) & (w0, Gamma0));
+rew_app in *; auto; PPermut_simpl.
+eapply IHHT with (w1:=w) (Gamma1:=Gamma) (w':=w'0) (Gamma':=Gamma'0)
+                 (G0:=GH ++ GT & (w0, Gamma0)) (A0:=A0); rew_app; auto; subst;
+rew_app; auto;
+rewrite H1 in H3;
+assert (GH ++ (w, Gamma) :: GT ~=~ G0) by
+  (apply PPermut_last_rev_simpl with (a:=(w'0, (v, A0) :: Gamma'0));
+  rew_app in *; rewrite <- H0; rewrite <- H; auto; PPermut_simpl).
+PPermut_simpl; auto.
+assert (GH ++ (w, Gamma) :: GT & (w0, Gamma0) ~=~ G0 & (w0,Gamma0)) by
+  (rewrite <- H5; rew_app; auto; PPermut_simpl);
+rewrite H6; auto.
+subst; rewrite H2; PPermut_simpl.
+apply PPermut_last_rev with (w:=w'0) (Gamma:=Gamma') (Gamma':=(v,A0)::Gamma'0);
+[ | symmetry]; auto; transitivity G'; auto; rewrite <- H; PPermut_simpl.
+
+(* letdia *)
+apply t_letdia_LF with
+  (L_t := L_t \u \{v})
+  (L_w := L_w \u used_w_vars ((w0, nil) :: emptyEquiv G)) (A:=A);
+[ apply ok_Bg_permut_first_tail with (C:=Gamma0) (x:=v) (A:=A0) |
+  eapply IHHT |
+  intros]; eauto;
+unfold open_t in *; unfold open_w in *;
+rewrite notin_union in H2; rewrite notin_singleton in H2; destruct H2;
+rewrite <- subst_order_irrelevant_bound;
+[ rewrite <- subst_t_comm | assumption ];
+[ eapply H | |] ; eauto;
+apply BackgroundSubsetImpl with (G:=emptyEquiv G); auto;
+[ exists ((w', (@nil (var*ty)))::nil);
+  PPermut_simpl ; rew_app; PPermut_simpl | ].
+assert ((w0, nil) :: (w', nil) :: emptyEquiv G ~=~
+  (w',nil) :: (w0, nil) :: emptyEquiv G) by PPermut_simpl;
+rewrite H5; apply ok_Bg_fresh_wo;
+[ apply emptyEquiv_ok_Bg in Ok_Bg;  simpl in * | ]; auto.
+
+eapply t_letdia_LF with
+  (L_t := L_t \u \{v})
+  (L_w := L_w \u  used_w_vars ((w', nil) :: emptyEquiv (G0 & (w0, Gamma0))));
+[ rewrite H2; rewrite H0 in Ok_Bg | eapply IHHT | intros]; eauto with ok_bg_rew;
+unfold open_t in *; unfold open_w in *.
+rewrite notin_union in H4; rewrite notin_singleton in H4; destruct H4;
+rewrite <- subst_order_irrelevant_bound;
+[ rewrite <- subst_t_comm | assumption ];
+[ eapply H with (G0:=(w'0, (v',A)::nil)::G0) (w'0:=w')
+  (Gamma':=Gamma') (A0:=A0) | | ]; auto;
+rew_app; rewrite H1 in H3; rew_app in *; simpl; try PPermut_simpl;
+apply BackgroundSubsetImpl with (G:= emptyEquiv (G0 & (w0, Gamma0))); auto;
+[exists ((w'0, (@nil (var*ty))):: nil); PPermut_simpl | ];
+assert ((w'0, nil) :: (w', nil)::emptyEquiv(G0 & (w0, Gamma0)) ~=~
+  (w', nil) :: (w'0, nil) :: emptyEquiv (G0 & (w0, Gamma0))) by auto;
+rewrite <- H7; apply ok_Bg_fresh_wo;
+[rewrite H0 in Ok_Bg; apply emptyEquiv_ok_Bg in Ok_Bg | ]; auto;
+  assert (emptyEquiv((w', (v, A0) :: Gamma') :: G0 & (w0, Gamma0)) ~=~
+    (w', nil) :: emptyEquiv (G0 & (w0, Gamma0))) by (simpl; auto);
+rewrite <- H8;
+assert ((w0, Gamma0) :: G0 & (w', (v, A0) :: Gamma') ~=~
+  ((w', (v, A0) :: Gamma') :: G0 & (w0, Gamma0))) by auto;
+rewrite <- H9; auto.
+
+(* letdia_get *)
+assert (w <> w0) by eauto with ok_bg_rew;
+eapply t_letdia_get_LF with (G:=G) (Gamma:=Gamma) (L_t := L_t \u \{v}) (A:=A)
+  (L_w:=L_w \u used_w_vars ((w0, nil) :: emptyEquiv (G & (w, Gamma)))); auto.
+apply ok_Bg_permut_no_last_spec with (v:=v) (A:=A0);
+apply ok_Bg_ppermut with (G:= (w, Gamma) :: G & (w0, Gamma0)); auto.
+eapply IHHT with (w':=w0) (Gamma':=Gamma1) (v:=v) (A0:=A0); auto.
+rew_app; rewrite <- H0 in H2; auto.
+intros; unfold open_t in *; unfold open_w in *;
+rewrite notin_union in H5; rewrite notin_singleton in H5; destruct H5;
+rewrite <- subst_order_irrelevant_bound;
+[rewrite <- subst_t_comm | ]; auto.
+eapply H with (v:=v) (A0:=A0); auto.
+rewrite <- H0 in H2;
+apply BackgroundSubsetImpl with (G:=emptyEquiv (G & (w, Gamma))); auto;
+[ exists ((w', (@ nil (var * ty)))::nil); PPermut_simpl | ];
+assert ((w0, nil) :: (w', nil) :: emptyEquiv (G & (w, Gamma)) ~=~
+  (w', nil) :: (w0, nil) ::emptyEquiv (G & (w, Gamma))) by PPermut_simpl;
+rewrite H8;
+apply ok_Bg_fresh_wo; [apply emptyEquiv_ok_Bg in Ok_Bg | auto];
+assert ((w, Gamma) :: G & (w0, Gamma0) ~=~ (w0, Gamma0):: G & (w, Gamma)) by
+  auto;
+rewrite H9 in Ok_Bg; simpl in Ok_Bg; auto.
+
+assert (w <> w0) by eauto with ok_bg_rew;
+destruct (eq_var_dec w w'); subst.
+(* = *)
+assert (G ~=~ G1 /\ Gamma *=* (v, A0) :: Gamma') by
+  (apply ok_Bg_impl_ppermut with (w:=w');
+    [ | rewrite H0; rewrite <- H1]; eauto);
+destruct H7; rewrite H3; rewrite <- H7;
+apply t_letdia_get_LF with (G:=G) (Gamma:=Gamma') (L_t:=L_t \u \{v}) (A:=A)
+  (L_w:=L_w \u used_w_vars ((w', nil) :: emptyEquiv (G1 & (w0, Gamma0)))).
+eauto with ok_bg_rew.
+eapply IHHT with (v:=v) (A0:=A0); auto;
+rewrite H2 in H4; rewrite H7; auto.
+intros; unfold open_t in *; unfold open_w in *;
+rewrite notin_union in H9; rewrite notin_singleton in H9; destruct H9;
+rewrite <- subst_order_irrelevant_bound;
+[ rewrite <- subst_t_comm | ]; auto.
+edestruct H with (v:=v) (w'0 := w'0) (Gamma1:=Gamma0) (A0:=A0)
+  (v':=v') (M:=M0) as (Ha, Hb);
+auto.
+eapply Hb with (G0 := (w'0, (v',A)::nil) ::G) (w'1 := w') (Gamma':=Gamma');
+[ | auto |  | ]; try PPermut_simpl.
+rewrite H2 in H4; rewrite H7.
+apply BackgroundSubsetImpl with (G:=emptyEquiv (G1 & (w0, Gamma0))); auto.
+exists (((w'0, (@nil (prod var ty))) :: nil)); rew_app; simpl; auto;
+PPermut_simpl.
+assert ((w', nil) :: (w'0, nil) :: emptyEquiv (G1 & (w0, Gamma0)) ~=~
+  (w'0, nil) :: (w',nil) :: emptyEquiv (G1 & (w0, Gamma0))) by auto;
+rewrite H12; apply ok_Bg_fresh_wo; auto;
+assert ((w', nil) :: emptyEquiv (G1 & (w0, Gamma0)) ~=~
+  emptyEquiv ((w', Gamma) :: G & (w0, Gamma0))) by
+  (simpl in *; rewrite H7; auto);
+rewrite H13; apply emptyEquiv_ok_Bg in Ok_Bg; auto.
+auto.
+(* <> *)
+assert (G & (w, Gamma) ~=~ G1 & (w', (v, A0) :: Gamma')) by
+  (transitivity G0; auto);
+symmetry in H7;
+assert (exists Gamma0, exists GH, exists GT,
+  Gamma0 *=* Gamma /\ G1 = GH & (w, Gamma0) ++ GT) by
+  (apply PPermut_split_neq with (w:=w') (Gamma:=(v,A0) :: Gamma') (G':=G);
+    auto);
+destruct H8 as (Gamma'', (GH, H8)); destruct H8 as (GT, H8);
+destruct H8.
+apply t_letdia_get_LF with (G:=GH++GT & (w', Gamma')) (Gamma:=Gamma) (A:=A)
+  (L_t:=L_t \u \{v}) (L_w:=L_w \u used_w_vars
+     ((w', nil) :: emptyEquiv (GH ++ GT ++ (w, Gamma) :: (w0, Gamma0) :: nil))).
+assert (G & (w, Gamma) & (w0, Gamma0) ~=~ (w, Gamma) :: G & (w0, Gamma0)) by
+  auto.
+rewrite <- H10 in Ok_Bg; rewrite <- H7 in Ok_Bg;
+subst; apply ok_Bg_ppermut with
+  (G:=((w, Gamma) :: (GH & (w', Gamma') ++ GT) & (w0, Gamma0))); [ | rew_app];
+auto.
+apply ok_Bg_ppermut with
+  (G:= (((w, Gamma) :: (GH & (w0, Gamma0) ++ GT)) & (w', Gamma')));
+[rew_app; PPermut_simpl | apply ok_Bg_permut_no_last_spec with (v:=v)(A:=A0)];
+apply ok_Bg_ppermut with
+  ((GH & (w, Gamma'') ++ GT) & (w', (v, A0) :: Gamma') & (w0, Gamma0));
+[ rew_app | ]; auto; try PPermut_simpl.
+eapply IHHT with (w1:=w) (Gamma1:=Gamma) (A0:=A0) (w':=w')
+  (G0:=GH++GT & (w0,Gamma0)) (Gamma':=Gamma'); auto;
+[ symmetry; subst; rew_app in * | rew_app | ]; auto.
+PPermut_simpl; apply PPermut_last_rev_simpl with (a:=(w, Gamma));
+rewrite <- H7; PPermut_simpl.
+rewrite H2 in H4; rewrite H9 in H4;
+assert ((GH & (w, Gamma'') ++ GT) & (w0, Gamma0) ~=~
+  (GH ++ GT & (w0, Gamma0)) ++ nil & (w, Gamma)) by (rew_app; PPermut_simpl);
+rewrite <- H10; auto.
+intros; unfold open_t in *; unfold open_w in *;
+rewrite notin_union in H10; rewrite notin_singleton in H10; destruct H10;
+rewrite <- subst_order_irrelevant_bound;
+[rewrite <- subst_t_comm | ]; auto;
+eapply H with (v':=v') (w':=w'0) (Gamma1:=Gamma0) (w1:=w0) (A0:=A0)
+              (v:=v) (G0:=(w'0, (v', A) :: nil) :: (GH ++ GT) & (w, Gamma))
+              (w'0:=w') (Gamma':=Gamma'); auto; try PPermut_simpl.
+apply PPermut_last_rev_simpl with (a:=(w, Gamma)); rewrite <- H7;
+subst; PPermut_simpl.
+rew_app; rewrite H2 in H4; rewrite H9 in H4; simpl;
+apply BackgroundSubsetImpl with
+  (G:=emptyEquiv (GH ++ GT ++ (w, Gamma) :: (w0, Gamma0) :: nil)); auto.
+assert (GH ++ GT ++ (w, Gamma) :: (w0, Gamma0) :: nil ~=~
+  (GH & (w, Gamma'') ++ GT) & (w0, Gamma0)) by (rew_app; PPermut_simpl);
+rewrite H13; auto.
+exists ((w'0, (@nil (var*ty))) :: nil); PPermut_simpl.
+assert ((w, Gamma) :: G & (w0, Gamma0) ~=~ G0 & (w0, Gamma0)) by
+  (rewrite <- H0; auto);
+rewrite H13 in Ok_Bg; rewrite H1 in Ok_Bg; subst;
+assert ((w', nil)
+      :: (w'0, nil)
+         :: emptyEquiv (GH ++ GT ++ (w, Gamma) :: (w0, Gamma0) :: nil) ~=~
+      (w'0, nil)
+      :: (w', nil)
+         :: emptyEquiv (GH ++ GT ++ (w, Gamma) :: (w0, Gamma0) :: nil)) by auto;
+rewrite H9; apply ok_Bg_fresh_wo;
+assert (((GH & (w, Gamma'') ++ GT) & (w', (v, A0) :: Gamma')) & (w0, Gamma0) ~=~
+  ((w', (v, A0) :: Gamma') :: GH ++ GT ++ (w, Gamma) :: nil) &  (w0, Gamma0)) by
+  (eapply PPermut_last_rev; auto; try PPermut_simpl);
+rew_app in *; [rewrite H14 in Ok_Bg | auto];
+apply emptyEquiv_ok_Bg in Ok_Bg; simpl in *; auto.
+symmetry; transitivity (G1 & (w', Gamma')); subst; rew_app in *; PPermut_simpl.
+Existential 1 := v'.
+Existential 1 := Gamma.
+Existential 1 := v'.
+Existential 1 := Gamma.
+Qed.
+
+Lemma subst_t_preserv_types_inner:
+forall G w Gamma A B M N v
+  (H_lc_t: lc_t_LF M)
+  (H_lc_w: lc_w_LF M)
+  (HT: G |= (w, (v, A) :: Gamma) |- N ::: B)
+  (HM: emptyEquiv G |= (w, nil) |- M ::: A),
+  G |= (w, Gamma) |- [M//fte v] N ::: B.
+intros; eapply subst_t_preserv_types with (Gamma := (v, A) :: Gamma); eauto.
+Qed.
+
+Lemma subst_t_preserv_types_outer:
+forall G0 G G' G'' w w' Gamma Gamma' A B M N v
+  (H_lc_t: lc_t_LF M)
+  (H_lc_w: lc_w_LF M)
+  (G0G: G ~=~ (G0 & (w', (v, A) :: Gamma')))
+  (G0G': G' ~=~ (G0 & (w, Gamma)))
+  (G0G'': G'' ~=~ (G0 & (w', Gamma')))
+  (HM: emptyEquiv G' |= (w', nil) |- M ::: A)
+  (HT: G |= (w, Gamma) |- N ::: B),
+  G'' |= (w, Gamma) |- [M // fte v] N ::: B.
+intros; eapply subst_t_preserv_types; eauto.
+Qed.
+
+(*
+Proof: induction on typing
+  * for terms with world change: we again have to check whether the
+  world which we will switch into is one of those in renaming
+*)
+Lemma rename_w_preserv_types:
+forall G w Gamma A M G' w' Gamma'
+  (HT: G |= (w, Gamma) |- M ::: A),
+  (* "new" substitution *)
+  ( G ~=~ (G' & (w', Gamma')) ->
+    G' |= (w, Gamma ++ Gamma') |- {{ fwo w // fwo w' }} M ::: A) /\
+  (* "old" substitution *)
+  ( G ~=~ (G' & (w', Gamma')) ->
+    G' |= (w', Gamma' ++ Gamma) |- {{ fwo w' // fwo w }} M ::: A) /\
+  (* "outer" substitution *)
+  (forall G0 w'' Gamma'',
+    G ~=~ (G0 & (w', Gamma') & (w'', Gamma'')) ->
+    G' ~=~ (G0 & (w', Gamma' ++ Gamma'')) ->
+    G' |= (w, Gamma) |- {{ fwo w' // fwo w''}} M ::: A).
+intros;
+remember (w, Gamma) as Ctx;
+generalize dependent Gamma;
+generalize dependent w;
+generalize dependent w';
+generalize dependent Gamma';
+generalize dependent G';
+induction HT; repeat split; intros;
+inversion HeqCtx; subst;
+simpl in *.
+
+(* hyp *)
+constructor;
+[ rewrite H in Ok_Bg  |
+  rewrite Mem_app_or_eq; left ]; auto;
+eapply ok_Bg_split2; eauto.
+constructor;
+[ rewrite H in Ok_Bg |
+  rewrite Mem_app_or_eq; right ]; auto;
+eapply ok_Bg_split2; eauto.
+constructor;
+[ rewrite H in Ok_Bg; rewrite H0 | ]; auto;
+eapply ok_Bg_split3; eauto.
+(* lam *)
+apply t_lam_LF with (L := L);
+[ rewrite H0 in Ok_Bg; eapply ok_Bg_split2; eauto |
+  intros; unfold open_t in *];
+rewrite subst_order_irrelevant_free; simpl; auto;
+apply H with (v':=v') (G':=G') (Gamma := (v',A)::Gamma0); auto.
+apply t_lam_LF with (L := L);
+[ rewrite H0 in Ok_Bg; eapply ok_Bg_split2; eauto |
+  intros]; unfold open_t in *;
+rewrite subst_order_irrelevant_free;
+edestruct H; eauto; destruct H3;
+[ apply ContextPermutImpl with (Gamma := (Gamma' ++ (v', A) :: Gamma0));
+  [permut_simpl | ] | simpl; apply notin_empty ]; eauto.
+apply t_lam_LF with (L := L);
+[ rewrite H0 in Ok_Bg |
+  intros];
+rewrite H1; try eapply ok_Bg_split3; eauto;
+unfold open_t in *;
+rewrite subst_order_irrelevant_free;
+edestruct H; eauto; destruct H4;
+eauto;
+simpl; apply notin_empty.
+
+(* appl *)
+apply t_appl_LF with (A:=A);
+[ rewrite H in Ok_Bg |
+  apply IHHT1 with (Gamma:=Gamma0) |
+  apply IHHT2 with (Gamma:=Gamma0) ];
+eauto; eapply ok_Bg_split2; eauto.
+apply t_appl_LF with (A:=A);
+[ rewrite H in Ok_Bg |
+  apply IHHT1 with (Gamma:=Gamma0) |
+  apply IHHT2 with (Gamma:=Gamma0) ];
+eauto; eapply ok_Bg_split2; eauto.
+apply t_appl_LF with (A:=A);
+[ rewrite H in Ok_Bg; rewrite H0 |
+  eapply IHHT1 |
+  eapply IHHT2 ]; eauto;
+eapply ok_Bg_split3; eauto.
+
+(* box *)
+apply t_box_LF with (L:=\{w'} \u L);
+[ rewrite H0 in Ok_Bg; eapply ok_Bg_split4; eauto |
+  intros];
+unfold open_w in *; rewrite notin_union in H1; destruct H1;
+rewrite notin_singleton in *; rewrite <- subst_w_comm; auto;
+eapply H; eauto; PPermut_simpl.
+apply t_box_LF with (L:=\{w0} \u L);
+[ rewrite H0 in Ok_Bg; apply ok_Bg_split4 with (w:=w0);
+  apply ok_Bg_ppermut with (G:=G' & (w', Gamma') & (w0, Gamma0)); auto |
+  intros]; try PPermut_simpl;
+unfold open_w in *; rewrite notin_union in H1; destruct H1;
+rewrite notin_singleton in *; rewrite <- subst_w_comm; auto;
+eapply H; eauto.
+apply t_box_LF with (L:=\{w''} \u L);
+[ rewrite H0 in Ok_Bg; rewrite H1; eapply ok_Bg_split6; eauto |
+  intros];
+unfold open_w in *;
+rewrite notin_union in H2; destruct H2;
+rewrite notin_singleton in *;
+rewrite <- subst_w_comm; auto;
+eapply H with (G0:=G0 & (w0, Gamma0)) (Gamma':=Gamma') (Gamma'':=Gamma''); auto;
+try PPermut_simpl; rewrite H0; PPermut_simpl.
+
+(* unbox *)
+case_if.
+inversion H0; subst; rewrite H in Ok_Bg;
+apply ok_Bg_first_last_neq in Ok_Bg; elim Ok_Bg; auto.
+constructor; [rewrite H in Ok_Bg | apply IHHT with (Gamma:=Gamma0)]; eauto;
+eapply ok_Bg_split2; eauto.
+
+case_if; constructor;
+[ rewrite H in Ok_Bg |
+  apply IHHT with (Gamma:=Gamma0) ]; eauto;
+eapply ok_Bg_split2; eauto.
+
+case_if.
+inversion H1; subst; rewrite H in Ok_Bg;
+apply ok_Bg_first_last_neq in Ok_Bg; elim Ok_Bg; auto.
+constructor; [rewrite H0; rewrite H in Ok_Bg | eapply IHHT]; eauto;
+eapply ok_Bg_split3; eauto.
+
+(* unbox_fetch *)
+case_if.
+inversion H1; subst;
+assert (G ~=~ G'0 /\ Gamma *=* Gamma'0) as HP by
+  (apply ok_Bg_impl_ppermut with (w:=w'0);
+   [eauto | rewrite H; rewrite H0; auto]);
+destruct HP; constructor.
+rewrite <- H2; apply ok_Bg_split2 with (w:=w'0);
+eapply ok_Bg_permut; eauto.
+apply ContextPermutImpl with (Gamma:=Gamma0 ++ Gamma);
+[ permut_simpl |
+  apply IHHT] ; auto.
+assert (G'0 & (w'0, Gamma'0) ~=~ G & (w, Gamma)) by
+  (symmetry; transitivity G'; auto);
+assert (exists Gamma'', exists GH, exists GT,
+  Gamma'' *=* Gamma /\ G'0 = GH & (w, Gamma'') ++ GT) as Split by
+  (eapply PPermut_split_neq; eauto; right; intro; subst; elim H1; reflexivity);
+destruct Split as (Gamma'', (GH, Split)); destruct Split as (GT, H3);
+destruct H3 as (H3a, H3b).
+apply t_unbox_fetch_LF with (G:=GH++GT) (Gamma:=Gamma).
+assert ((w, Gamma) :: G & (w0, Gamma0) ~=~ G & (w, Gamma) & (w0, Gamma0)) by
+  auto.
+rewrite H3 in Ok_Bg; rewrite <- H2 in Ok_Bg; rew_app in *;
+assert (GH & (w, Gamma) ++ GT ~=~ (w, Gamma) :: GH ++ GT) by (PPermut_simpl);
+apply ok_Bg_ppermut with
+  (G:= (GH & (w, Gamma) ++ GT) & (w0, Gamma0 ++ Gamma'0));
+[ rewrite H4 |
+  apply ok_Bg_split4 with (w:=w'0)]; rew_app; auto.
+subst; rew_app in *;
+apply ok_Bg_ppermut with
+  (G:=(GH ++ (w, Gamma'') :: GT ++ (w'0, Gamma'0) :: (w0, Gamma0) :: nil));
+try PPermut_simpl; auto.
+eapply IHHT with (w1:=w) (Gamma1:=Gamma); auto; subst; symmetry; PPermut_simpl;
+apply PPermut_last_rev_simpl with (a:=(w, Gamma)); rew_app in *; auto;
+rew_app; auto; rewrite <- H2; PPermut_simpl.
+apply PPermut_last_rev_simpl with (a:=(w, Gamma)); rew_app in *; auto; subst;
+PPermut_simpl.
+
+case_if;
+[ inversion H1; subst; apply ok_Bg_first_last_neq in Ok_Bg; elim Ok_Bg; auto |
+  destruct (eq_var_dec w w'0)].
+subst; assert (G ~=~ G'0 /\ Gamma *=* Gamma'0) by
+  (apply ok_Bg_impl_ppermut with (w:=w'0); [ | rewrite <- H0]; eauto);
+destruct H2; constructor.
+rewrite <- H2; apply ok_Bg_permut with (Ctx := (Gamma ++ Gamma0)); eauto;
+eapply ok_Bg_split2; eauto.
+apply ContextPermutImpl with (Gamma:=Gamma ++ Gamma0);
+[ permut_simpl |
+  eapply IHHT with (w:=w'0) (Gamma1:=Gamma) (Gamma':=Gamma0)] ; auto.
+assert (G'0 & (w'0, Gamma'0) ~=~ G & (w, Gamma)) by
+  (symmetry; transitivity G'; auto);
+assert (exists Gamma'', exists GH, exists GT,
+  Gamma'' *=* Gamma /\ G'0 = GH & (w, Gamma'') ++ GT) as Split by
+  (eapply PPermut_split_neq; eauto; right; intro; subst; elim H1; reflexivity);
+destruct Split as (Gamma'', (GH, Split));
+destruct Split as (GT, (Ha, Hb)); subst;
+apply t_unbox_fetch_LF with (G:=GH++GT) (Gamma:=Gamma).
+assert (GH & (w, Gamma) ++ GT ~=~ (w, Gamma) :: GH ++ GT)
+  by PPermut_simpl;
+apply ok_Bg_ppermut with
+  (G:= (GH & (w, Gamma'') ++ GT) & (w'0, Gamma0 ++ Gamma'0));
+[ PPermut_simpl | apply ok_Bg_split4 with (w:=w0)]; rew_app; auto.
+assert ((w, Gamma) :: G & (w0, Gamma0) ~=~
+  (G & (w, Gamma)) & (w0, Gamma0)) by auto;
+rewrite H4 in Ok_Bg; rewrite <- H2 in Ok_Bg; rew_app in *;
+remember (GH ++ (w, Gamma'') :: GT) as GHT;
+assert (GH ++ (w, Gamma'') :: GT ++ (w0, Gamma'0) :: (w'0, Gamma0) :: nil ~=~
+  GHT & (w0, Gamma'0) & (w'0, Gamma0)) by (subst; rew_app; auto).
+rewrite H5; apply ok_Bg_swap_worlds; subst; rew_app in *; auto.
+eapply IHHT; auto; PPermut_simpl.
+apply PPermut_last_rev_simpl with (a:=(w, Gamma)); rew_app in *;
+rewrite H; rewrite H0; PPermut_simpl.
+transitivity (GH & (w, Gamma) ++ GT); PPermut_simpl.
+
+case_if.
+inversion H2; subst;
+assert (G ~=~ G0 & (w'0, Gamma'0) /\ Gamma *=* Gamma'') by
+  (apply ok_Bg_impl_ppermut with (w:=w''); [ | rewrite H; rewrite H0]; eauto);
+destruct H3; apply t_unbox_fetch_LF with (G:=G0) (Gamma := Gamma'0 ++ Gamma);
+[ rewrite H3 in Ok_Bg | apply IHHT | rewrite H1]; eauto.
+apply ok_Bg_split9 with (w':=w'');
+apply ok_Bg_ppermut with (G:= (w'', Gamma)::G0 & (w'0, Gamma'0) & (w0, Gamma0));
+eauto; PPermut_simpl.
+rewrite H3; PPermut_simpl.
+destruct (eq_var_dec w w'0).
+subst; assert (G ~=~ G0 & (w'', Gamma'') /\ Gamma *=* Gamma'0) by
+  (apply ok_Bg_impl_ppermut with (w:=w'0); [ | rewrite H; rewrite H0];
+   eauto; PPermut_simpl);
+destruct H3;
+apply t_unbox_fetch_LF with (G:=G0) (Gamma := Gamma ++ Gamma'');
+[ rewrite H3 in Ok_Bg |
+  eapply IHHT with (G':=G0 & (w0, Gamma0)) (Gamma' := Gamma'') |
+  rewrite H1]; eauto.
+eapply ok_Bg_split9; eauto.
+rewrite H3; PPermut_simpl.
+assert (G0 & (w'0, Gamma'0) & (w'', Gamma'')  ~=~ G & (w, Gamma)) by
+  (symmetry; transitivity G'; auto);
+assert (exists Gamma'', exists GH, exists GT,
+  Gamma'' *=* Gamma /\ G0 & (w'0, Gamma'0) = GH & (w, Gamma'') ++ GT)
+  as Split.
+apply PPermut_split_neq with (w:=w'')
+  (Gamma:=Gamma'') (G':= G); auto; right; intro; subst; elim H2; auto.
+assert (exists Gamma'', exists GH, exists GT,
+  Gamma'' *=* Gamma /\ G0 = GH & (w, Gamma'') ++ GT) as Split' by
+  (destruct Split as (Gamma''', (GH, Split));
+    destruct Split as (GT, (Ha, Hb));
+   apply PPermut_split_neq with (w:=w'0) (Gamma:=Gamma'0) (G':=GH ++ GT);
+   [ rew_app; transitivity (GH & (w, Gamma) ++ GT) |
+     right; intro; subst; elim n]; auto; rewrite Hb; auto);
+destruct Split' as (Gamma''',(GH, Split'));
+destruct Split' as (GT, (Ha, Hb));
+apply t_unbox_fetch_LF with (G:=GH++GT & (w'0, Gamma'0++Gamma''))
+  (Gamma:=Gamma).
+apply ok_Bg_ppermut with (G':=(G' & (w0, Gamma0))) in Ok_Bg;
+[ | rewrite <- H; auto]; rewrite H0 in Ok_Bg; subst G0.
+apply ok_Bg_ppermut with
+  (G:= (GH & (w, Gamma''') ++ GT) & (w'0, Gamma'0 ++ Gamma'') & (w0, Gamma0));
+[ rew_app | ]; auto; try PPermut_simpl; eapply ok_Bg_split6; eauto.
+eapply IHHT with (w1:=w) (Gamma1:=Gamma) (G0:=GH++GT & (w0,Gamma0))
+  (Gamma':=Gamma'0) (Gamma'':=Gamma''); auto.
+PPermut_simpl. apply PPermut_last_rev_simpl with (a:=(w, Gamma));
+rewrite <- H3; subst; PPermut_simpl.
+PPermut_simpl.
+rewrite H1; subst; PPermut_simpl.
+
+(* here *)
+case_if.
+inversion H0; subst; rewrite H in Ok_Bg;
+apply ok_Bg_first_last_neq in Ok_Bg; elim Ok_Bg; auto.
+constructor;
+[ rewrite H in Ok_Bg | apply IHHT with (Gamma:=Gamma0)]; eauto;
+eapply ok_Bg_split2; eauto.
+
+case_if; constructor;
+[ rewrite H in Ok_Bg |
+  apply IHHT with (Gamma:=Gamma0) ]; eauto;
+eapply ok_Bg_split2; eauto.
+
+case_if.
+inversion H1; subst; rewrite H in Ok_Bg;
+apply ok_Bg_first_last_neq in Ok_Bg; elim Ok_Bg; auto.
+constructor; [rewrite H0; rewrite H in Ok_Bg | eapply IHHT]; eauto;
+eapply ok_Bg_split3; eauto.
+
+(* get_here *)
+case_if.
+inversion H1; subst;
+assert (G ~=~ G'0 /\ Gamma *=* Gamma'0) as HP by
+  (apply ok_Bg_impl_ppermut with (w:=w'0);
+   [eauto | rewrite H; rewrite H0; auto]);
+destruct HP; constructor.
+rewrite <- H2; apply ok_Bg_split2 with (w:=w'0);
+eapply ok_Bg_permut; eauto.
+apply ContextPermutImpl with (Gamma:=Gamma0 ++ Gamma);
+[ permut_simpl |
+  apply IHHT] ; auto.
+assert (G'0 & (w'0, Gamma'0) ~=~ G & (w, Gamma)) by
+  (symmetry; transitivity G'; auto);
+assert (exists Gamma'', exists GH, exists GT,
+  Gamma'' *=* Gamma /\ G'0 = GH & (w, Gamma'') ++ GT) as Split by
+  (eapply PPermut_split_neq; eauto; right; intro; subst; elim H1; reflexivity);
+destruct Split as (Gamma'', (GH, Split)); destruct Split as (GT, H3);
+destruct H3 as (H3a, H3b).
+apply t_get_here_LF with (G:=GH++GT) (Gamma:=Gamma).
+assert ((w, Gamma) :: G & (w0, Gamma0) ~=~ G & (w, Gamma) & (w0, Gamma0)) by
+  auto.
+rewrite H3 in Ok_Bg; rewrite <- H2 in Ok_Bg; rew_app in *;
+assert (GH & (w, Gamma) ++ GT ~=~ (w, Gamma) :: GH ++ GT) by (PPermut_simpl);
+apply ok_Bg_ppermut with
+  (G:= (GH & (w, Gamma) ++ GT) & (w0, Gamma0 ++ Gamma'0));
+[ rewrite H4 |
+  apply ok_Bg_split4 with (w:=w'0)]; rew_app; auto.
+subst; rew_app in *;
+apply ok_Bg_ppermut with
+  (G:=(GH ++ (w, Gamma'') :: GT ++ (w'0, Gamma'0) :: (w0, Gamma0) :: nil));
+try PPermut_simpl; auto.
+eapply IHHT with (w1:=w) (Gamma1:=Gamma); auto; subst; symmetry; PPermut_simpl;
+apply PPermut_last_rev_simpl with (a:=(w, Gamma)); rew_app in *; auto;
+rew_app; auto; rewrite <- H2; PPermut_simpl.
+apply PPermut_last_rev_simpl with (a:=(w, Gamma)); rew_app in *; auto; subst;
+PPermut_simpl.
+
+case_if;
+[ inversion H1; subst; apply ok_Bg_first_last_neq in Ok_Bg; elim Ok_Bg; auto |
+  destruct (eq_var_dec w w'0)].
+subst; assert (G ~=~ G'0 /\ Gamma *=* Gamma'0) by
+  (apply ok_Bg_impl_ppermut with (w:=w'0); [ | rewrite <- H0]; eauto);
+destruct H2; constructor.
+rewrite <- H2; apply ok_Bg_permut with (Ctx := (Gamma ++ Gamma0)); eauto;
+eapply ok_Bg_split2; eauto.
+apply ContextPermutImpl with (Gamma:=Gamma ++ Gamma0);
+[ permut_simpl |
+  eapply IHHT with (w:=w'0) (Gamma1:=Gamma) (Gamma':=Gamma0)] ; auto.
+assert (G'0 & (w'0, Gamma'0) ~=~ G & (w, Gamma)) by
+  (symmetry; transitivity G'; auto);
+assert (exists Gamma'', exists GH, exists GT,
+  Gamma'' *=* Gamma /\ G'0 = GH & (w, Gamma'') ++ GT) as Split by
+  (eapply PPermut_split_neq; eauto; right; intro; subst; elim H1; reflexivity);
+destruct Split as (Gamma'', (GH, Split));
+destruct Split as (GT, (Ha, Hb)); subst;
+apply t_get_here_LF with (G:=GH++GT) (Gamma:=Gamma).
+assert (GH & (w, Gamma) ++ GT ~=~ (w, Gamma) :: GH ++ GT)
+  by PPermut_simpl;
+apply ok_Bg_ppermut with
+  (G:= (GH & (w, Gamma'') ++ GT) & (w'0, Gamma0 ++ Gamma'0));
+[ PPermut_simpl | apply ok_Bg_split4 with (w:=w0)]; rew_app; auto.
+assert ((w, Gamma) :: G & (w0, Gamma0) ~=~
+  (G & (w, Gamma)) & (w0, Gamma0)) by auto;
+rewrite H4 in Ok_Bg; rewrite <- H2 in Ok_Bg; rew_app in *;
+remember (GH ++ (w, Gamma'') :: GT) as GHT;
+assert (GH ++ (w, Gamma'') :: GT ++ (w0, Gamma'0) :: (w'0, Gamma0) :: nil ~=~
+  GHT & (w0, Gamma'0) & (w'0, Gamma0)) by (subst; rew_app; auto).
+rewrite H5; apply ok_Bg_swap_worlds; subst; rew_app in *; auto.
+eapply IHHT; auto; PPermut_simpl.
+apply PPermut_last_rev_simpl with (a:=(w, Gamma)); rew_app in *;
+rewrite H; rewrite H0; PPermut_simpl.
+transitivity (GH & (w, Gamma) ++ GT); PPermut_simpl.
+
+case_if.
+inversion H2; subst;
+assert (G ~=~ G0 & (w'0, Gamma'0) /\ Gamma *=* Gamma'') by
+  (apply ok_Bg_impl_ppermut with (w:=w''); [ | rewrite H; rewrite H0]; eauto);
+destruct H3; apply t_get_here_LF with (G:=G0) (Gamma := Gamma'0 ++ Gamma);
+[ rewrite H3 in Ok_Bg | apply IHHT | rewrite H1]; eauto.
+apply ok_Bg_split9 with (w':=w'');
+apply ok_Bg_ppermut with (G:= (w'', Gamma)::G0 & (w'0, Gamma'0) & (w0, Gamma0));
+eauto; PPermut_simpl.
+rewrite H3; PPermut_simpl.
+destruct (eq_var_dec w w'0).
+subst; assert (G ~=~ G0 & (w'', Gamma'') /\ Gamma *=* Gamma'0) by
+  (apply ok_Bg_impl_ppermut with (w:=w'0); [ | rewrite H; rewrite H0];
+   eauto; PPermut_simpl);
+destruct H3;
+apply t_get_here_LF with (G:=G0) (Gamma := Gamma ++ Gamma'');
+[ rewrite H3 in Ok_Bg |
+  eapply IHHT with (G':=G0 & (w0, Gamma0)) (Gamma' := Gamma'') |
+  rewrite H1]; eauto.
+eapply ok_Bg_split9; eauto.
+rewrite H3; PPermut_simpl.
+assert (G0 & (w'0, Gamma'0) & (w'', Gamma'')  ~=~ G & (w, Gamma)) by
+  (symmetry; transitivity G'; auto);
+assert (exists Gamma'', exists GH, exists GT,
+  Gamma'' *=* Gamma /\ G0 & (w'0, Gamma'0) = GH & (w, Gamma'') ++ GT)
+  as Split.
+apply PPermut_split_neq with (w:=w'')
+  (Gamma:=Gamma'') (G':= G); auto; right; intro; subst; elim H2; auto.
+assert (exists Gamma'', exists GH, exists GT,
+  Gamma'' *=* Gamma /\ G0 = GH & (w, Gamma'') ++ GT) as Split' by
+  (destruct Split as (Gamma''', (GH, Split));
+    destruct Split as (GT, (Ha, Hb));
+   apply PPermut_split_neq with (w:=w'0) (Gamma:=Gamma'0) (G':=GH ++ GT);
+   [ rew_app; transitivity (GH & (w, Gamma) ++ GT) |
+     right; intro; subst; elim n]; auto; rewrite Hb; auto);
+destruct Split' as (Gamma''',(GH, Split'));
+destruct Split' as (GT, (Ha, Hb));
+apply t_get_here_LF with (G:=GH++GT & (w'0, Gamma'0++Gamma''))
+  (Gamma:=Gamma).
+apply ok_Bg_ppermut with (G':=(G' & (w0, Gamma0))) in Ok_Bg;
+[ | rewrite <- H; auto]; rewrite H0 in Ok_Bg; subst G0.
+apply ok_Bg_ppermut with
+  (G:= (GH & (w, Gamma''') ++ GT) & (w'0, Gamma'0 ++ Gamma'') & (w0, Gamma0));
+[ rew_app | ]; auto; try PPermut_simpl; eapply ok_Bg_split6; eauto.
+eapply IHHT with (w1:=w) (Gamma1:=Gamma) (G0:=GH++GT & (w0,Gamma0))
+  (Gamma':=Gamma'0) (Gamma'':=Gamma''); auto.
+PPermut_simpl. apply PPermut_last_rev_simpl with (a:=(w, Gamma));
+rewrite <- H3; subst; PPermut_simpl.
+PPermut_simpl.
+rewrite H1; subst; PPermut_simpl.
+
+(* letdia *)
+case_if.
+inversion H1; subst; rewrite H0 in Ok_Bg;
+apply ok_Bg_first_last_neq in Ok_Bg; elim Ok_Bg; auto.
+apply t_letdia_LF with (L_w:=L_w \u \{w'}) (L_t:=L_t) (A:=A);
+[ rewrite H0 in Ok_Bg |
+  eapply IHHT with (w:=w0) (Gamma:=Gamma0) | ]; eauto.
+eapply ok_Bg_split2; eauto.
+intros; rewrite notin_union in H3; destruct H3;
+rewrite notin_singleton in H4;
+unfold open_t in *; unfold open_w in *;
+rewrite <- subst_w_comm; auto;
+rewrite subst_order_irrelevant_free;
+[ eapply H with (w:=w0) (Gamma:=Gamma0) (w':=w'0) | simpl]; eauto;
+rewrite H0; PPermut_simpl.
+
+case_if.
+apply t_letdia_LF with (L_w:=L_w \u \{w0}) (L_t:=L_t) (A:=A);
+[ rewrite H0 in Ok_Bg | eapply IHHT with (w:=w0) (Gamma:=Gamma0) | ]; eauto.
+eapply ok_Bg_split2; eauto.
+intros; rewrite notin_union in H2; destruct H2;
+rewrite notin_singleton in H3;
+unfold open_t in *; unfold open_w in *;
+rewrite <- subst_w_comm; auto;
+rewrite subst_order_irrelevant_free;
+[ eapply H with (w:=w0) (Gamma:=Gamma0) (w':=w'0) | simpl]; eauto;
+rewrite H0; PPermut_simpl.
+
+case_if.
+inversion H2; subst; rewrite H0 in Ok_Bg;
+apply ok_Bg_first_last_neq in Ok_Bg; elim Ok_Bg; auto.
+apply t_letdia_LF with (L_w:=L_w \u \{w''}) (L_t:=L_t) (A:=A);
+[ rewrite H0 in Ok_Bg; rewrite H1 |
+  eapply IHHT with (w:=w0) (Gamma:=Gamma0) | ]; eauto.
+eapply ok_Bg_split3; eauto.
+intros; rewrite notin_union in H4; destruct H4;
+rewrite notin_singleton in H5;
+unfold open_t in *; unfold open_w in *;
+rewrite <- subst_w_comm; auto;
+rewrite subst_order_irrelevant_free; simpl; auto;
+eapply H with (w:=w0) (Gamma:=Gamma0) (G0:=G0 & ((w'0, (v', A)::nil)))
+  (Gamma':=Gamma') (Gamma'':=Gamma''); auto;
+[ rewrite H0 |rewrite H1 ]; rew_app; auto;
+PPermut_simpl.
+
+(* letdia_get *)
+case_if.
+inversion H3; subst;
+assert (G ~=~ G' /\ Gamma *=* Gamma') by
+  (apply ok_Bg_impl_ppermut with (w:=w'); [ | transitivity G0]; eauto);
+destruct H4;
+eapply t_letdia_LF with (L_w := L_w \u \{w'}).
+rewrite <- H4; apply ok_Bg_permut with (Ctx:=(Gamma0 ++ Gamma)); auto;
+eapply ok_Bg_split1; eauto.
+apply ContextPermutImpl with (Gamma := Gamma0++Gamma); [permut_simpl|]; auto;
+eapply IHHT; auto.
+intros; rewrite notin_union in H7; destruct H7;
+rewrite notin_singleton in H8;
+unfold open_t in *; unfold open_w in *;
+rewrite <- subst_w_comm; auto;
+rewrite subst_order_irrelevant_free; simpl; auto;
+eapply H with (v':=v') (w'0:=w'0) (w:=w0); auto;
+[ | rew_app]; eauto.
+destruct (eq_var_dec w w0).
+subst; apply ok_Bg_first_last_neq in Ok_Bg; elim Ok_Bg; auto.
+assert (G' & (w', Gamma') ~=~ G & (w, Gamma)) by
+  (symmetry; transitivity G0; auto);
+assert (exists Gamma'', exists GH, exists GT,
+  Gamma'' *=* Gamma /\ G' = GH & (w, Gamma'') ++ GT) by
+  (eapply PPermut_split_neq; eauto; right; intro; subst; eauto);
+destruct H5 as (Gamma'', (GH, (GT, (Ha, Hb))));
+assert (G & (w, Gamma) ~=~
+       (GH ++ GT ++ (w', Gamma') :: nil) &  (w, Gamma));
+[subst; symmetry | rew_app]; auto.
+rewrite <- H4; PPermut_simpl.
+apply t_letdia_get_LF with (L_w:=L_w \u \{w'}) (L_t:=L_t) (A:=A)
+  (G:=GH++GT) (Gamma:=Gamma);
+assert ((w, Gamma) :: G & (w0, Gamma0) ~=~
+  (GH ++ GT & (w', Gamma')) & (w, Gamma) & (w0, Gamma0)) by
+  (PPermut_simpl; apply PPermut_last_rev_simpl with (a:=(w,Gamma)); auto).
+rewrite H6 in Ok_Bg.
+apply ok_Bg_ppermut with (G:=(GH ++ GT & (w, Gamma)) & (w0, Gamma0 ++ Gamma')).
+PPermut_simpl.
+rew_app in *; eauto. eapply ok_Bg_split8; eauto.
+eapply IHHT with (w1:=w) (G0:=GH++GT) (w':=w0)
+  (Gamma':=Gamma0) (Gamma'':=Gamma');
+auto.
+PPermut_simpl; apply PPermut_last_rev_simpl with (a:=(w, Gamma));
+rewrite H5; PPermut_simpl.
+intros; rewrite notin_union in H8; destruct H8;
+rewrite notin_singleton in H9;
+unfold open_t in *; unfold open_w in *;
+rewrite <- subst_w_comm; auto;
+rewrite subst_order_irrelevant_free; simpl; auto;
+eapply H with (w1:=w0) (Gamma1:=Gamma0); auto.
+rewrite H5; PPermut_simpl.
+subst; PPermut_simpl.
+
+case_if.
+inversion H3; subst;
+apply ok_Bg_first_last_neq in Ok_Bg; elim Ok_Bg; auto.
+destruct (eq_var_dec w w').
+subst; assert (G ~=~ G' /\ Gamma *=* Gamma').
+  apply ok_Bg_impl_ppermut with (w:=w'); auto. eauto with ok_bg_rew.
+  transitivity G0; auto.
+destruct H4;
+apply t_letdia_LF with (L_w:=L_w \u \{w0}) (L_t:=L_t) (A:=A).
+rewrite <- H4; apply ok_Bg_permut with (Ctx := Gamma ++ Gamma0); auto;
+eapply ok_Bg_split2; eauto.
+apply ContextPermutImpl with (Gamma:=Gamma++Gamma0); auto;
+eapply IHHT with (Gamma1:=Gamma); eauto.
+intros; rewrite <- H4;
+apply ContextPermutImpl with (Gamma:=Gamma++Gamma0); auto;
+unfold open_t in *; unfold open_w in *;
+rewrite <- subst_w_comm; auto;
+rewrite subst_order_irrelevant_free; simpl; auto.
+eapply H with (w'0 := w'0); eauto.
+assert (G' & (w', Gamma') ~=~ G & (w, Gamma)) by
+  (symmetry; transitivity G0; auto);
+assert (exists Gamma'', exists GH, exists GT,
+  Gamma'' *=* Gamma /\ G' = GH & (w, Gamma'') ++ GT) by
+  (eapply PPermut_split_neq; eauto).
+destruct H5 as (Gamma'', (GH, (GT, (Ha, Hb)))).
+apply t_letdia_get_LF with (L_w:=L_w \u \{w0})
+  (L_t:=L_t) (A:=A) (G:=GH++GT) (Gamma:=Gamma).
+subst; assert ((w, Gamma) :: G & (w0, Gamma0) ~=~
+  (GH & (w, Gamma'') ++ GT) & (w', Gamma') & (w0, Gamma0)) by
+(rewrite H4; auto).
+rewrite H5 in Ok_Bg.
+apply ok_Bg_ppermut with (G:= GH & (w, Gamma'') ++ GT & (w', Gamma' ++ Gamma0));
+rew_app in *; [ PPermut_simpl | ];
+apply ok_Bg_ppermut with
+  (G:=(GH ++ (w, Gamma'') :: GT) & (w', Gamma' ++ Gamma0));
+[ | apply ok_Bg_split4 with (w:=w0)]; rew_app; auto;
+apply ok_Bg_ppermut with (G:=GH ++ (w, Gamma'') :: GT ++ (w', Gamma') ::
+  (w0, Gamma0) :: nil); eauto.
+eapply IHHT; auto.
+PPermut_simpl; apply PPermut_last_rev_simpl with (a:=(w, Gamma));
+rewrite <- H4; subst; PPermut_simpl.
+intros. rewrite notin_union in H6; destruct H6;
+rewrite notin_singleton in H7; unfold open_t in *; unfold open_w in *;
+rewrite <- subst_w_comm; auto;
+rewrite subst_order_irrelevant_free; simpl; auto;
+eapply H with (w1:=w0) (Gamma1:=Gamma0); auto; PPermut_simpl.
+apply PPermut_last_rev_simpl with (a:=(w,Gamma));
+rewrite <- H4; subst; PPermut_simpl.
+subst; PPermut_simpl.
+
+case_if.
+inversion H4; subst;
+assert (G ~=~ G1 & (w', Gamma') /\ Gamma *=* Gamma'') by
+ (apply ok_Bg_impl_ppermut with (w:=w'');
+  [ | transitivity G0]; eauto);
+destruct H5;
+eapply t_letdia_get_LF with (G:=G1) (Gamma:=Gamma'++Gamma) (L_w:=L_w \u \{w''}).
+rewrite H5 in Ok_Bg; eauto.
+clear H HT2 IHHT.
+eapply ok_Bg_split2; eauto; apply ok_Bg_ppermut with
+  (G:=(w'', Gamma) :: G1 & (w', Gamma') & (w0, Gamma0));
+eauto; PPermut_simpl.
+eapply IHHT with (Gamma':=Gamma'); auto;
+try PPermut_simpl.
+intros; unfold open_t in *; unfold open_w in *;
+rewrite <- subst_w_comm; auto;
+rewrite subst_order_irrelevant_free; simpl; auto;
+eapply H with (w:=w0) (G0:=(w'0, (v',A)::nil)::G1)
+  (Gamma':=Gamma') (Gamma'':=Gamma); auto;
+[ eauto | rew_app]; constructor; [ | symmetry]; auto;
+rewrite H5; rew_app; auto.
+rewrite H2; PPermut_simpl.
+destruct (eq_var_dec w w').
+subst.
+assert (G ~=~ G1 & (w'', Gamma'') /\ Gamma *=* Gamma').
+  apply ok_Bg_impl_ppermut with (w:=w'); [ | transitivity G0]; eauto;
+  rewrite H1; PPermut_simpl.
+destruct H5;
+eapply t_letdia_get_LF with (G:=G1) (Gamma:=Gamma++Gamma'')
+  (L_w:=L_w \u \{w''}) (L_t := L_t).
+clear H HT2 IHHT.
+rewrite H5 in Ok_Bg; eapply ok_Bg_split9; eauto.
+eapply IHHT with (w:=w'); auto; PPermut_simpl.
+intros; unfold open_t in *; unfold open_w in *;
+rewrite <- subst_w_comm; auto;
+rewrite subst_order_irrelevant_free; simpl; auto;
+eapply H with (w:=w0) (G0:=(w'0, (v',A)::nil)::G1)
+  (Gamma':=Gamma) (Gamma'':=Gamma''); auto;
+rew_app; constructor; auto;
+symmetry; transitivity ((G1 ++ (w'', Gamma'')::nil) & (w', Gamma)); auto;
+rew_app; auto.
+rewrite H2; PPermut_simpl.
+assert (G & (w, Gamma) ~=~ G1 & (w', Gamma') & (w'', Gamma'')) by
+  (symmetry; transitivity G0; symmetry; auto);
+assert (exists Gamma0, exists GH, exists GT,
+  Gamma0 *=* Gamma /\ G1 & (w'', Gamma'') = GH & (w, Gamma0) ++ GT) by
+  (apply PPermut_split_neq with (w:=w') (G':=G) (Gamma:=Gamma');
+   try symmetry; auto; transitivity (G1 & (w', Gamma') & (w'', Gamma'')); auto;
+  PPermut_simpl).
+assert (exists Gamma0, exists GH, exists GT,
+  Gamma0 *=* Gamma /\ G1 = GH & (w, Gamma0) ++ GT) by
+  (destruct H6 as (Gamma5, (GH, (GT, (H6a, H6b)))); subst;
+   apply PPermut_split_neq with (w:=w'') (G':=GH++GT) (Gamma:=Gamma''); auto;
+   [rewrite H6b; rew_app; auto | right; intro; subst; elim H4; reflexivity];
+  PPermut_simpl).
+destruct H7 as (Gamma'1, (GH, (GT, (H7a, H7b)))); subst.
+apply t_letdia_get_LF with (L_w:=L_w \u \{w''})
+  (L_t:=L_t) (A:=A) (G:=GH++GT & (w', Gamma'++Gamma'')) (Gamma:=Gamma).
+assert ((w, Gamma) :: G & (w0, Gamma0) ~=~ G0  & (w0, Gamma0)) by
+  (rewrite <- H0; auto);
+rewrite H7 in Ok_Bg; rewrite H1 in Ok_Bg.
+apply ok_Bg_ppermut with (G:= (GH & (w, Gamma'1) ++ GT) &
+  (w', Gamma' ++ Gamma'') & (w0, Gamma0));
+rew_app in *; eauto; try PPermut_simpl.
+clear IHHT H HT2. eapply ok_Bg_split10; eauto.
+eapply IHHT with (w1:=w) (G0:=GH++GT & (w0, Gamma0))
+  (Gamma':=Gamma') (Gamma'':=Gamma''); rew_app; auto;
+rew_app in *; transitivity ((GH ++ GT ++ (w', Gamma') ::
+  (w'', Gamma'') :: nil) & (w0, Gamma0));
+[ PPermut_simpl | rew_app]; auto;
+apply PPermut_last_rev_simpl with (a:=(w, Gamma));
+rewrite H5; symmetry; transitivity (GH ++ GT ++ (w, Gamma) :: (w', Gamma') ::
+  (w'', Gamma'') :: nil); [rew_app |  apply PPermut_app_head; symmetry]; auto;
+try PPermut_simpl.
+intros; unfold open_t in *; unfold open_w in *;
+rewrite <- subst_w_comm; auto;
+rewrite subst_order_irrelevant_free; simpl; auto;
+eapply H with (G0:=(w'0, (v', A) :: nil) :: (GH ++ GT) & (w, Gamma))
+  (Gamma':=Gamma') (Gamma'':=Gamma''); auto; PPermut_simpl.
+apply PPermut_last_rev_simpl with (a:=(w, Gamma)); rewrite H5;
+PPermut_simpl.
+rewrite H2; PPermut_simpl.
+Existential 1 := G.
+Existential 1 := Gamma'.
+Existential 1 := w'.
+Existential 1 := G.
+Existential 1 := Gamma'.
+Existential 1 := w'.
+Qed.
+
+Lemma rename_w_preserv_types_new:
+forall G w Gamma A M G' w' Gamma'
+  (HT: G |= (w, Gamma) |- M ::: A)
+  (GG': PPermut G (G' & (w', Gamma'))),
+  G' |= (w, Gamma ++ Gamma') |- {{ fwo w // fwo w' }} M ::: A.
+intros; apply rename_w_preserv_types with (G := G) (w := w) (w':= w'); eauto.
+Qed.
+
+Lemma rename_w_preserv_types_old:
+forall G w Gamma A M G' w' Gamma'
+  (HT: G |= (w, Gamma) |- M ::: A)
+  (GG': PPermut G (G' & (w', Gamma'))),
+  G' |= (w', Gamma' ++ Gamma) |- {{ fwo w' // fwo w }} M ::: A.
+intros; apply rename_w_preserv_types with (G := G) (w := w) (w':= w'); eauto.
+Qed.
+
+Lemma rename_w_preserv_types_outer:
+forall G G0 w Gamma A M G' w' Gamma' w'' Gamma''
+  (HT: G |= (w, Gamma) |- M ::: A)
+  (GG: PPermut G (G0 & (w', Gamma') & (w'', Gamma'')))
+  (GG': PPermut G' (G0 & (w', Gamma' ++ Gamma''))),
+  G' |= (w, Gamma) |- {{ fwo w' // fwo w'' }} M ::: A.
+intros; eapply rename_w_preserv_types; eauto.
+Qed.
+
+(*
+Proof sketch: double induction: on term and on typing
+  * for hypothesis, it is not possible to type it in empty context
+  * for cases where M is already a value, there is no problem
+  * otherwise we know, that for a simple term the theorem was true,
+  so we do case analysis to obtain the step
+  * the only exception is here M, where we know it is a value when
+  M was also a value
+*)
+Lemma Progress:
+forall G w M A
+  (H_lc_w: lc_w_LF M)
+  (H_lc_t: lc_t_LF M)
+  (HT: emptyEquiv G |= (w, nil) |- M ::: A),
+  value_LF M \/ exists N, (M, fwo w) |-> (N, fwo w).
+intros;
+remember (w, (@nil ty)) as Ctx;
+generalize dependent Ctx;
+generalize dependent A;
+generalize dependent w;
+generalize dependent G;
+induction M; intros; eauto using value_LF;
+inversion HeqCtx; subst.
+(* hyp *)
+inversion HT; subst;
+rewrite Mem_nil_eq in HT0;
+contradiction.
+(* appl *)
+right; inversion HT; subst;
+inversion H_lc_t; subst;
+inversion H_lc_w; subst;
+edestruct IHM1 with (A := A0 ---> A); eauto;
+[ inversion H0; subst; inversion HT1; subst; inversion H3 |
+  inversion H0];
+eexists; constructor; eauto;
+inversion H5; subst; auto.
+(* unbox & unbox_fetch *)
+right; inversion HT; subst;
+inversion H_lc_w; subst;
+inversion H_lc_t; subst.
+(* unbox *)
+edestruct IHM with (A := [*]A); eauto;
+[ inversion H0; subst; inversion HT0; subst; inversion H3 |
+  destruct H0];
+eexists; constructor; eauto;
+inversion H1; inversion H2; subst; auto;
+erewrite closed_var_subst_ctx; eauto; constructor.
+(* unbox_fetch *)
+assert (Gamma = nil) by
+  ( apply emptyEquiv_permut_empty with
+    (G:= (G0 & (w0, Gamma))) (G':=G) (w:=w0); auto;
+    apply Mem_last); subst;
+destruct IHM with (A := [*]A)
+                  (Ctx := (w0, (@nil ty)))
+                  (G := G0 & (w, nil))
+                  (w := w0);
+eauto.
+assert (emptyEquiv (G0 & (w, nil)) = G0 & (w, nil)) by
+  ( repeat rewrite emptyEquiv_rewrite; simpl;
+   apply emptyEquiv_permut_split_last in H6; rewrite H6; reflexivity);
+rewrite H0; auto.
+inversion H0; subst; inversion HT0; subst;
+eexists; constructor; eauto; inversion H2; auto; subst.
+inversion H3; subst; auto.
+destruct H0; eexists; constructor; eauto.
+(* here & get_here *)
+inversion HT; subst;
+inversion H_lc_w; subst;
+inversion H_lc_t; subst.
+(* here *)
+edestruct IHM; eauto;
+[ left; econstructor|
+  right; destruct H0; eexists];
+eauto using step_LF.
+(* get_here *)
+assert (Gamma = nil) by
+  ( apply emptyEquiv_permut_empty with
+    (G:= (G0 & (w0, Gamma))) (G':=G) (w:=w0); auto;
+    apply Mem_last); subst;
+destruct IHM with (A := A0)
+                  (Ctx := (w0, (@nil ty)))
+                  (G := G0 & (w, nil))
+                  (w := w0);
+eauto.
+assert (emptyEquiv (G0 & (w, nil)) = G0 & (w, nil)) by
+  ( repeat rewrite emptyEquiv_rewrite; simpl;
+   apply emptyEquiv_permut_split_last in H6; rewrite H6; reflexivity);
+rewrite H0; auto.
+left; inversion H0; subst; inversion HT0; subst;
+econstructor; eauto using step_LF.
+right; destruct H0; eexists;
+econstructor; eauto using step_LF.
+(* letdia & letdia_get *)
+right; inversion HT; subst;
+inversion H_lc_w; subst;
+inversion H_lc_t; subst.
+(* letdia *)
+edestruct IHM1 with (A := <*>A0); eauto;
+[ inversion H0; subst; inversion HT1; subst |
+  destruct H0];
+eexists; constructor; eauto.
+inversion H5; subst; auto.
+inversion H7; subst; auto.
+inversion H5; subst; auto.
+inversion H7; subst; auto.
+(* letdia_get *)
+assert (Gamma = nil) by
+  ( apply emptyEquiv_permut_empty with (G:= (G0 & (w0, Gamma))) (G':=G) (w:=w0);
+    auto; apply Mem_last); subst;
+edestruct IHM1 with (G := G0 & (w, nil))
+                    (w := w0)
+                    (Ctx := (w0, (@nil ty)))
+                    (A := <*>A0); eauto;
+assert ( emptyEquiv (G0 & (w, nil)) = G0 & (w, nil)) by
+   ( repeat rewrite emptyEquiv_rewrite; simpl;
+     apply emptyEquiv_permut_split_last in H6; rewrite H6; reflexivity).
+rewrite H0; auto.
+inversion H0; subst; inversion HT1; subst;
+eexists; constructor; eauto;
+try apply closed_t_succ; auto;
+inversion H5; inversion H8; subst; auto.
+destruct H0;
+eexists; constructor; eauto;
+try apply closed_t_succ; auto;
+inversion H5; inversion H8; subst; auto.
+Qed.
+
+(*
+   Proof sketch: double induction on typing and making a step
+   * FIXME: eauto takes ages :(
+   * for beta reduction we take a fresh variable and expand the
+   substitution a little bit, then apply the previously proven lemma
+   that substitution preserves types
+   * for unbox box reduction, the schema is basically the same
+   * for letdia here we combine the two above + use the knowledge
+   that term and world substitution can be done in any order
+*)
+Lemma Preservation:
+forall G M N A w
+  (HT: emptyEquiv G |= (w, nil) |- M ::: A)
+  (HS: (M, fwo w) |-> (N, fwo w)),
+  emptyEquiv G |= (w, nil) |- N ::: A.
+intros;
+remember (w, (@nil (var * ty))) as Ctx;
+remember (emptyEquiv G) as G';
+generalize dependent w;
+generalize dependent N;
+generalize dependent G;
+induction HT; intros;
+inversion HS; subst;
+try (inversion HeqCtx; subst);
+try (econstructor; eauto).
+(* appl_lam *)
+inversion HT1; subst;
+unfold open_t in *;
+assert (exists v, v \notin L \u free_vars_LF M0) as HF by apply Fresh;
+destruct HF as (v_fresh).
+rewrite subst_t_neutral_free with (v:=v_fresh);
+[ eapply subst_t_preserv_types_inner; eauto |
+  rewrite notin_union in H; destruct H]; auto.
+rewrite <- double_emptyEquiv; auto.
+(* unbox_box *)
+inversion HT; subst;
+assert (exists v, v \notin L \u (free_worlds_LF M0)) as HF by apply Fresh;
+destruct HF as (w_fresh);
+unfold open_w in *;
+replace ({{fwo w0 // bwo 0}}M0)
+  with ({{fwo w0 // fwo w_fresh}} {{fwo w_fresh // bwo 0}}M0)
+  by (rewrite subst_w_neutral_free; auto);
+replace (@nil (var * ty)) with (nil ++ (@nil (var * ty))); eauto;
+apply rename_w_preserv_types_old with (G := emptyEquiv G0 & (w0, nil));
+auto.
+(* unbox_fetch_box *)
+inversion HT; subst;
+assert (exists v, v \notin L \u (free_worlds_LF M0)) as HF by apply Fresh;
+destruct HF as (w_fresh);
+unfold open_w in *;
+replace ({{fwo w0 // bwo 0}}M0)
+  with ({{fwo w0 // fwo w_fresh}} {{fwo w_fresh // bwo 0}}M0)
+  by (rewrite subst_w_neutral_free; auto);
+replace (@nil (var * ty)) with (nil ++ (@nil (var * ty))); eauto;
+apply rename_w_preserv_types_old with (G := G & (w0, nil) & (w, Gamma));
+auto; PPermut_simpl.
+(* unbox_fetch *)
+assert (Gamma = nil) by
+  ( apply emptyEquiv_permut_empty with (G:= (G & (w, Gamma))) (G':=G0) (w:=w);
+    auto; apply Mem_last); subst;
+eapply IHHT with (G0:=G & (w0, nil)); eauto;
+repeat rewrite emptyEquiv_rewrite; simpl;
+apply emptyEquiv_permut_split_last in H; rewrite H; reflexivity.
+(* get_here *)
+assert (Gamma = nil) by
+  ( apply emptyEquiv_permut_empty with (G:= (G & (w, Gamma))) (G':=G0) (w:=w);
+    auto; apply Mem_last); subst;
+eapply IHHT with (G0:=G & (w0, nil)); eauto;
+repeat rewrite emptyEquiv_rewrite; simpl;
+apply emptyEquiv_permut_split_last in H; rewrite H; reflexivity.
+(* letdia + (here | get_here ) *)
+assert (exists w1, w1 \notin L_w \u free_worlds_LF N) as HF by apply Fresh;
+assert (exists v1, v1 \notin L_t \u free_vars_LF N) as HF2 by apply Fresh;
+destruct HF as (w_fresh); destruct HF2 as (v_fresh);
+inversion HT; subst.
+(* letdia #1 *)
+rewrite notin_union in *; destruct H0; destruct H1;
+unfold open_t in *; unfold open_w in *;
+rewrite subst_t_neutral_free with (v:=v_fresh);
+[ rewrite subst_order_irrelevant_bound |
+  apply subst_world_preserv_free_vars]; auto;
+[ rewrite <- subst_w_neutral_free with (w0:=w_fresh) |
+  constructor];
+[ apply subst_t_preserv_types_inner with (A:=A) |
+  apply subst_var_preserv_free_worlds]; auto;
+[ | rewrite <- double_emptyEquiv; auto];
+replace ((v_fresh, A) :: nil) with (nil ++ (v_fresh, A) :: nil) by auto;
+apply rename_w_preserv_types_new with
+  (G:= (w_fresh, (v_fresh, A)::nil) :: emptyEquiv G0);
+[ rewrite <- subst_order_irrelevant_bound |
+  rew_app]; auto; try PPermut_simpl; constructor.
+(* letdia #2 *)
+rewrite notin_union in *; destruct H0; destruct H1;
+unfold open_t in *; unfold open_w in *;
+rewrite subst_t_neutral_free with (v:=v_fresh);
+[ rewrite subst_order_irrelevant_bound |
+  apply subst_world_preserv_free_vars]; auto;
+[ rewrite <- subst_w_neutral_free with (w0:=w_fresh) |
+  constructor];
+[ eapply subst_t_preserv_types_outer with (A:=A) (G0:=G)
+  (Gamma':=Gamma) (w':=w) |
+  apply subst_var_preserv_free_worlds]; auto;
+rew_app;
+assert ( emptyEquiv (G & (w0, nil)) = G & (w0, nil)) by
+   ( repeat rewrite emptyEquiv_rewrite; simpl;
+     apply emptyEquiv_permut_split_last in H4; rewrite H4; reflexivity);
+assert (Gamma = nil) by
+  ( apply emptyEquiv_permut_empty with (G:= (G & (w, Gamma)))
+    (G':=G0) (w:=w); auto; apply Mem_last).
+subst; rew_app; rewrite <- H9 in HT0; auto.
+apply rename_w_preserv_types_outer with (G0:=G) (Gamma'':=(v_fresh,A) :: nil)
+      (Gamma':=Gamma) (G:=G & (w, Gamma) & (w_fresh, (v_fresh,A)::nil));
+assert (G & (w, Gamma) & (w_fresh, (v_fresh, A) :: nil) ~=~
+  (w_fresh, (v_fresh, A) :: nil) :: emptyEquiv G0) by PPermut_simpl.
+rewrite H11; rewrite <- subst_order_irrelevant_bound;
+[eapply HT2; auto | constructor].
+PPermut_simpl; auto.
+PPermut_simpl.
+(* letdia *)
+assert (exists w1, w1 \notin L_w \u free_worlds_LF N) as HF by apply Fresh;
+assert (exists v1, v1 \notin L_t \u free_vars_LF N) as HF2 by apply Fresh;
+destruct HF as (w_fresh); destruct HF2 as (v_fresh);
+inversion HT; subst.
+(* letdia #1 *)
+rewrite notin_union in *; destruct H1; destruct H2;
+unfold open_t in *; unfold open_w in *;
+rewrite subst_t_neutral_free with (v:=v_fresh);
+[ rewrite subst_order_irrelevant_bound |
+  apply subst_world_preserv_free_vars]; auto;
+[ rewrite <- subst_w_neutral_free with (w0:=w_fresh) |
+  constructor];
+[ eapply subst_t_preserv_types_outer with (A:=A) (G0:=G) (w':=w)
+  (Gamma':=Gamma) |
+ apply subst_var_preserv_free_worlds]; eauto;
+assert (Gamma = nil) by
+  (apply emptyEquiv_permut_empty with
+    (G:= (G & (w, Gamma))) (G':=G1) (w:=w); auto; apply Mem_last); subst;
+rew_app;
+assert ( emptyEquiv (G & (w0, nil)) = G & (w0, nil)) by
+   ( repeat rewrite emptyEquiv_rewrite; simpl;
+     apply emptyEquiv_permut_split_last in H0; rewrite H0; reflexivity);
+[ rewrite <- H5 in HT0 |
+  eapply rename_w_preserv_types_outer
+    with (G:= (w_fresh, (v_fresh,A)::nil):: G & (w,nil))
+         (Gamma'':=(v_fresh,A)::nil) (Gamma':=nil) (G0:=G)]; auto.
+rewrite <- subst_order_irrelevant_bound;
+[ eapply HT2; eauto | constructor].
+PPermut_simpl.
+(* letdia #2 *)
+assert (Gamma = nil) by
+  (apply emptyEquiv_permut_empty with
+    (G:= (G & (w, Gamma))) (G':=G1) (w:=w); auto; apply Mem_last); subst.
+assert (w <> w0) by eauto with ok_bg_rew.
+assert (w1 <> w) by eauto with ok_bg_rew.
+rewrite <- H0; rewrite notin_union in *; destruct H1; destruct H2;
+unfold open_t in *; unfold open_w in *; destruct (eq_var_dec w1 w0); subst.
+assert (G0  ~=~ G /\ Gamma0 *=* nil) by
+  (apply ok_Bg_impl_ppermut with (w:=w0); eauto);
+destruct H12; symmetry in H13; apply permut_nil_eq in H13;
+rewrite subst_t_neutral_free with (v:=v_fresh);
+[ eapply subst_t_preserv_types_inner with (A:=A) |
+  apply subst_world_preserv_free_vars]; eauto;
+[ rewrite subst_order_irrelevant_bound |
+  assert ( emptyEquiv (G & (w, nil)) = G & (w, nil)) by
+    ( repeat rewrite emptyEquiv_rewrite; simpl;
+      apply emptyEquiv_permut_split_last in H0; rewrite H0; reflexivity)];
+[ rewrite <- subst_w_neutral_free with (w0:=w_fresh) |
+  constructor | ]; auto;
+[ replace ((v_fresh,A)::nil) with (nil++(v_fresh,A)::nil) by auto |
+  apply subst_var_preserv_free_worlds | ]; auto.
+apply rename_w_preserv_types_new with
+  (G:= (w_fresh, (v_fresh,A)::nil) :: G0 & (w, nil));
+[ rewrite <- subst_order_irrelevant_bound; try constructor; subst |
+  rew_app; eauto].
+rewrite H12; eapply HT2; auto.
+PPermut_simpl.
+rewrite H14; rewrite <- H12; subst; auto.
+assert (Gamma0 = nil) by
+  ( apply emptyEquiv_permut_empty with (G:= (G0 & (w1, Gamma0)))
+      (G':=G & (w0, nil)) (w:=w1); auto;
+    assert (emptyEquiv G = G) by
+      (apply emptyEquiv_permut_split_last with (C:=(w, nil)) (H:=G1); auto);
+    [ rewrite emptyEquiv_rewrite; simpl | apply Mem_last ]; rewrite H12; auto);
+subst; assert (exists Gamma'', exists GH, exists GT,
+  Gamma'' *=* nil /\ G = GH & (w1, Gamma'') ++ GT) by
+  ( apply PPermut_split_neq with (w:=w0) (G':=G0) (Gamma:=nil);
+    [ symmetry | right; intro; subst; elim n]; auto);
+destruct H12 as (Gamma'', (GH, (GT, (H12a, H12b))));
+symmetry in H12a; apply permut_nil_eq in H12a; subst;
+rewrite subst_t_neutral_free with (v:=v_fresh);
+[ apply subst_t_preserv_types_outer with (A:=A) (G0 :=GH ++ GT & (w, nil))
+          (G := GH ++ GT & (w,nil) & (w1, (v_fresh, A) :: nil))
+       (G' := GH ++ GT & (w,nil) & (w0, nil)) (w' :=w1) (Gamma':=nil) |
+  apply subst_world_preserv_free_vars]; auto; subst; rew_app; auto.
+assert (G0 & (w, nil) ~=~ GH ++ GT & (w,nil) & (w0, nil)) by
+  ( transitivity ((GH++GT & (w0,nil) &(w, nil))); auto;
+    assert (G0 & (w1, nil) ~=~  (GH ++ GT & (w0, nil) & (w1, nil))) by
+      (transitivity ((GH & (w1, nil) ++ GT) & (w0, nil)); rew_app in *; auto);
+    assert (G0 ~=~ GH ++ GT & (w0, nil)) by
+      (apply PPermut_last_rev_simpl with (a:=(w1,nil)); rew_app in *; auto);
+  try PPermut_simpl;
+  rewrite H13; rew_app; auto); rew_app in *; rewrite <- H12.
+assert (emptyEquiv G0 = G0) by
+( assert (G0 ~=~ GH ++ GT & (w0, nil)) by
+    ( apply PPermut_last_rev_simpl with (a:=(w, nil));
+      transitivity (GH ++ GT & (w, nil) & (w0, nil)); rew_app in *; auto);
+  apply emptyEquiv_permut_split_last with (C:=(w1, nil)) (H := (w0, nil) ::
+    GH & (w1, nil) ++ GT);
+  assert (emptyEquiv ((w0, nil) :: GH & (w1, nil) ++ GT) = ((w0, nil) ::
+    GH & (w1, nil) ++ GT)) by
+  ( apply emptyEquiv_permut_split_last with (C:=(w, nil)) (H:= (w0,nil)::G1);
+    simpl; rewrite <- H0; rew_app; symmetry; auto);
+  rewrite H13; rewrite H14; rew_app;
+  transitivity (GH ++ (w0, nil) :: (w1, nil)::GT); auto; PPermut_simpl);
+rewrite emptyEquiv_rewrite; simpl; rewrite H13; auto.
+rewrite subst_order_irrelevant_bound;
+[ rewrite <- subst_w_neutral_free with (w0:=w_fresh) | constructor];
+[ apply rename_w_preserv_types_outer
+    with (G0 := GH ++ GT & (w,nil))
+         (G := (w_fresh, (v_fresh, A) :: nil) :: (GH & (w1, nil) ++ GT) &
+           (w, nil))
+         (Gamma':=nil)
+         (Gamma'':=(v_fresh, A)::nil) |
+  apply subst_var_preserv_free_worlds]; auto.
+rewrite <- subst_order_irrelevant_bound;
+[eapply HT2; eauto | constructor].
+PPermut_simpl.
+PPermut_simpl.
+(* letdia_step *)
+destruct (eq_var_dec w0 w); subst.
+eapply ok_Bg_first_last_neq in Ok_Bg;
+elim Ok_Bg; auto.
+assert (Gamma = nil) by
+  ( apply emptyEquiv_permut_empty with (G:= (G & (w, Gamma))) (G':=G1) (w:=w);
+    auto; apply Mem_last);
+subst;
+apply IHHT with (G0:=G & (w0,nil)) (w1:=w); auto;
+assert (emptyEquiv G = G) by
+  (apply emptyEquiv_permut_split_last with (C:=(w,nil)) (H:=G1); auto);
+rewrite emptyEquiv_rewrite; simpl; rewrite H1; reflexivity.
+Qed.
+
+Close Scope label_free_is5_scope.
+Close Scope is5_scope.
+Close Scope permut_scope.
