LabelFree/SingleUnbox/EmptyEquiv.v
@@ -1,0 +1,29 @@
+Require Export LFFPPermutLib.
+
+Fixpoint emptyEquiv (G: list (list (var * ty))) :=
+match G with
+| nil => nil
+| a::G' => (@nil (var * ty)) :: emptyEquiv G'
+end.
+
+Lemma emptyEquiv_permut_empty:
+forall G G',
+  G ~=~ emptyEquiv G' ->
+  forall C, Mem C G -> C = nil.
+Admitted.
+
+Lemma double_emptyEquiv:
+forall G,
+ emptyEquiv G = emptyEquiv (emptyEquiv G).
+Admitted.
+
+Lemma emptyEquiv_last:
+forall G,
+  emptyEquiv G & nil = (emptyEquiv G) & nil.
+Admitted.
+
+Lemma emptyEquiv_PPermut:
+forall G Gamma G',
+  G & Gamma ~=~ emptyEquiv G' ->
+  Gamma = nil.
+Admitted.
