LabelFree/SingleUnbox/OkLib.v
@@ -1,0 +1,116 @@
+Require Export PPermutLib.
+Require Export FSetLib.
+
+Inductive ok_LF {A}: list (prod var A) -> list var -> Prop :=
+| Ok_nil: forall U, ok_LF nil U
+| Ok_step: forall G T w U,
+  ~ Mem w U -> ok_LF G (w::U) -> ok_LF ((w, T)::G) U
+.
+
+Definition ok_Bg (G: bg_LF) : Prop := ok_LF (concat G) nil.
+
+Definition used_vars_ctx_LF (L: bg_LF) :=
+  from_list (map fst_ (concat L)).
+
+Lemma used_vars_app:
+forall x y,
+  used_vars_ctx_LF (x ++ y) = used_vars_ctx_LF x \u used_vars_ctx_LF y.
+induction x; intros; unfold used_vars_ctx_LF in *; rew_app; simpl.
+rewrite from_list_nil; rewrite union_empty_l; auto.
+rew_concat; rew_map; repeat rewrite from_list_app;
+rewrite <- IHx; rew_concat; rew_map; rewrite from_list_app;
+rewrite union_assoc; auto.
+Qed.
+
+Add Morphism used_vars_ctx_LF: PPermut_used_t.
+induction x; intros.
+apply PPermut_nil_impl in H; subst; auto.
+simpl; unfold used_vars_ctx_LF in *; simpl;
+rew_concat; rew_map.
+assert (a :: x ~=~ y) by auto.
+apply PPermut_split_head in H;
+destruct H as (l', (hd, (tl, (Ha, Hb)))).
+subst.
+assert (x & a ~=~  (hd ++ tl) & l').
+  transitivity (a::x); [ | rewrite H0];
+  PPermut_simpl.
+apply PPermut_last_rev in H; auto.
+rew_concat; rew_map;
+repeat rewrite from_list_app.
+rewrite IHx with (y:=hd ++ tl); auto.
+rew_concat; rew_map.
+rewrite from_list_app.
+rewrite <- union_comm_assoc.
+assert (from_list (map fst_ a) = from_list (map fst_ l')).
+  apply from_list_map; auto.
+rewrite H1; auto.
+Qed.
+
+Lemma ok_LF_used_permut:
+forall A G U U',
+  U *=* U' ->
+  (@ok_LF A G U) ->
+  (@ok_LF A G U').
+induction G; intros.
+destruct U'; econstructor; eauto.
+destruct a; inversion H0; subst;
+constructor; [ intro | apply IHG with (U:=v::U)]; auto;
+apply Mem_permut with (l':=U) in H1; [ elim H5 | symmetry]; auto.
+Qed.
+
+Lemma ok_LF_used_weakening:
+forall A G x U,
+  (@ok_LF A G (x::U)) ->
+  (@ok_LF A G U).
+induction G; intros; try constructor;
+destruct a; inversion H; subst;
+constructor.
+intro; apply Mem_permut with (l':=U) in H0; auto; elim H4;
+rewrite Mem_cons_eq; right; auto.
+apply ok_LF_used_permut with (U' := (x::v::U)) in H5;
+[ | permut_simpl]; apply IHG with (x:=x); auto.
+Qed.
+
+Lemma ok_LF_split:
+forall A G1 G2 U,
+  (@ok_LF A (G1++G2) U) ->
+  ok_LF G1 U /\ ok_LF G2 U.
+induction G1; intros; split; try destruct a; eauto using (@ok_LF A);
+rew_app in *; inversion H; subst; try constructor; auto.
+eapply IHG1 with (G2:=G2); auto.
+rew_app in *; inversion H; subst; eapply IHG1 with (G2:=G2); auto;
+eapply ok_LF_used_weakening in H5; eauto.
+Qed.
+
+Lemma ok_Bg_PPermut:
+forall G G',
+  ok_Bg G -> G ~=~ G' -> ok_Bg G'.
+Admitted. (* This will be fun... it goes from ok_LF G U (for any U) but then..*)
+
+Lemma ok_Bg_fresh:
+forall G Gamma x A,
+  ok_Bg (Gamma::G) ->
+  x \notin (used_vars_ctx_LF (Gamma::G)) ->
+  ok_Bg (((x, A) :: Gamma)::G).
+Admitted.
+
+Lemma ok_Bg_nil:
+forall G,
+  ok_Bg G ->
+  ok_Bg (nil::G).
+intros; unfold ok_Bg; rew_concat; rew_app; auto.
+Qed.
+
+Hint Resolve ok_Bg_nil.
+
+Lemma ok_Bg_concat:
+forall c1 c2 G0 G1 G2,
+  c1::c2::G0 ~=~ G1 ->
+  (c1++c2)::G0 ~=~ G2 ->
+  ok_Bg G1 <-> ok_Bg G2.
+Admitted.
+
+Lemma ok_Bg_empty:
+forall G,
+  ok_Bg (emptyEquiv G).
+Admitted.
