LabelFree/SingleUnbox/Semantics.v
@@ -1,0 +1,1499 @@
+Require Import Syntax.
+Require Import Substitution.
+Require Import LFFOkLib.
+Require Import LFFEmptyEquiv.
+
+Open Scope permut_scope.
+Open Scope is5_scope.
+
+Reserved Notation " G  '|=' Gamma '|-' M ':::' A" (at level 70).
+
+Inductive types_LF : bg_LF -> ctx_LF -> te_LF -> ty -> Prop :=
+
+| t_hyp_LF: forall A G Gamma v
+  (Ok: ok_Bg (Gamma::G))
+  (H: Mem (v, A) Gamma),
+  G |= Gamma |- hyp_LF (fte v) ::: A
+
+| t_lam_LF: forall L A B G Gamma M
+  (Ok: ok_Bg (Gamma::G))
+  (H: forall v, v \notin L ->
+    G |= (v, A)::Gamma |- M ^t^ (hyp_LF (fte v)) ::: B),
+  G |= Gamma |- lam_LF A M ::: A ---> B
+
+| t_appl_LF: forall A B G Gamma M N
+  (Ok: ok_Bg (Gamma::G))
+  (H1: G |= Gamma |- M ::: A ---> B)
+  (H2: G |= Gamma |- N ::: A),
+  G |= Gamma |- appl_LF M N ::: B
+
+| t_box_LF: forall G Gamma M A
+  (Ok: ok_Bg (G & Gamma))
+  (H: G & Gamma |= nil |- M ::: A),
+  G |= Gamma |- box_LF M ::: [*] A
+
+| t_unbox_LF: forall G Gamma M A
+  (Ok: ok_Bg (Gamma :: G))
+  (H: G |= Gamma |- M ::: [*] A),
+  G |= Gamma |- unbox_LF M ::: A
+
+| t_unbox_fetch_LF: forall G Gamma Gamma' M A
+  (Ok: ok_Bg (Gamma:: G & Gamma'))
+  (H: G & Gamma' |= Gamma |- M ::: [*] A),
+  forall G', G & Gamma ~=~ G' ->
+    G' |= Gamma' |- unbox_LF M ::: A
+
+| t_here_LF: forall A G Gamma M
+  (Ok: ok_Bg (Gamma :: G))
+  (H: G |= Gamma |- M ::: A),
+  G |= Gamma |- here_LF M ::: <*> A
+
+| t_get_here_LF: forall A G Gamma Gamma' M
+  (Ok: ok_Bg (Gamma :: G & Gamma'))
+  (H: G & Gamma' |= Gamma |- M ::: A),
+  forall G', G & Gamma ~=~ G' ->
+    G' |= Gamma' |- here_LF M ::: <*> A
+
+| t_letdia_LF: forall L A B G Gamma M N
+  (Ok_Bg: ok_Bg (Gamma :: G))
+  (HT1: G |= Gamma |- M ::: <*> A)
+  (HT2: forall G' v, v \notin L ->
+    ((v, A) :: nil) :: G ~=~ G' ->
+    G' |= Gamma |- N ^t^ (hyp_LF (fte v)) ::: B),
+  G |= Gamma |- letdia_LF M N ::: B
+
+| t_letdia_get_LF: forall L A B G Gamma Gamma' M N
+  (Ok_Bg: ok_Bg (Gamma :: G & Gamma'))
+  (HT1: G & Gamma' |= Gamma |- M ::: <*> A)
+  (HT2: forall v, v \notin L ->
+    ((v, A) :: nil) :: G & Gamma |= Gamma' |-
+      N ^t^ (hyp_LF (fte v))::: B),
+  forall G0, G & Gamma ~=~ G0 ->
+    G0 |= Gamma' |- letdia_LF M N ::: B
+
+where " G '|=' Gamma '|-' M ':::' A" := (types_LF G Gamma M A).
+
+Inductive value_LF: te_LF -> Prop :=
+| val_lam: forall A M, value_LF (lam_LF A M)
+| val_box: forall M, value_LF (box_LF M)
+| val_here: forall M, value_LF M -> value_LF (here_LF M)
+.
+
+Reserved Notation " M |-> N " (at level 70).
+
+Inductive step_LF: te_LF -> te_LF -> Prop :=
+
+| red_appl_lam_LF: forall M N A,
+  lc_t_n_LF 1 M -> lc_t_LF N ->
+  appl_LF (lam_LF A M) N |-> [N // bte 0] M
+
+| red_unbox_box_LF: forall M,
+  lc_t_LF M ->
+  unbox_LF (box_LF M)|-> M
+
+| red_letdia_here_LF: forall M N ,
+  lc_t_LF M -> lc_t_n_LF 1 N ->
+  letdia_LF (here_LF M) N |-> N ^t^ M
+
+| red_appl_LF: forall M M' N,
+  lc_t_LF M -> lc_t_LF N ->
+  M |-> M'->
+  appl_LF M N |-> appl_LF M' N
+
+| red_unbox_LF: forall M M',
+  lc_t_LF M -> M |-> M' ->
+  unbox_LF M |-> unbox_LF M'
+
+| red_here_LF: forall M M' ,
+  lc_t_LF M -> M |-> M' ->
+  here_LF M |-> here_LF M'
+
+| red_letdia_LF: forall M M' N,
+  lc_t_LF M -> lc_t_n_LF 1 N ->
+  M |-> M'->
+  letdia_LF M N |-> letdia_LF M' N
+
+where " M |-> N " := (step_LF M N ).
+
+Inductive steps_LF : te_LF -> te_LF -> Prop :=
+| single_step_LF: forall M M', M |-> M' -> steps_LF M M'
+| multi_step_LF: forall M M' M'',
+  M |-> M' -> steps_LF M' M'' -> steps_LF M M''
+.
+
+Lemma PPermutationG:
+forall G Gamma M A G',
+  G |= Gamma |- M ::: A ->
+  G ~=~ G' ->
+  G' |= Gamma |- M ::: A.
+intros; generalize dependent G'; induction H; intros; simpl in *.
+
+constructor; [apply ok_Bg_PPermut with (G:=Gamma::G)| ]; auto; PPermut_simpl.
+
+apply t_lam_LF with (L:=L);
+[apply ok_Bg_PPermut with (G:=Gamma::G)| ]; auto; PPermut_simpl.
+
+apply t_appl_LF with (A:=A);
+[apply ok_Bg_PPermut with (G:=Gamma::G)| |]; auto; PPermut_simpl.
+
+constructor;
+[apply ok_Bg_PPermut with (G:=G & Gamma)|]; auto.
+
+constructor;
+[apply ok_Bg_PPermut with (G:=Gamma::G)|]; auto.
+
+apply t_unbox_fetch_LF with (G:=G) (Gamma:=Gamma); auto. rewrite H0; auto.
+
+constructor;
+[apply ok_Bg_PPermut with (G:=Gamma::G)|]; auto.
+
+apply t_get_here_LF with (G:=G) (Gamma:=Gamma); auto. rewrite H0; auto.
+
+apply t_letdia_LF with (A:=A) (L:=L);
+[apply ok_Bg_PPermut with (G:=Gamma::G) | | ]; auto.
+intros; apply HT2; auto. rewrite H1; auto.
+
+apply t_letdia_get_LF with (A:=A) (L:=L) (G:=G) (Gamma:=Gamma);
+[apply ok_Bg_PPermut with (G:=Gamma::G & Gamma') | | | ]; auto.
+rewrite <- H2; auto.
+Qed.
+
+Lemma PermutationGamma:
+forall G Gamma M A Gamma',
+  G |= Gamma |- M ::: A ->
+  Gamma *=* Gamma' ->
+  G |= Gamma' |- M ::: A.
+intros. generalize dependent Gamma'.
+induction H; intros; simpl in *.
+
+constructor;
+[apply ok_Bg_PPermut with (G:=Gamma::G) |
+ apply Mem_permut with (l:=Gamma)]; auto.
+
+apply t_lam_LF with (L:=L);
+[apply ok_Bg_PPermut with (G:=Gamma::G) |]; auto.
+
+apply t_appl_LF with (A:=A);
+[apply ok_Bg_PPermut with (G:=Gamma::G) | |]; auto.
+
+constructor;
+[apply ok_Bg_PPermut with (G:=G & Gamma) |]; auto.
+apply PPermutationG with (G:=G & Gamma);
+auto.
+
+constructor;
+[apply ok_Bg_PPermut with (G:= Gamma :: G) |]; auto.
+
+apply t_unbox_fetch_LF with (G:=G) (Gamma:=Gamma);
+[apply ok_Bg_PPermut with (G:= Gamma :: G & Gamma') | |]; auto.
+apply PPermutationG with (G:=G & Gamma'); auto.
+
+constructor;
+[apply ok_Bg_PPermut with (G:= Gamma :: G) |]; auto.
+
+apply t_get_here_LF with (G:=G) (Gamma:=Gamma);
+[apply ok_Bg_PPermut with (G:= Gamma :: G & Gamma') | |]; auto.
+apply PPermutationG with (G:=G & Gamma'); auto.
+
+apply t_letdia_LF with (A:=A) (L:=L);
+[apply ok_Bg_PPermut with (G:= Gamma :: G) | |]; auto.
+
+apply t_letdia_get_LF with (A:=A) (L:=L) (G:=G) (Gamma:=Gamma);
+[apply ok_Bg_PPermut with (G:= Gamma :: G & Gamma') | | |]; auto.
+apply PPermutationG with (G:=G & Gamma'); auto.
+Qed.
+
+Lemma WeakeningG:
+forall G Gamma M A Delta,
+  G |= Gamma |- M ::: A ->
+  ok_Bg (Gamma::Delta::G) ->
+  Delta :: G |= Gamma |- M ::: A.
+intros; generalize dependent Delta; induction H;
+intros; simpl in *; eauto using types_LF.
+
+apply t_lam_LF with (L:=L \u used_vars_ctx_LF (Gamma:: Delta :: G));
+auto; intros;
+apply H0; auto; apply ok_Bg_fresh; auto;
+apply notin_Mem; rewrite notin_union in H2; destruct H2; auto.
+
+constructor;
+[apply ok_Bg_PPermut with (G:=Gamma::Delta::G) | rew_app ];
+auto. rew_app; PPermut_simpl. apply IHtypes_LF; apply ok_Bg_nil;
+apply ok_Bg_PPermut with (G:=Gamma::Delta::G); auto. PPermut_simpl.
+
+apply t_unbox_fetch_LF with (Gamma:=Gamma) (G:=Delta :: G);
+[apply ok_Bg_PPermut with (G:=Gamma'::Delta::G') | |]; auto;
+rew_app. rewrite <- H0; PPermut_simpl.
+apply IHtypes_LF; eapply ok_Bg_PPermut; eauto.
+rewrite <- H0; PPermut_simpl. rewrite H0; auto.
+
+apply t_get_here_LF with (Gamma:=Gamma) (G:=Delta :: G);
+[apply ok_Bg_PPermut with (G:=Gamma'::Delta::G') | |]; auto.
+rewrite <- H0; rew_app; PPermut_simpl.
+rew_app; apply IHtypes_LF; eapply ok_Bg_PPermut; eauto.
+rewrite <- H0; PPermut_simpl.
+rewrite <- H0; PPermut_simpl.
+
+apply t_letdia_LF with
+  (L:=L \u used_vars_ctx_LF (Gamma :: Delta :: G)) (A:=A);
+auto; intros.
+apply PPermutationG with (G:=Delta :: ((v, A)::nil) :: G).
+apply H0; auto.
+apply ok_Bg_PPermut with (G:=((v,A)::nil) :: Gamma :: Delta :: G).
+apply ok_Bg_fresh; [apply ok_Bg_nil | ]; auto.
+unfold used_vars_ctx_LF in *; rew_concat in *; eauto.
+PPermut_simpl. rewrite <- H3; PPermut_simpl.
+
+apply t_letdia_get_LF with
+  (L:=L \u from_list (map fst (Gamma' ++ Delta ++ concat G0)))
+  (A:=A) (G:=Delta::G) (Gamma:=Gamma);
+[apply ok_Bg_PPermut with (G:=Gamma'::Delta::G0) | | |]; auto.
+rewrite <- H1; PPermut_simpl.
+apply IHtypes_LF;
+apply ok_Bg_PPermut with (G:=Gamma'::Delta::G0); auto.
+rewrite <- H1; PPermut_simpl.
+intros; apply PPermutationG with (G:=Delta :: ((v, A) :: nil) :: G & Gamma).
+apply H0; auto.
+apply ok_Bg_PPermut with (G:= ((v, A)::nil) :: Gamma' :: Delta :: G0).
+apply ok_Bg_fresh; [apply ok_Bg_nil | ]; auto.
+unfold used_vars_ctx_LF in *; rew_concat in *; eauto.
+rewrite notin_union in H3; destruct H3; auto.
+rewrite H1; PPermut_simpl.
+rew_app; PPermut_simpl.
+rewrite <- H1; PPermut_simpl.
+Qed.
+
+Lemma WeakeningWithinContext:
+forall G Gamma M A,
+  G |= Gamma |- M ::: A ->
+  (forall Delta Delta' G',
+    G' & Delta ~=~ G ->
+    ok_Bg (Gamma :: G' & (Delta ++ Delta')) ->
+    G' & (Delta++Delta') |= Gamma |- M ::: A)
+  /\
+  (forall Gamma',
+    ok_Bg ((Gamma++Gamma')::G) ->
+    G |= Gamma ++ Gamma' |- M ::: A).
+intros G Gamma M A H;
+induction H; split; intros; subst.
+constructor; auto.
+constructor; auto; rewrite Mem_app_or_eq; left; auto.
+apply t_lam_LF with
+  (L:=L \u
+    (used_vars_ctx_LF (Gamma :: G' & (Delta ++ Delta'))));
+auto; intros; eapply H0; eauto;
+rew_app; apply ok_Bg_fresh; eauto; apply notin_Mem;
+rewrite notin_union in H3; destruct H3; auto.
+apply t_lam_LF with
+  (L:=L \u
+    (used_vars_ctx_LF ((Gamma ++ Gamma') :: G)));
+auto; intros; eapply H0; eauto;
+rew_app; apply ok_Bg_fresh; eauto;
+rewrite notin_union in H2; destruct H2; auto.
+econstructor; eauto; [eapply IHtypes_LF1 | eapply IHtypes_LF2]; eauto.
+econstructor; eauto; [eapply IHtypes_LF1 | eapply IHtypes_LF2]; eauto.
+econstructor;
+[apply ok_Bg_PPermut with (G:=Gamma:: G' & (Delta++Delta')) | ];
+auto. PPermut_simpl.
+apply PPermutationG with (G:= ((G'& Gamma) & (Delta ++ Delta'))).
+eapply IHtypes_LF. rewrite <- H0; PPermut_simpl.
+apply ok_Bg_nil; apply ok_Bg_PPermut with (G:=Gamma :: G' & (Delta ++ Delta'));
+auto. PPermut_simpl.
+econstructor;
+[apply ok_Bg_PPermut with (G:=(Gamma++Gamma'):: G) | ];
+auto. PPermut_simpl.
+eapply IHtypes_LF; auto.
+apply ok_Bg_nil; apply ok_Bg_PPermut with (G:=(Gamma++Gamma') :: G);
+auto. PPermut_simpl.
+constructor; eauto; eapply IHtypes_LF; eauto.
+constructor; eauto; eapply IHtypes_LF; eauto.
+assert (Delta::G'0 ~=~ G & Gamma).
+  transitivity G'; auto; rewrite <- H1; PPermut_simpl.
+assert ({Gamma *=* Delta} + {~ Gamma *=* Delta}).
+  eapply permut_dec; intros; destruct k; destruct k'; repeat decide equality.
+  apply eq_var_dec.
+destruct H4.
+(* Gamma *=* Delta *)
+assert (G'0 ~=~ G).
+  apply PPermut_last_rev with (Gamma:=Delta) (Gamma':=Gamma).
+  symmetry; auto.
+  rewrite <- H3; PPermut_simpl.
+apply t_unbox_fetch_LF with (G:=G'0) (Gamma:=Delta++Delta'); auto.
+apply ok_Bg_PPermut with (G:=Gamma'::G'0&(Delta++Delta')); auto.
+apply PPermutationG with (G:=G & Gamma'); auto.
+apply PermutationGamma with (Gamma:=Gamma++Delta'); auto.
+eapply IHtypes_LF.
+apply ok_Bg_PPermut with (G:=Gamma'::G'0&(Delta++Delta')); auto.
+rewrite H4; PPermut_simpl.
+(* ~ Gamma *=* Delta *)
+assert (G'0 & Delta ~=~ G & Gamma) by (rewrite <- H3; PPermut_simpl).
+apply PPermut_split_neq in H4; [ | intro; elim n; symmetry; auto];
+destruct H4 as (Gamma0, (hd, (tl, (H4, H5)))).
+subst.
+apply t_unbox_fetch_LF with (G:=hd++tl & (Delta++Delta')) (Gamma:=Gamma).
+apply ok_Bg_PPermut with (G:=Gamma' :: (hd & Gamma0 ++ tl) & (Delta ++ Delta'));
+auto; rew_app; PPermut_simpl.
+apply PPermutationG with (G:=(hd& Gamma' ++ tl) & (Delta ++ Delta')).
+eapply IHtypes_LF. rew_app; PPermut_simpl.
+apply PPermut_last_rev with (Gamma:=Gamma0) (Gamma':=Gamma); auto;
+rewrite <- H3; PPermut_simpl.
+apply ok_Bg_PPermut with (G:=Gamma' :: (hd & Gamma0 ++ tl) & (Delta ++ Delta'));
+auto; rew_app; PPermut_simpl.
+rew_app; PPermut_simpl.
+rew_app; PPermut_simpl.
+apply t_unbox_fetch_LF with (G:=G) (Gamma:=Gamma);
+[apply ok_Bg_PPermut with (G:=(Gamma'++Gamma'0):: G') | | ];
+auto. rewrite <- H0; PPermut_simpl.
+eapply IHtypes_LF; auto.
+apply ok_Bg_PPermut with (G:=(Gamma'++Gamma'0):: G'); auto.
+rewrite <- H0; PPermut_simpl.
+constructor; eauto; eapply IHtypes_LF; eauto.
+constructor; eauto; eapply IHtypes_LF; eauto.
+assert (G & Gamma ~=~ G'0 & Delta) by (rewrite  H1; auto).
+assert ({Gamma *=* Delta} + {~ Gamma *=* Delta}).
+  eapply permut_dec; intros; destruct k; destruct k'; repeat decide equality;
+  apply eq_var_dec.
+destruct H4.
+(* Gamma *=* Delta *)
+assert (G'0 ~=~ G).
+  apply PPermut_last_rev with (Gamma:=Delta) (Gamma':=Gamma).
+  symmetry; auto.
+  rewrite <- H3; PPermut_simpl.
+apply t_get_here_LF with (G:=G'0) (Gamma:=Delta++Delta'); auto.
+apply ok_Bg_PPermut with (G:=Gamma'::G'0&(Delta++Delta')); auto.
+apply PPermutationG with (G:=G & Gamma'); auto.
+apply PermutationGamma with (Gamma:=Gamma++Delta'); auto.
+eapply IHtypes_LF.
+apply ok_Bg_PPermut with (G:=Gamma'::G'0&(Delta++Delta')); auto.
+rewrite H4; PPermut_simpl.
+(* ~ Gamma *=* Delta *)
+assert (G'0 & Delta ~=~ G & Gamma) by (rewrite <- H3; PPermut_simpl).
+apply PPermut_split_neq in H4; [ | intro; elim n; symmetry; auto];
+destruct H4 as (Gamma0, (hd, (tl, (H4, H5)))).
+subst.
+apply t_get_here_LF with (G:=hd++tl & (Delta++Delta')) (Gamma:=Gamma).
+apply ok_Bg_PPermut with (G:=Gamma' :: (hd & Gamma0 ++ tl) & (Delta ++ Delta'));
+auto; rew_app; PPermut_simpl.
+apply PPermutationG with (G:=(hd& Gamma' ++ tl) & (Delta ++ Delta')).
+eapply IHtypes_LF. rew_app; PPermut_simpl.
+apply PPermut_last_rev with (Gamma:=Gamma0) (Gamma':=Gamma); auto.
+rewrite H3; PPermut_simpl.
+apply ok_Bg_PPermut with (G:=Gamma' :: (hd & Gamma0 ++ tl) & (Delta ++ Delta'));
+auto; rew_app; PPermut_simpl.
+rew_app; PPermut_simpl.
+rew_app; PPermut_simpl.
+apply t_get_here_LF with (G:=G) (Gamma:=Gamma);
+[apply ok_Bg_PPermut with (G:=(Gamma'++Gamma'0):: G') | | ];
+auto. rewrite <- H0; PPermut_simpl.
+eapply IHtypes_LF. auto.
+apply ok_Bg_PPermut with (G:=(Gamma'++Gamma'0):: G'); auto.  rewrite <- H0;
+PPermut_simpl.
+apply t_letdia_LF with (A:=A)
+  (L:=L \u (used_vars_ctx_LF (Gamma :: G' & (Delta ++ Delta'))));
+auto; [apply IHtypes_LF | intros]; auto.
+apply PPermutationG with (G:= (((v, A) :: nil) :: G') & (Delta ++ Delta')).
+eapply H0 with (G':=((v, A)::nil) :: G' & Delta).
+auto. rewrite H1; rew_app; PPermut_simpl. rew_app; PPermut_simpl.
+apply ok_Bg_PPermut with (G:=((v, A) :: nil) :: Gamma :: G' & (Delta ++Delta')).
+apply ok_Bg_fresh. apply ok_Bg_nil; auto.
+unfold used_vars_ctx_LF in *; rew_concat in *; eauto.
+rew_app; PPermut_simpl.
+rew_app; auto.
+apply t_letdia_LF with (A:=A)
+  (L:=L \u (used_vars_ctx_LF ((Gamma++Gamma') :: G)));
+auto; [apply IHtypes_LF | intros]; auto.
+eapply H0; eauto.
+apply ok_Bg_PPermut with (G:=((v, A) :: nil) :: (Gamma++Gamma') :: G).
+apply ok_Bg_fresh. apply ok_Bg_nil; auto.
+unfold used_vars_ctx_LF in *; rew_concat in *; eauto.
+rewrite <- H3; PPermut_simpl.
+assert (Gamma::G ~=~ G' & Delta).
+  transitivity G0; auto; rewrite <- H1; PPermut_simpl.
+assert ({Gamma *=* Delta} + {~ Gamma *=* Delta}).
+  eapply permut_dec; intros; destruct k; destruct k'; repeat decide equality.
+  apply eq_var_dec.
+destruct H5.
+(* Gamma *=* Delta *)
+assert (G ~=~ G').
+  apply PPermut_last_rev with (Gamma:=Gamma) (Gamma':=Delta).
+  auto.
+  rewrite <- H4; PPermut_simpl.
+apply t_letdia_get_LF with (A:=A)
+(L:=L \u used_vars_ctx_LF (nil :: Gamma' :: G' & (Delta ++ Delta'))) (G:=G')
+(Gamma:=Delta++Delta'); auto.
+apply ok_Bg_PPermut with (G:=Gamma'::G'&(Delta++Delta')); auto.
+apply PPermutationG with (G:=G & Gamma'); auto.
+apply PermutationGamma with (Gamma:=Gamma++Delta'); auto.
+eapply IHtypes_LF.
+apply ok_Bg_PPermut with (G:=Gamma'::G'&(Delta++Delta')); auto.
+rewrite H5; PPermut_simpl.
+intros; destruct H0 with (v:=v); auto.
+apply PPermutationG with (G:=((((v, A) :: nil) :: G') & (Delta ++ Delta'))).
+eapply H7. rewrite H5; PPermut_simpl.
+apply ok_Bg_PPermut with (G:=((v,A)::nil)::Gamma' :: G' & (Delta ++ Delta')).
+apply ok_Bg_fresh. auto. rewrite notin_union in H6; destruct H6. auto.
+PPermut_simpl. PPermut_simpl.
+(* ~ Gamma *=* Delta *)
+assert (G' & Delta ~=~ G & Gamma) by (rewrite <- H4; PPermut_simpl).
+apply PPermut_split_neq in H5; [ | intro; elim n; symmetry; auto];
+destruct H5 as (Gamma0, (hd, (tl, (H5, H6)))).
+subst.
+apply t_letdia_get_LF with (G:=hd++tl & (Delta++Delta')) (Gamma:=Gamma)
+ (L:=L \u used_vars_ctx_LF
+     (nil :: Gamma' :: (hd & Gamma0 ++ tl) & (Delta ++ Delta'))) (A:=A).
+apply ok_Bg_PPermut with (G:=Gamma' :: (hd & Gamma0 ++ tl) & (Delta ++ Delta'));
+auto; rew_app; PPermut_simpl.
+apply PPermutationG with (G:=(hd& Gamma' ++ tl) & (Delta ++ Delta')).
+eapply IHtypes_LF. rew_app; PPermut_simpl.
+apply PPermut_last_rev with (Gamma:=Gamma0) (Gamma':=Gamma); auto.
+transitivity (Gamma::G); auto. rewrite H4; PPermut_simpl. PPermut_simpl.
+apply ok_Bg_PPermut with (G:=Gamma' :: (hd & Gamma0 ++ tl) & (Delta ++ Delta'));
+auto; rew_app; PPermut_simpl.
+rew_app; PPermut_simpl.
+intros; destruct H0 with (v:=v); auto.
+apply PPermutationG with (G:=((((v, A) :: nil) :: Gamma0:: hd++tl) &
+  (Delta ++ Delta'))).
+eapply H7. PPermut_simpl; transitivity (Gamma::G); auto.
+rewrite H4; PPermut_simpl. PPermut_simpl.
+apply ok_Bg_PPermut with (G:=((v,A)::nil)::Gamma' ::
+  (hd & Gamma0 ++ tl) & (Delta ++ Delta')).
+apply ok_Bg_fresh. auto. rewrite notin_union in H6; destruct H6. auto.
+rew_app; PPermut_simpl. rew_app; PPermut_simpl.
+rew_app; PPermut_simpl.
+apply t_letdia_get_LF with (A:=A) (G:=G) (Gamma:=Gamma)
+  (L:=L \u (used_vars_ctx_LF ((Gamma' ++ Gamma'0) :: G0)));
+[apply ok_Bg_PPermut with (G:=(Gamma'++Gamma'0):: G0) | | | ];
+auto.  rewrite <- H1; PPermut_simpl.
+eapply IHtypes_LF. auto.
+apply ok_Bg_PPermut with (G:=(Gamma'++Gamma'0):: G0); auto. rewrite <- H1;
+PPermut_simpl.
+intros. eapply H0; eauto.
+apply ok_Bg_PPermut with (G:=((v,A)::nil) :: (Gamma'++Gamma'0) :: G0).
+apply ok_Bg_fresh. apply ok_Bg_nil; auto.
+unfold used_vars_ctx_LF in *; rew_concat in *; eauto.
+rewrite <- H1; PPermut_simpl.
+Qed.
+
+Lemma WeakeneningGamma:
+forall G Gamma M A Gamma',
+  G |= Gamma |- M ::: A ->
+  ok_Bg ((Gamma++Gamma')::G) ->
+  G |= Gamma ++ Gamma' |- M ::: A.
+intros; eapply WeakeningWithinContext; eauto.
+Qed.
+
+Lemma WeakeningWithinG:
+forall G Gamma M A Delta Delta',
+  G & Delta |= Gamma |- M ::: A ->
+  ok_Bg (Gamma :: G & (Delta ++ Delta')) ->
+  G & (Delta++Delta')|= Gamma |- M ::: A.
+intros; eapply WeakeningWithinContext; eauto.
+Qed.
+
+Lemma subst_t_preserv_types:
+forall G Gamma B M N v A
+  (H_lc_t: lc_t_LF M)
+  (HT: G |= Gamma |- N ::: B),
+  (* "inner" substitution *)
+  ( forall Gamma0,
+    Gamma *=* ((v, A) :: Gamma0) ->
+    emptyEquiv G |= nil |- M ::: A ->
+    G |= Gamma0 |- [M // fte v] N ::: B)
+  /\
+  (* "outer" substitution *)
+  ( forall G0 G' G'' Gamma',
+    G ~=~ (G0 & ((v,A)::Gamma')) ->
+    G' ~=~ (G0 & Gamma) ->
+    G'' ~=~ (G0 & Gamma') ->
+    emptyEquiv G' |= nil |- M ::: A ->
+    G'' |= Gamma |- [M // fte v] N ::: B).
+(*
+intros;
+generalize dependent v;
+generalize dependent A;
+generalize dependent M;
+induction HT; split; intros;
+simpl in *.
+
+(* hyp *)
+case_if.
+inversion H1; subst;
+assert (A = A0) by (eapply ok_Bg_Mem_eq; eauto);
+subst; replace G with (G ++ nil) by (rew_app; auto);
+apply types_weakened;
+[eapply ok_Bg_permut_first_tail with (C:=Gamma0) | ]; rew_app; eauto.
+constructor;
+[ apply ok_Bg_permut_first_tail with (C:=Gamma0) (x:=v0) (A:=A0) |
+  apply Mem_permut with (l' := (v0, A0) :: Gamma1) in HT]; eauto.
+rewrite Mem_cons_eq in HT; destruct HT; auto;
+inversion H2; subst; elim H1; reflexivity.
+
+case_if.
+inversion H3; subst;
+eapply ok_Bg_Mem_contradict in Ok_Bg;
+contradiction || eauto.
+constructor; auto;
+apply ok_Bg_ppermut with (G:=((w0, Gamma0)::G0) & (w', Gamma'));
+[ rewrite H1 |
+  eapply ok_Bg_permut_no_last; rewrite H in Ok_Bg; rew_app]; eauto.
+
+(* lam *)
+apply t_lam_LF with (L:=L \u \{v});
+[ apply ok_Bg_permut_first_tail with (C:=Gamma0) (x:=v) (A:=A0) |
+  intros]; auto;
+rewrite notin_union in H2; rewrite notin_singleton in H2; destruct H2;
+unfold open_t in *;
+rewrite <- subst_t_comm; auto;
+eapply H; auto;
+permut_simpl || rew_app; eauto.
+
+apply t_lam_LF with (L:=L \u \{v});
+[ apply ok_Bg_ppermut with (G:=((w0, Gamma0)::G0) & (w', Gamma'));
+  [ rewrite H2 |
+    rewrite H0 in Ok_Bg; rew_app] |
+  intros]; eauto with ok_bg_rew;
+rewrite notin_union in H4; rewrite notin_singleton in H4; destruct H4;
+unfold open_t in *;
+rewrite <- subst_t_comm; auto;
+eapply H with (G0:=G0) (w':=w'); eauto;
+assert (emptyEquiv G' ~=~ emptyEquiv (G0 ++ nil & (w0, (v', A) :: Gamma0))) as E
+ by (rewrite H1; rew_app; eapply emptyEquiv_last_change; auto);
+rew_app in *; rewrite <- E; auto.
+
+(* appl *)
+econstructor;  [ | eapply IHHT1 | eapply IHHT2];
+try apply ok_Bg_permut_first_tail with (C:=Gamma0) (x:=v) (A:=A0); eauto.
+
+econstructor;
+[ apply ok_Bg_ppermut with (G:=((w0, Gamma0)::G0) & (w', Gamma'));
+  [rewrite H1 | rewrite H in Ok_Bg] |
+  eapply IHHT1 |
+  eapply IHHT2]; eauto;
+apply ok_Bg_permut_no_last_spec in Ok_Bg; rew_app; auto.
+
+(* box *)
+apply t_box_LF with (L:=L \u used_w_vars (emptyEquiv G & (w0, nil)));
+[ apply ok_Bg_permut_no_last with (v:=v) (A:=A0);
+  eapply ok_Bg_permut_last |
+  intros; unfold open_w]; eauto;
+rewrite <- subst_order_irrelevant_bound;
+[ eapply H; eauto |
+  repeat rewrite emptyEquiv_rewrite];
+simpl; rew_app; auto;
+apply BackgroundSubsetImpl with (G:=emptyEquiv G); auto;
+[ exists ((w', (@nil (prod var ty))) :: nil); rew_app; auto |
+  assert ((w0, nil) :: emptyEquiv G & (w', nil) ~=~
+    (w', nil) :: emptyEquiv G & (w0, nil)) by auto];
+rew_app; rewrite emptyEquiv_rewrite_last; simpl; auto;
+rewrite H3;
+apply ok_Bg_fresh_wo; auto;
+apply emptyEquiv_ok_Bg in Ok_Bg;
+rewrite emptyEquiv_rewrite in Ok_Bg;
+simpl in *; auto.
+
+apply t_box_LF with
+  (L:=L \u used_w_vars(emptyEquiv G0 ++ (w', nil) :: (w0, nil) :: nil));
+[ rewrite H2; rewrite H0 in Ok_Bg |
+  intros; unfold open_w; rewrite <- subst_order_irrelevant_bound];
+eauto with ok_bg_rew;
+eapply H with (G'' := G'' & (w0, Gamma0)) (G0:=G0 & (w0, Gamma0)) (w'0:=w')
+  (Gamma':=Gamma') (A0:=A0); auto;
+repeat rewrite emptyEquiv_rewrite;
+simpl; rew_app; try PPermut_simpl;
+apply BackgroundSubsetImpl with (G:=emptyEquiv G0 & (w0, nil));
+[ rewrite H1 in H3; rewrite emptyEquiv_rewrite in H3 |
+  exists ((w'0, (@nil (var * ty)))::nil); rew_app |
+  apply emptyEquiv_ok_Bg in Ok_Bg; rewrite H0 in Ok_Bg]; auto;
+repeat rewrite emptyEquiv_rewrite in Ok_Bg;
+simpl in *; rew_app in *;
+apply ok_Bg_ppermut with
+  (G:=(w'0, nil) :: emptyEquiv G0 ++ (w', nil) :: (w0, nil) :: nil);
+[eauto with ppermut_rew | apply ok_Bg_fresh_wo ]; auto.
+
+(* unbox *)
+econstructor; [ | eapply IHHT];
+try apply ok_Bg_permut_first_tail with (C:=Gamma0) (x:=v) (A:=A0); eauto.
+
+econstructor;
+[ rewrite H1; rewrite H in Ok_Bg |
+  eapply IHHT]; eauto with ok_bg_rew.
+
+(* unbox_fetch *)
+apply t_unbox_fetch_LF with (G:=G) (Gamma:=Gamma); auto;
+[ apply ok_Bg_permut_no_last_spec with (v:=v) (A:=A0);
+  apply ok_Bg_ppermut with (G:= (w, Gamma) :: G & (w0, Gamma0)) |
+  eapply IHHT; eauto; rewrite <- H in H1; rew_app]; auto.
+
+destruct (eq_var_dec w w'0).
+(* = *)
+subst;
+assert (G ~=~ G0 /\ Gamma *=* (v, A0) :: Gamma'0) as HP by
+  (apply ok_Bg_impl_ppermut with (w:=w'0);
+   [eauto with ok_bg_rew | transitivity G'; auto]);
+destruct HP;
+apply t_unbox_fetch_LF with (G:=G) (Gamma:=Gamma'0);
+eauto with ok_bg_rew;
+specialize IHHT with (Gamma1:=Gamma) (w:=w'0);
+destruct IHHT with (M0:=M0) (A0:=A0) (v:=v); auto;
+[ apply H6; auto; rewrite H1 in H3; rewrite H4 |
+  rewrite H4; symmetry]; auto.
+(* <> *)
+assert (exists Gamma', exists GH, exists GT,
+  Gamma' *=* (v, A0)::Gamma'0 /\ G = GH & (w'0, Gamma') ++ GT) as HP by
+  (apply PPermut_split_neq with (w:=w) (Gamma:=Gamma) (G':=G0);
+    auto; transitivity G'; auto).
+destruct HP as (Gamma', (GH, (GT, (HPa, HPb)))).
+assert (GH & (w'0, Gamma') ++ GT ~=~ GH & (w'0, (v, A0)::Gamma'0) ++ GT)
+  by PPermut_simpl;
+apply t_unbox_fetch_LF with (G:=GH ++ GT & (w'0, Gamma'0)) (Gamma:=Gamma).
+subst;
+apply ok_Bg_ppermut with
+  (G:= (((w, Gamma) :: (GH & (w0, Gamma0) ++ GT)) & (w'0, Gamma'0)));
+[rew_app | ]; auto;
+apply ok_Bg_permut_no_last_spec with (v:=v)(A:=A0).
+apply ok_Bg_ppermut with
+  (G:=(w, Gamma):: (GH & (w'0, Gamma') ++ GT) & (w0, Gamma0));
+rew_app in *; auto; PPermut_simpl.
+eapply IHHT with (w1:=w) (Gamma1:=Gamma) (w':=w'0) (Gamma':=Gamma'0)
+                 (G0:=GH ++ GT & (w0, Gamma0)); rew_app; auto; subst;
+rew_app; auto;
+rewrite H1 in H3;
+assert (GH ++ (w, Gamma) :: GT ~=~ G0) by
+  (apply PPermut_last_rev_simpl with (a:=(w'0, (v, A0) :: Gamma'0));
+  rew_app in *; rewrite <- H0; rewrite <- H; auto; PPermut_simpl).
+PPermut_simpl; eauto.
+assert (GH ++ (w, Gamma) :: GT & (w0, Gamma0) ~=~ G0 & (w0,Gamma0)) by
+  (rewrite <- H5; rew_app; auto; PPermut_simpl);
+rewrite H6; auto.
+subst; rewrite H2; PPermut_simpl.
+apply PPermut_last_rev with (w:=w'0) (Gamma:=Gamma') (Gamma':=(v,A0)::Gamma'0);
+[ | symmetry]; auto; transitivity G'; auto; rewrite <- H; PPermut_simpl.
+
+(* here *)
+econstructor; [ | eapply IHHT];
+try apply ok_Bg_permut_first_tail with (C:=Gamma0) (x:=v) (A:=A0); eauto.
+
+econstructor;
+[ rewrite H1; rewrite H in Ok_Bg |
+  eapply IHHT]; eauto with ok_bg_rew.
+
+(* get_here *)
+apply t_get_here_LF with (G:=G) (Gamma:=Gamma); auto;
+[ apply ok_Bg_permut_no_last_spec with (v:=v) (A:=A0);
+  apply ok_Bg_ppermut with (G:= (w, Gamma) :: G & (w0, Gamma0)) |
+  eapply IHHT; eauto; rewrite <- H in H1; rew_app]; auto.
+
+destruct (eq_var_dec w w'0).
+(* = *)
+subst;
+assert (G ~=~ G0 /\ Gamma *=* (v, A0) :: Gamma'0) as HP by
+  (apply ok_Bg_impl_ppermut with (w:=w'0);
+   [eauto with ok_bg_rew | transitivity G'; auto]);
+destruct HP;
+apply t_get_here_LF with (G:=G) (Gamma:=Gamma'0);
+eauto with ok_bg_rew;
+specialize IHHT with (Gamma1:=Gamma) (w:=w'0);
+destruct IHHT with (M0:=M0) (A0:=A0) (v:=v); auto;
+[ apply H6; auto; rewrite H1 in H3; rewrite H4 |
+  rewrite H4; symmetry]; auto.
+(* <> *)
+assert (exists Gamma', exists GH, exists GT,
+  Gamma' *=* (v, A0)::Gamma'0 /\ G = GH & (w'0, Gamma') ++ GT) as HP by
+  (apply PPermut_split_neq with (w:=w) (Gamma:=Gamma) (G':=G0);
+    eauto; transitivity G'; auto).
+destruct HP as (Gamma', (GH, (GT, (HPa, HPb)))).
+assert (GH & (w'0, Gamma') ++ GT ~=~ GH & (w'0, (v, A0)::Gamma'0) ++ GT)
+  by PPermut_simpl;
+apply t_get_here_LF with (G:=GH ++ GT & (w'0, Gamma'0)) (Gamma:=Gamma).
+subst;
+apply ok_Bg_ppermut with
+  (G:= (((w, Gamma) :: (GH & (w0, Gamma0) ++ GT)) & (w'0, Gamma'0)));
+[rew_app | ]; auto;
+apply ok_Bg_permut_no_last_spec with (v:=v)(A:=A0).
+apply ok_Bg_ppermut with
+  (G:=(w, Gamma):: (GH & (w'0, Gamma') ++ GT) & (w0, Gamma0));
+rew_app in *; auto; PPermut_simpl.
+eapply IHHT with (w1:=w) (Gamma1:=Gamma) (w':=w'0) (Gamma':=Gamma'0)
+                 (G0:=GH ++ GT & (w0, Gamma0)) (A0:=A0); rew_app; auto; subst;
+rew_app; auto;
+rewrite H1 in H3;
+assert (GH ++ (w, Gamma) :: GT ~=~ G0) by
+  (apply PPermut_last_rev_simpl with (a:=(w'0, (v, A0) :: Gamma'0));
+  rew_app in *; rewrite <- H0; rewrite <- H; auto; PPermut_simpl).
+PPermut_simpl; auto.
+assert (GH ++ (w, Gamma) :: GT & (w0, Gamma0) ~=~ G0 & (w0,Gamma0)) by
+  (rewrite <- H5; rew_app; auto; PPermut_simpl);
+rewrite H6; auto.
+subst; rewrite H2; PPermut_simpl.
+apply PPermut_last_rev with (w:=w'0) (Gamma:=Gamma') (Gamma':=(v,A0)::Gamma'0);
+[ | symmetry]; auto; transitivity G'; auto; rewrite <- H; PPermut_simpl.
+
+(* letdia *)
+apply t_letdia_LF with
+  (L_t := L_t \u \{v})
+  (L_w := L_w \u used_w_vars ((w0, nil) :: emptyEquiv G)) (A:=A);
+[ apply ok_Bg_permut_first_tail with (C:=Gamma0) (x:=v) (A:=A0) |
+  eapply IHHT |
+  intros]; eauto;
+unfold open_t in *; unfold open_w in *;
+rewrite notin_union in H2; rewrite notin_singleton in H2; destruct H2;
+rewrite <- subst_order_irrelevant_bound;
+[ rewrite <- subst_t_comm | assumption ];
+[ eapply H | |] ; eauto;
+apply BackgroundSubsetImpl with (G:=emptyEquiv G); auto;
+[ exists ((w', (@nil (var*ty)))::nil);
+  PPermut_simpl ; rew_app; PPermut_simpl | ].
+assert ((w0, nil) :: (w', nil) :: emptyEquiv G ~=~
+  (w',nil) :: (w0, nil) :: emptyEquiv G) by PPermut_simpl;
+rewrite H5; apply ok_Bg_fresh_wo;
+[ apply emptyEquiv_ok_Bg in Ok_Bg;  simpl in * | ]; auto.
+
+eapply t_letdia_LF with
+  (L_t := L_t \u \{v})
+  (L_w := L_w \u  used_w_vars ((w', nil) :: emptyEquiv (G0 & (w0, Gamma0))));
+[ rewrite H2; rewrite H0 in Ok_Bg | eapply IHHT | intros]; eauto with ok_bg_rew;
+unfold open_t in *; unfold open_w in *.
+rewrite notin_union in H4; rewrite notin_singleton in H4; destruct H4;
+rewrite <- subst_order_irrelevant_bound;
+[ rewrite <- subst_t_comm | assumption ];
+[ eapply H with (G0:=(w'0, (v',A)::nil)::G0) (w'0:=w')
+  (Gamma':=Gamma') (A0:=A0) | | ]; auto;
+rew_app; rewrite H1 in H3; rew_app in *; simpl; try PPermut_simpl;
+apply BackgroundSubsetImpl with (G:= emptyEquiv (G0 & (w0, Gamma0))); auto;
+[exists ((w'0, (@nil (var*ty))):: nil); PPermut_simpl | ];
+assert ((w'0, nil) :: (w', nil)::emptyEquiv(G0 & (w0, Gamma0)) ~=~
+  (w', nil) :: (w'0, nil) :: emptyEquiv (G0 & (w0, Gamma0))) by auto;
+rewrite <- H7; apply ok_Bg_fresh_wo;
+[rewrite H0 in Ok_Bg; apply emptyEquiv_ok_Bg in Ok_Bg | ]; auto;
+  assert (emptyEquiv((w', (v, A0) :: Gamma') :: G0 & (w0, Gamma0)) ~=~
+    (w', nil) :: emptyEquiv (G0 & (w0, Gamma0))) by (simpl; auto);
+rewrite <- H8;
+assert ((w0, Gamma0) :: G0 & (w', (v, A0) :: Gamma') ~=~
+  ((w', (v, A0) :: Gamma') :: G0 & (w0, Gamma0))) by auto;
+rewrite <- H9; auto.
+
+(* letdia_get *)
+assert (w <> w0) by eauto with ok_bg_rew;
+eapply t_letdia_get_LF with (G:=G) (Gamma:=Gamma) (L_t := L_t \u \{v}) (A:=A)
+  (L_w:=L_w \u used_w_vars ((w0, nil) :: emptyEquiv (G & (w, Gamma)))); auto.
+apply ok_Bg_permut_no_last_spec with (v:=v) (A:=A0);
+apply ok_Bg_ppermut with (G:= (w, Gamma) :: G & (w0, Gamma0)); auto.
+eapply IHHT with (w':=w0) (Gamma':=Gamma1) (v:=v) (A0:=A0); auto.
+rew_app; rewrite <- H0 in H2; auto.
+intros; unfold open_t in *; unfold open_w in *;
+rewrite notin_union in H5; rewrite notin_singleton in H5; destruct H5;
+rewrite <- subst_order_irrelevant_bound;
+[rewrite <- subst_t_comm | ]; auto.
+eapply H with (v:=v) (A0:=A0); auto.
+rewrite <- H0 in H2;
+apply BackgroundSubsetImpl with (G:=emptyEquiv (G & (w, Gamma))); auto;
+[ exists ((w', (@ nil (var * ty)))::nil); PPermut_simpl | ];
+assert ((w0, nil) :: (w', nil) :: emptyEquiv (G & (w, Gamma)) ~=~
+  (w', nil) :: (w0, nil) ::emptyEquiv (G & (w, Gamma))) by PPermut_simpl;
+rewrite H8;
+apply ok_Bg_fresh_wo; [apply emptyEquiv_ok_Bg in Ok_Bg | auto];
+assert ((w, Gamma) :: G & (w0, Gamma0) ~=~ (w0, Gamma0):: G & (w, Gamma)) by
+  auto;
+rewrite H9 in Ok_Bg; simpl in Ok_Bg; auto.
+
+assert (w <> w0) by eauto with ok_bg_rew;
+destruct (eq_var_dec w w'); subst.
+(* = *)
+assert (G ~=~ G1 /\ Gamma *=* (v, A0) :: Gamma') by
+  (apply ok_Bg_impl_ppermut with (w:=w');
+    [ | rewrite H0; rewrite <- H1]; eauto);
+destruct H7; rewrite H3; rewrite <- H7;
+apply t_letdia_get_LF with (G:=G) (Gamma:=Gamma') (L_t:=L_t \u \{v}) (A:=A)
+  (L_w:=L_w \u used_w_vars ((w', nil) :: emptyEquiv (G1 & (w0, Gamma0)))).
+eauto with ok_bg_rew.
+eapply IHHT with (v:=v) (A0:=A0); auto;
+rewrite H2 in H4; rewrite H7; auto.
+intros; unfold open_t in *; unfold open_w in *;
+rewrite notin_union in H9; rewrite notin_singleton in H9; destruct H9;
+rewrite <- subst_order_irrelevant_bound;
+[ rewrite <- subst_t_comm | ]; auto.
+edestruct H with (v:=v) (w'0 := w'0) (Gamma1:=Gamma0) (A0:=A0)
+  (v':=v') (M:=M0) as (Ha, Hb);
+auto.
+eapply Hb with (G0 := (w'0, (v',A)::nil) ::G) (w'1 := w') (Gamma':=Gamma');
+[ | auto |  | ]; try PPermut_simpl.
+rewrite H2 in H4; rewrite H7.
+apply BackgroundSubsetImpl with (G:=emptyEquiv (G1 & (w0, Gamma0))); auto.
+exists (((w'0, (@nil (prod var ty))) :: nil)); rew_app; simpl; auto;
+PPermut_simpl.
+assert ((w', nil) :: (w'0, nil) :: emptyEquiv (G1 & (w0, Gamma0)) ~=~
+  (w'0, nil) :: (w',nil) :: emptyEquiv (G1 & (w0, Gamma0))) by auto;
+rewrite H12; apply ok_Bg_fresh_wo; auto;
+assert ((w', nil) :: emptyEquiv (G1 & (w0, Gamma0)) ~=~
+  emptyEquiv ((w', Gamma) :: G & (w0, Gamma0))) by
+  (simpl in *; rewrite H7; auto);
+rewrite H13; apply emptyEquiv_ok_Bg in Ok_Bg; auto.
+auto.
+(* <> *)
+assert (G & (w, Gamma) ~=~ G1 & (w', (v, A0) :: Gamma')) by
+  (transitivity G0; auto);
+symmetry in H7;
+assert (exists Gamma0, exists GH, exists GT,
+  Gamma0 *=* Gamma /\ G1 = GH & (w, Gamma0) ++ GT) by
+  (apply PPermut_split_neq with (w:=w') (Gamma:=(v,A0) :: Gamma') (G':=G);
+    auto);
+destruct H8 as (Gamma'', (GH, H8)); destruct H8 as (GT, H8);
+destruct H8.
+apply t_letdia_get_LF with (G:=GH++GT & (w', Gamma')) (Gamma:=Gamma) (A:=A)
+  (L_t:=L_t \u \{v}) (L_w:=L_w \u used_w_vars
+     ((w', nil) :: emptyEquiv (GH ++ GT ++ (w, Gamma) :: (w0, Gamma0) :: nil))).
+assert (G & (w, Gamma) & (w0, Gamma0) ~=~ (w, Gamma) :: G & (w0, Gamma0)) by
+  auto.
+rewrite <- H10 in Ok_Bg; rewrite <- H7 in Ok_Bg;
+subst; apply ok_Bg_ppermut with
+  (G:=((w, Gamma) :: (GH & (w', Gamma') ++ GT) & (w0, Gamma0))); [ | rew_app];
+auto.
+apply ok_Bg_ppermut with
+  (G:= (((w, Gamma) :: (GH & (w0, Gamma0) ++ GT)) & (w', Gamma')));
+[rew_app; PPermut_simpl | apply ok_Bg_permut_no_last_spec with (v:=v)(A:=A0)];
+apply ok_Bg_ppermut with
+  ((GH & (w, Gamma'') ++ GT) & (w', (v, A0) :: Gamma') & (w0, Gamma0));
+[ rew_app | ]; auto; try PPermut_simpl.
+eapply IHHT with (w1:=w) (Gamma1:=Gamma) (A0:=A0) (w':=w')
+  (G0:=GH++GT & (w0,Gamma0)) (Gamma':=Gamma'); auto;
+[ symmetry; subst; rew_app in * | rew_app | ]; auto.
+PPermut_simpl; apply PPermut_last_rev_simpl with (a:=(w, Gamma));
+rewrite <- H7; PPermut_simpl.
+rewrite H2 in H4; rewrite H9 in H4;
+assert ((GH & (w, Gamma'') ++ GT) & (w0, Gamma0) ~=~
+  (GH ++ GT & (w0, Gamma0)) ++ nil & (w, Gamma)) by (rew_app; PPermut_simpl);
+rewrite <- H10; auto.
+intros; unfold open_t in *; unfold open_w in *;
+rewrite notin_union in H10; rewrite notin_singleton in H10; destruct H10;
+rewrite <- subst_order_irrelevant_bound;
+[rewrite <- subst_t_comm | ]; auto;
+eapply H with (v':=v') (w':=w'0) (Gamma1:=Gamma0) (w1:=w0) (A0:=A0)
+              (v:=v) (G0:=(w'0, (v', A) :: nil) :: (GH ++ GT) & (w, Gamma))
+              (w'0:=w') (Gamma':=Gamma'); auto; try PPermut_simpl.
+apply PPermut_last_rev_simpl with (a:=(w, Gamma)); rewrite <- H7;
+subst; PPermut_simpl.
+rew_app; rewrite H2 in H4; rewrite H9 in H4; simpl;
+apply BackgroundSubsetImpl with
+  (G:=emptyEquiv (GH ++ GT ++ (w, Gamma) :: (w0, Gamma0) :: nil)); auto.
+assert (GH ++ GT ++ (w, Gamma) :: (w0, Gamma0) :: nil ~=~
+  (GH & (w, Gamma'') ++ GT) & (w0, Gamma0)) by (rew_app; PPermut_simpl);
+rewrite H13; auto.
+exists ((w'0, (@nil (var*ty))) :: nil); PPermut_simpl.
+assert ((w, Gamma) :: G & (w0, Gamma0) ~=~ G0 & (w0, Gamma0)) by
+  (rewrite <- H0; auto);
+rewrite H13 in Ok_Bg; rewrite H1 in Ok_Bg; subst;
+assert ((w', nil)
+      :: (w'0, nil)
+         :: emptyEquiv (GH ++ GT ++ (w, Gamma) :: (w0, Gamma0) :: nil) ~=~
+      (w'0, nil)
+      :: (w', nil)
+         :: emptyEquiv (GH ++ GT ++ (w, Gamma) :: (w0, Gamma0) :: nil)) by auto;
+rewrite H9; apply ok_Bg_fresh_wo;
+assert (((GH & (w, Gamma'') ++ GT) & (w', (v, A0) :: Gamma')) & (w0, Gamma0) ~=~
+  ((w', (v, A0) :: Gamma') :: GH ++ GT ++ (w, Gamma) :: nil) &  (w0, Gamma0)) by
+  (eapply PPermut_last_rev; auto; try PPermut_simpl);
+rew_app in *; [rewrite H14 in Ok_Bg | auto];
+apply emptyEquiv_ok_Bg in Ok_Bg; simpl in *; auto.
+symmetry; transitivity (G1 & (w', Gamma')); subst; rew_app in *; PPermut_simpl.
+Existential 1 := v'.
+Existential 1 := Gamma.
+Existential 1 := v'.
+Existential 1 := Gamma.
+Qed.
+*)
+Admitted.
+
+Lemma subst_t_preserv_types_inner:
+forall G Gamma A B M N v
+  (H_lc_t: lc_t_LF M)
+  (HT: G |= (v, A) :: Gamma |- N ::: B)
+  (HM: emptyEquiv G |= nil |- M ::: A),
+  G |= Gamma |- [M//fte v] N ::: B.
+intros; eapply subst_t_preserv_types with (Gamma := (v, A) :: Gamma); eauto.
+Qed.
+
+Lemma subst_t_preserv_types_outer:
+forall G0 G G' G'' Gamma Gamma' A B M N v
+  (H_lc_t: lc_t_LF M)
+  (G0G: G ~=~ (G0 & ((v, A) :: Gamma')))
+  (G0G': G' ~=~ (G0 & Gamma))
+  (G0G'': G'' ~=~ (G0 & Gamma'))
+  (HM: emptyEquiv G' |= nil |- M ::: A)
+  (HT: G |= Gamma |- N ::: B),
+  G'' |= Gamma |- [M // fte v] N ::: B.
+intros; eapply subst_t_preserv_types; eauto.
+Qed.
+
+Lemma merge_preserv_types:
+forall G Gamma M A
+  (H: G |= Gamma |- M ::: A),
+  (* outer *)
+  (forall G0 G1 Gamma0 Delta0,
+    G ~=~ Gamma0::Delta0::G0 ->
+    G1 ~=~ (Gamma0++Delta0) :: G0 ->
+    G1 |= Gamma |- M ::: A) /\
+  (* new or old - by PermutationGamma *)
+  (forall G0 Delta0,
+    G ~=~ Delta0 :: G0 ->
+    G0 |= Gamma ++ Delta0 |- M ::: A).
+intros; induction H; repeat split; intros.
+(* hyp *)
+constructor; auto. skip.
+(* Everywhere: eapply ok_Bg_concat; eauto *)
+constructor. skip. rewrite Mem_app_or_eq; left; auto.
+(* lam *)
+apply t_lam_LF with (L:=L). skip. intros; eapply H0; eauto.
+apply t_lam_LF with (L:=L). skip. intros; eapply H0; eauto.
+(* appl *)
+apply t_appl_LF with (A:=A). skip. eapply IHtypes_LF1; eauto.
+eapply IHtypes_LF2; eauto.
+apply t_appl_LF with (A:=A). skip. eapply IHtypes_LF1; eauto.
+eapply IHtypes_LF2; eauto.
+(* box *)
+constructor. skip. eapply IHtypes_LF with (G0:=G0 & Gamma)
+(Gamma0:=Gamma0) (Delta0:=Delta0); eauto. rewrite H0; PPermut_simpl.
+rewrite H1; PPermut_simpl.
+constructor. skip. eapply IHtypes_LF with (G0:=G0) (Gamma0:=Gamma)
+  (Delta0:=Delta0); eauto. rewrite H0; PPermut_simpl. PPermut_simpl.
+(* unbox *)
+constructor. skip. eapply IHtypes_LF; eauto.
+constructor. skip. eapply IHtypes_LF; eauto.
+(* Gamma *=* Gamma0 \/ Gamma *=* Gamma1 \/ neither *)
+assert (G & Gamma ~=~ Gamma0 :: Delta0 :: G0).
+  transitivity G'; auto.
+assert ((Gamma *=* Gamma0 /\ G ~=~ Delta0::G0) \/
+        (Gamma *=* Delta0 /\ G ~=~ Gamma0::G0) \/
+        (exists c, exists hd, exists tl, Gamma *=* c /\ G0 = hd & c ++ tl)).
+  assert ({Gamma *=* Gamma0} + {~ Gamma *=* Gamma0}).
+  apply permut_dec. intros. destruct k; destruct k'; decide equality.
+  apply eq_ty_dec. apply eq_var_dec.
+  assert ({Gamma *=* Delta0} + {~ Gamma *=* Delta0}).
+  apply permut_dec. intros. destruct k; destruct k'; decide equality.
+  apply eq_ty_dec. apply eq_var_dec.
+  destruct H4. left; split; auto. apply PPermut_last_rev with (Gamma:=Gamma)
+  (Gamma':=Gamma0); auto; rewrite H3; PPermut_simpl.
+  destruct H5.
+  right; left; split; auto. apply PPermut_last_rev with (Gamma:=Gamma)
+  (Gamma':=Delta0); auto; rewrite H3; PPermut_simpl.
+  right; right.
+  assert (G & Gamma ~=~ G0 & Delta0 & Gamma0) by (rewrite H3; PPermut_simpl).
+  symmetry in H4.
+  apply PPermut_split_neq in H4; auto.
+  destruct H4 as (Gamma'', (hd, (tl, (H4, H5)))).
+  assert (G0 & Delta0 ~=~ (hd ++ tl) & Gamma).
+    rewrite H5; PPermut_simpl.
+  apply PPermut_split_neq in H6; auto.
+  destruct H6 as (Delta'', (hd', (tl', (H6, H7)))).
+  exists Delta''; exists hd'; exists tl'; split; auto; symmetry; auto.
+  intro nn; symmetry in nn; elim n0; auto.
+  intro nn; symmetry in nn; elim n; auto.
+destruct H4. destruct H4.
+apply t_unbox_fetch_LF with (G:=G0) (Gamma:=Gamma0++Delta0).
+skip.
+apply PermutationGamma with (Gamma:=Gamma++Delta0); auto.
+eapply IHtypes_LF. rewrite H5; auto. rewrite H2; PPermut_simpl.
+destruct H4.
+destruct H4.
+apply t_unbox_fetch_LF with (G:=G0) (Gamma:=Delta0++Gamma0).
+skip.
+apply PermutationGamma with (Gamma:=Gamma++Gamma0); auto.
+eapply IHtypes_LF. rewrite H5; auto. rewrite H2; PPermut_simpl.
+destruct H4 as (c, (hd, (tl, (H4a, H4)))).
+apply t_unbox_fetch_LF with (G:=(Gamma0++Delta0)::hd++tl) (Gamma:=c).
+skip.
+apply PermutationGamma with (Gamma:=Gamma); auto.
+assert (G ~=~ Gamma0::Delta0::hd ++ tl).
+  subst; apply PPermut_last_rev with (Gamma:=Gamma) (Gamma':=c); auto;
+  rewrite H3; PPermut_simpl.
+eapply IHtypes_LF with (Gamma0:=Gamma0) (Delta0:=Delta0) (G0:=hd ++tl & Gamma');
+eauto.
+rewrite H5. rew_app; auto. rew_app; auto. rewrite H2; subst; PPermut_simpl.
+assert (G & Gamma ~=~ Delta0 :: G0).
+  transitivity G'; auto.
+assert ((Gamma *=* Delta0 /\ G ~=~ G0) \/
+        (exists c, exists hd, exists tl, c *=* Gamma /\ G0 = hd & c ++ tl)).
+  assert ({Gamma *=* Delta0} + {~ Gamma *=* Delta0}).
+  apply permut_dec. intros. destruct k; destruct k'; decide equality.
+  apply eq_ty_dec. apply eq_var_dec.
+  destruct H3. left; split; auto. apply PPermut_last_rev with (Gamma:=Gamma)
+  (Gamma':=Delta0); auto; rewrite H2; PPermut_simpl.
+  right.
+  assert (G & Gamma ~=~ G0 & Delta0) by (rewrite H2; PPermut_simpl).
+  symmetry in H3.
+  apply PPermut_split_neq in H3; auto.
+  intro nn; symmetry in nn; elim n; auto.
+destruct H3.
+destruct H3.
+constructor. skip.
+apply PermutationGamma with (Gamma:=Gamma++Gamma').
+eapply IHtypes_LF. rewrite H4; PPermut_simpl.
+permut_simpl; auto.
+destruct H3 as (c, (hd, (tl, (H3a, H3)))); subst.
+apply t_unbox_fetch_LF with (G:=hd++tl) (Gamma:=Gamma).
+skip.
+assert (G ~=~ Delta0::hd ++ tl).
+  apply PPermut_last_rev with (Gamma:=Gamma) (Gamma':=c). symmetry; auto.
+  rewrite H2; PPermut_simpl.
+eapply IHtypes_LF with (Gamma0:=Gamma') (Delta0 :=Delta0) (G0:= hd ++ tl).
+rewrite H3; PPermut_simpl. PPermut_simpl. PPermut_simpl.
+(* here *)
+constructor. skip. eapply IHtypes_LF; eauto.
+constructor. skip. eapply IHtypes_LF; eauto.
+(* Gamma *=* Gamma0 \/ Gamma *=* Gamma1 \/ neither *)
+assert (G & Gamma ~=~ Gamma0 :: Delta0 :: G0).
+  transitivity G'; auto.
+assert ((Gamma *=* Gamma0 /\ G ~=~ Delta0::G0) \/
+        (Gamma *=* Delta0 /\ G ~=~ Gamma0::G0) \/
+        (exists c, exists hd, exists tl, Gamma *=* c /\ G0 = hd & c ++ tl)).
+  assert ({Gamma *=* Gamma0} + {~ Gamma *=* Gamma0}).
+  apply permut_dec. intros. destruct k; destruct k'; decide equality.
+  apply eq_ty_dec. apply eq_var_dec.
+  assert ({Gamma *=* Delta0} + {~ Gamma *=* Delta0}).
+  apply permut_dec. intros. destruct k; destruct k'; decide equality.
+  apply eq_ty_dec. apply eq_var_dec.
+  destruct H4. left; split; auto. apply PPermut_last_rev with (Gamma:=Gamma)
+  (Gamma':=Gamma0); auto; rewrite H3; PPermut_simpl.
+  destruct H5.
+  right; left; split; auto. apply PPermut_last_rev with (Gamma:=Gamma)
+  (Gamma':=Delta0); auto; rewrite H3; PPermut_simpl.
+  right; right.
+  assert (G & Gamma ~=~ G0 & Delta0 & Gamma0) by (rewrite H3; PPermut_simpl).
+  symmetry in H4.
+  apply PPermut_split_neq in H4; auto.
+  destruct H4 as (Gamma'', (hd, (tl, (H4, H5)))).
+  assert (G0 & Delta0 ~=~ (hd ++ tl) & Gamma).
+    rewrite H5; PPermut_simpl.
+  apply PPermut_split_neq in H6; auto.
+  destruct H6 as (Delta'', (hd', (tl', (H6, H7)))).
+  exists Delta''; exists hd'; exists tl'; split; auto; symmetry; auto.
+  intro nn; symmetry in nn; elim n0; auto.
+  intro nn; symmetry in nn; elim n; auto.
+destruct H4. destruct H4.
+apply t_get_here_LF with (G:=G0) (Gamma:=Gamma0++Delta0).
+skip.
+apply PermutationGamma with (Gamma:=Gamma++Delta0); auto.
+eapply IHtypes_LF. rewrite H5; auto. rewrite H2; PPermut_simpl.
+destruct H4.
+destruct H4.
+apply t_get_here_LF with (G:=G0) (Gamma:=Delta0++Gamma0).
+skip.
+apply PermutationGamma with (Gamma:=Gamma++Gamma0); auto.
+eapply IHtypes_LF. rewrite H5; auto. rewrite H2; PPermut_simpl.
+destruct H4 as (c, (hd, (tl, (H4a, H4)))).
+apply t_get_here_LF with (G:=(Gamma0++Delta0)::hd++tl) (Gamma:=c).
+skip.
+apply PermutationGamma with (Gamma:=Gamma); auto.
+assert (G ~=~ Gamma0::Delta0::hd ++ tl).
+  subst; apply PPermut_last_rev with (Gamma:=Gamma) (Gamma':=c); auto;
+  rewrite H3; PPermut_simpl.
+eapply IHtypes_LF with (Gamma0:=Gamma0) (Delta0:=Delta0) (G0:=hd ++tl & Gamma');
+eauto.
+rewrite H5. rew_app; auto. rew_app; auto. rewrite H2; subst; PPermut_simpl.
+assert (G & Gamma ~=~ Delta0 :: G0).
+  transitivity G'; auto.
+assert ((Gamma *=* Delta0 /\ G ~=~ G0) \/
+        (exists c, exists hd, exists tl, c *=* Gamma /\ G0 = hd & c ++ tl)).
+  assert ({Gamma *=* Delta0} + {~ Gamma *=* Delta0}).
+  apply permut_dec. intros. destruct k; destruct k'; decide equality.
+  apply eq_ty_dec. apply eq_var_dec.
+  destruct H3. left; split; auto. apply PPermut_last_rev with (Gamma:=Gamma)
+  (Gamma':=Delta0); auto; rewrite H2; PPermut_simpl.
+  right.
+  assert (G & Gamma ~=~ G0 & Delta0) by (rewrite H2; PPermut_simpl).
+  symmetry in H3.
+  apply PPermut_split_neq in H3; auto.
+  intro nn; symmetry in nn; elim n; auto.
+destruct H3.
+destruct H3.
+constructor. skip.
+apply PermutationGamma with (Gamma:=Gamma++Gamma').
+eapply IHtypes_LF. rewrite H4; PPermut_simpl.
+permut_simpl; auto.
+destruct H3 as (c, (hd, (tl, (H3a, H3)))); subst.
+apply t_get_here_LF with (G:=hd++tl) (Gamma:=Gamma).
+skip.
+assert (G ~=~ Delta0::hd ++ tl).
+  apply PPermut_last_rev with (Gamma:=Gamma) (Gamma':=c). symmetry; auto.
+  rewrite H2; PPermut_simpl.
+eapply IHtypes_LF with (Gamma0:=Gamma') (Delta0 :=Delta0) (G0:= hd ++ tl).
+rewrite H3; PPermut_simpl. PPermut_simpl. PPermut_simpl.
+(* letdia *)
+apply t_letdia_LF with (L:=L) (A:=A).
+skip.
+  eapply IHtypes_LF; eauto. intros.
+  apply PPermutationG with  (G:=((v, A) :: nil) :: G1).
+  apply PPermutationG with (G:= ((v,A)::nil)::(Gamma0 ++ Delta0) :: G0).
+  eapply H0 with (G':=((v,A)::nil)::G) (G0:= ((v,A)::nil)::G0)
+    (Delta0:=Delta0)(Gamma0:=Gamma0); eauto.
+  PPermut_simpl. PPermut_simpl; auto. auto.
+apply t_letdia_LF with (L:=L) (A:=A).
+skip.
+  eapply IHtypes_LF; eauto. intros.
+  apply PPermutationG with (G:=((v, A) :: nil) :: G0).
+  eapply H0 with (G':=((v,A)::nil)::G); eauto. rewrite H1; PPermut_simpl. auto.
+assert (G & Gamma ~=~ Gamma0 :: Delta0 :: G1).
+  transitivity G0; auto.
+assert ((Gamma *=* Gamma0 /\ G ~=~ Delta0::G1) \/
+        (Gamma *=* Delta0 /\ G ~=~ Gamma0::G1) \/
+        (exists c, exists hd, exists tl, Gamma *=* c /\ G1 = hd & c ++ tl)).
+  assert ({Gamma *=* Gamma0} + {~ Gamma *=* Gamma0}).
+  apply permut_dec. intros. destruct k; destruct k'; decide equality.
+  apply eq_ty_dec. apply eq_var_dec.
+  assert ({Gamma *=* Delta0} + {~ Gamma *=* Delta0}).
+  apply permut_dec. intros. destruct k; destruct k'; decide equality.
+  apply eq_ty_dec. apply eq_var_dec.
+  destruct H5. left; split; auto. apply PPermut_last_rev with (Gamma:=Gamma)
+  (Gamma':=Gamma0); auto; rewrite H4; PPermut_simpl.
+  destruct H6.
+  right; left; split; auto. apply PPermut_last_rev with (Gamma:=Gamma)
+  (Gamma':=Delta0); auto; rewrite H4; PPermut_simpl.
+  right; right.
+  assert (G & Gamma ~=~ G1 & Delta0 & Gamma0) by (rewrite H4; PPermut_simpl).
+  symmetry in H5.
+  apply PPermut_split_neq in H5; auto.
+  destruct H5 as (Gamma'', (hd, (tl, (H5, H6)))).
+  assert (G1 & Delta0 ~=~ (hd ++ tl) & Gamma).
+    rewrite H6; PPermut_simpl.
+  apply PPermut_split_neq in H7; auto.
+  destruct H7 as (Delta'', (hd', (tl', (H7, H8)))).
+  exists Delta''; exists hd'; exists tl'; split; auto; symmetry; auto.
+  intro nn; symmetry in nn; elim n0; auto.
+  intro nn; symmetry in nn; elim n; auto.
+destruct H5. destruct H5.
+apply t_letdia_get_LF with (G:=G1) (Gamma:=Gamma++Delta0) (L:=L) (A:=A).
+skip.
+eapply IHtypes_LF.
+rewrite H6; PPermut_simpl.
+intros. eapply H0 with (G0:=((v,A)::nil)::G1) (Gamma0:=Gamma0)(Delta0:=Delta0);
+eauto. rewrite H6; PPermut_simpl. PPermut_simpl.
+rewrite H3; PPermut_simpl.
+destruct H5. destruct H5.
+apply t_letdia_get_LF with (G:=G1) (Gamma:=Gamma++Gamma0) (A:=A) (L:=L).
+skip.
+eapply IHtypes_LF. rewrite H6; PPermut_simpl.
+intros.
+eapply H0 with (G0:=((v,A)::nil)::G1) (Gamma0:=Gamma0)(Delta0:=Delta0);
+eauto. rewrite H6; PPermut_simpl. PPermut_simpl; constructor. rewrite H5. auto.
+auto. rewrite H3; PPermut_simpl. constructor; auto; rewrite H5; auto.
+destruct H5 as (c, (hd, (tl, (H5a, H5)))).
+apply t_letdia_get_LF with
+  (G:=(Gamma0++Delta0)::hd++tl)(Gamma:=Gamma) (L:=L)(A:=A).
+skip.
+rew_app.
+eapply IHtypes_LF with (G0:=hd++tl & Gamma') (Gamma0:=Gamma0)(Delta0:=Delta0);
+eauto. PPermut_simpl; rew_app.
+subst.
+apply PPermut_last_rev with (Gamma:=Gamma) (Gamma':=c); auto; rewrite H4;
+PPermut_simpl.
+intros. rew_app.
+eapply H0 with (G0:=((v,A)::nil)::G1) (Gamma0:=Gamma0) (Delta0:=Delta0);
+eauto.
+rewrite H4; PPermut_simpl.
+subst; PPermut_simpl. rewrite H3; subst; PPermut_simpl.
+assert (G & Gamma ~=~ Delta0 :: G1).
+  transitivity G0; auto.
+assert ((Gamma *=* Delta0 /\ G ~=~ G1) \/
+        (exists c, exists hd, exists tl, Gamma *=* c /\ G1 = hd & c ++ tl)).
+  assert ({Gamma *=* Delta0} + {~ Gamma *=* Delta0}).
+  apply permut_dec. intros. destruct k; destruct k'; decide equality.
+  apply eq_ty_dec. apply eq_var_dec.
+  destruct H4. left; split; auto. apply PPermut_last_rev with (Gamma:=Gamma)
+  (Gamma':=Delta0); auto; rewrite H3; PPermut_simpl.
+  right.
+  assert (G & Gamma ~=~ G1 & Delta0) by (rewrite H3; PPermut_simpl).
+  symmetry in H4.
+  apply PPermut_split_neq in H4; auto.
+  destruct H4 as (Gamma'', (hd, (tl, (H5, H6)))).
+  exists Gamma''; exists hd; exists tl; split.
+  symmetry; auto. auto.
+  intro nn; symmetry in nn; elim n; auto.
+destruct H4.
+destruct H4.
+apply t_letdia_LF with (A:=A)(L:=L). skip.
+apply PermutationGamma with (Gamma:=Gamma++Gamma').
+eapply IHtypes_LF; eauto.
+rewrite H5; PPermut_simpl. rewrite H4; auto.
+intros.
+eapply H0; eauto.
+rewrite <- H7; rewrite H5; PPermut_simpl.
+destruct H4 as (c, (hd, (tl, (H4a, H4)))).
+apply t_letdia_get_LF with
+  (G:=hd++tl)(Gamma:=Gamma) (L:=L)(A:=A).
+skip.
+subst. rew_app.
+eapply IHtypes_LF with (G0:=hd++tl) (Gamma0:=Gamma')(Delta0:=Delta0);
+eauto. PPermut_simpl; apply PPermut_last_rev with (Gamma:=Gamma) (Gamma':=c);
+auto; rewrite H3; PPermut_simpl. PPermut_simpl.
+intros; subst; rew_app.
+eapply H0; eauto. rewrite H3; PPermut_simpl. subst; PPermut_simpl.
+Qed.
+
+Lemma merge_preserv_types_outer:
+forall G G0 G1 Gamma Gamma0 Delta0 M A,
+  G |= Gamma |- M ::: A ->
+  G ~=~ Gamma0 :: Delta0 :: G0 ->
+  G1 ~=~ (Gamma0 ++ Delta0) :: G0 ->
+  G1 |= Gamma |- M ::: A.
+intros; eapply merge_preserv_types; eauto.
+Qed.
+
+Lemma merge_preserv_types_new:
+forall G G0 Gamma Delta M A,
+  G |= Gamma |- M ::: A ->
+  G ~=~ Delta::G0 ->
+  G0 |= Gamma++Delta |- M ::: A.
+intros; eapply merge_preserv_types with (G:=G) (Gamma:=Gamma); eauto.
+Qed.
+
+Lemma merge_preserv_types_old:
+forall G G0 Gamma Delta M A,
+  G |= Delta |- M ::: A ->
+  G ~=~ Gamma::G0 ->
+  G0 |= Gamma++Delta |- M ::: A.
+intros;
+apply PermutationGamma with (Gamma:=Delta++Gamma).
+eapply merge_preserv_types; eauto.
+auto.
+Qed.
+
+Lemma Progress:
+forall G M A
+  (H_lc_t: lc_t_LF M)
+  (HT: emptyEquiv G |= nil |- M ::: A),
+  value_LF M \/ exists N, M |-> N.
+intros;
+remember (@nil (var * ty)) as Ctx;
+generalize dependent Ctx.
+generalize dependent A;
+generalize dependent G.
+induction M; intros; eauto using value_LF;
+inversion HeqCtx; subst.
+(* hyp *)
+inversion HT; subst.
+rewrite Mem_nil_eq in H3;
+contradiction.
+(* appl *)
+right; inversion HT; subst;
+inversion H_lc_t; subst;
+edestruct IHM1 with (A := A0 ---> A); eauto;
+[inversion H0; subst; inversion H4; subst | inversion H0];
+eexists; constructor; eauto;
+inversion H3; subst; auto.
+(* unbox *)
+right; inversion HT; subst;
+inversion H_lc_t; subst.
+edestruct IHM with (A := [*]A); eauto;
+[ inversion H0; subst; inversion H3; subst; inversion H3 |
+  destruct H0];
+eexists; constructor; eauto;
+inversion H1; inversion H2; subst; auto.
+assert (Gamma = nil) by
+  ( apply emptyEquiv_permut_empty with
+    (G:= G0 & Gamma) (G':=G); auto;
+    apply Mem_last); subst.
+destruct IHM with (A := [*]A)
+                  (Ctx := (@nil (var * ty)))
+                  (G := G0 & nil);
+eauto.
+assert (emptyEquiv (G0 & nil) = G0 & nil) by
+  skip.
+rewrite H0; auto.
+inversion H0; subst; inversion H1; subst.
+eexists; constructor; eauto. inversion H3; auto; subst.
+destruct H0; eexists; econstructor; eauto.
+(* here *)
+inversion HT; subst;
+inversion H_lc_t; subst.
+edestruct IHM; eauto;
+[left; econstructor | right; destruct H0; eexists];
+eauto using step_LF.
+assert (Gamma = nil) by
+  ( apply emptyEquiv_permut_empty with
+    (G:= G0 & Gamma) (G':=G); auto;
+    apply Mem_last); subst;
+destruct IHM with (A := A0)
+                  (Ctx := (@nil (var*ty)))
+                  (G := G0 & nil);
+eauto.
+assert (emptyEquiv (G0 & nil) = G0 & nil) by skip.
+rewrite H0; auto.
+left; inversion H0; subst; inversion H4; subst;
+econstructor; eauto using step_LF.
+right; destruct H0; eexists;
+econstructor; eauto using step_LF.
+(* letdia *)
+right; inversion HT; subst;
+inversion H_lc_t; subst.
+edestruct IHM1 with (A := <*>A0); eauto;
+[ inversion H0; subst; inversion HT1; subst |
+  destruct H0];
+eexists; constructor; eauto.
+inversion H4; subst; auto.
+inversion H4; subst; auto.
+assert (Gamma = nil) by
+  ( apply emptyEquiv_permut_empty with (G:= G0 & Gamma) (G':=G);
+    auto; apply Mem_last); subst;
+edestruct IHM1 with (G := G0 & nil)
+                    (Ctx := (@nil (var*ty)))
+                    (A := <*>A0); eauto;
+assert ( emptyEquiv (G0 & nil) = G0 & nil) by skip.
+rewrite H0; auto.
+inversion H0; subst; inversion HT1; subst;
+eexists; constructor; eauto;
+inversion H4; subst; auto.
+destruct H0;
+eexists; econstructor; eauto.
+Qed.
+
+(* this is also to be moved *)
+(* end *)
+
+Lemma Preservation:
+forall G M N A
+  (HT: emptyEquiv G |= nil |- M ::: A)
+  (HS: M |-> N),
+  emptyEquiv G |= nil |- N ::: A.
+intros; generalize dependent N.
+remember (emptyEquiv G) as G';
+remember (@nil (var*ty)) as Gamma.
+generalize dependent G.
+induction HT; intros;
+inversion HS; subst;
+try (econstructor; eauto).
+
+(* appl_lam *)
+inversion HT1; subst;
+unfold open_LF in *;
+assert (exists v, v \notin L \u used_vars_te_LF M0) as HF by apply Fresh;
+destruct HF as (v_fresh);
+rewrite subst_t_neutral_free with (v:=v_fresh);
+[ eapply subst_t_preserv_types_inner; eauto |
+  rewrite notin_union in H; destruct H]; auto;
+rewrite <- double_emptyEquiv; auto.
+
+(* unbox_box *)
+inversion HT; subst;
+replace (@nil (var * ty)) with (nil ++ (@nil (prod var ty)))
+  by (rew_app; auto);
+apply merge_preserv_types_old with (G:=emptyEquiv G0 & nil);
+rew_app; auto.
+skip.
+
+inversion HT; subst;
+replace (@nil (var * ty)) with (nil ++ (@nil (prod var ty)))
+  by (rew_app; auto);
+apply merge_preserv_types_old with (G:=G & nil & Gamma);
+auto. rewrite <- H; auto.
+
+skip.
+
+assert (Gamma = nil) by skip. (* from H *)
+subst. replace (emptyEquiv G0) with (G & nil).
+apply IHHT with (G0:=G0); auto.
+skip. (* these are all just nils but we should probably do sth about it in
+         the lemma statement *)
+skip. (* this is really permut rewrite using H *)
+
+(* here *)
+skip.
+
+assert (Gamma = nil) by skip. (* from H *)
+subst. replace (emptyEquiv G0) with (G & nil).
+apply IHHT with (G0:=G0); auto.
+skip. (* these are all just nils but we should probably do sth about it in
+         the lemma statement *)
+skip. (* this is really permut rewrite using H *)
+
+inversion HT; subst;
+unfold open_LF in *;
+assert (exists v, v \notin L \u used_vars_te_LF N) as HF by apply Fresh;
+destruct HF as (v_fresh);
+rewrite subst_t_neutral_free with (v:=v_fresh);
+replace (@nil (var * ty)) with (nil ++ (@nil (prod var ty)))
+  by (rew_app; auto).
+
+apply merge_preserv_types_old with (G:=emptyEquiv G0 & nil);
+rew_app; auto.
+apply subst_t_preserv_types_outer with
+  (A:=A) (G:=((v_fresh, A) :: nil) :: emptyEquiv G0) (G0:=emptyEquiv G0)
+  (Gamma':=nil) (G':=emptyEquiv G0 & nil); eauto.
+skip. skip. skip.
+assert (emptyEquiv G0 & nil = emptyEquiv (G0 & nil)) by skip.
+rewrite H1; rewrite <- double_emptyEquiv; rewrite <- H1.
+replace (emptyEquiv G0 & nil) with (nil::emptyEquiv G0) by skip.
+apply WeakeningG; auto.
+apply HT2.
+rewrite notin_union in H0; destruct H0; auto.
+skip. skip.
+rewrite notin_union in H0; destruct H0; auto.
+
+apply merge_preserv_types_old with (G:=emptyEquiv G0 & nil);
+rew_app; auto.
+apply subst_t_preserv_types_outer with
+  (A:=A) (G:=((v_fresh, A) :: nil) :: emptyEquiv G0) (G0:=emptyEquiv G0)
+  (Gamma':=nil) (G':=emptyEquiv G0 & nil); eauto.
+skip. skip. skip.
+assert (Gamma = nil) by skip; subst.
+assert (emptyEquiv G0 & nil = emptyEquiv (G0 & nil)) by skip.
+rewrite H1; rewrite <- double_emptyEquiv; rewrite <- H1.
+replace (emptyEquiv G0 & nil) with (nil::emptyEquiv G0) by skip.
+apply WeakeningG; auto. skip. (* rewrite by H7; exact H6 *)
+apply HT2.
+rewrite notin_union in H0; destruct H0; auto.
+skip. skip.
+
+rewrite notin_union in H0; destruct H0; auto.
+
+inversion HT; subst;
+unfold open_LF in *;
+assert (exists v, v \notin L \u used_vars_te_LF N) as HF by apply Fresh;
+destruct HF as (v_fresh);
+rewrite subst_t_neutral_free with (v:=v_fresh);
+replace (@nil (var * ty)) with (nil ++ (@nil (prod var ty)))
+  by (rew_app; auto).
+apply merge_preserv_types_old with (G:=emptyEquiv G1 & nil);
+rew_app; auto.
+apply subst_t_preserv_types_outer with
+  (A:=A) (G:=((v_fresh, A) :: nil) :: emptyEquiv G1) (G0:=emptyEquiv G1)
+  (Gamma':=nil) (G':=emptyEquiv G1 & nil); eauto.
+skip. skip. skip.
+assert (emptyEquiv G1 & nil = emptyEquiv (G1 & nil)) by skip.
+rewrite H2; rewrite <- double_emptyEquiv; rewrite <- H2.
+replace (emptyEquiv G1 & nil) with (nil::emptyEquiv G1) by skip.
+apply WeakeningG; auto.
+replace (emptyEquiv G1) with (G & Gamma) by skip.
+assert (Gamma = nil) by skip; subst; auto.
+skip.
+replace (emptyEquiv G1) with (G & Gamma) by skip.
+apply HT2; eauto.
+skip. eauto.
+apply merge_preserv_types_old with (G:=emptyEquiv G1 & nil);
+rew_app; auto.
+apply subst_t_preserv_types_outer with
+  (A:=A) (G:=((v_fresh, A) :: nil) :: emptyEquiv G1) (G0:=emptyEquiv G1)
+  (Gamma':=nil) (G':=emptyEquiv G1 & nil); eauto.
+skip. skip. skip.
+assert (emptyEquiv G1 & nil = emptyEquiv (G1 & nil)) by skip.
+rewrite H2; rewrite <- double_emptyEquiv; rewrite <- H2.
+replace (emptyEquiv G1 & nil) with (nil::emptyEquiv G1) by skip.
+apply WeakeningG; auto.
+replace (emptyEquiv G1) with (G & Gamma) by skip.
+assert (Gamma = nil) by skip; subst; auto.
+assert (Gamma0 = nil) by skip; subst; auto.
+assert (G0 ~=~ G) by skip. (* from H8 *)
+replace G with G0. auto. skip.
+skip.
+replace (emptyEquiv G1) with (G & Gamma) by skip.
+apply HT2; eauto.
+skip. eauto.
+skip.
+replace (emptyEquiv G1) with (G & Gamma) by skip.
+assert (Gamma = nil) by skip; subst; eapply IHHT; auto.
+skip.
+
+intros. unfold open_LF in *.
+assert (Gamma = nil) by skip; subst.
+replace G' with (((v,A)::nil) :: emptyEquiv G1) by skip.
+replace (emptyEquiv G1) with (G & nil) by skip.
+apply HT2; eauto.
+Admitted.
