LabelFree/SingleUnbox/Substitution.v
@@ -1,0 +1,76 @@
+Add LoadPath "../..".
+Require Import PermutLib.
+Require Import Syntax.
+Require Import Arith.
+Require Export LibTactics. (* case_if *)
+
+Open Scope permut_scope.
+
+Reserved Notation " [ M // x ] N " (at level 5).
+
+Fixpoint subst_t_LF M x N :=
+match N with
+| hyp_LF v => if (eq_vte_dec x v) then M else N
+| lam_LF t N' => lam_LF t [M//shift_vte x]N'
+| appl_LF N' N'' => appl_LF [M//x]N' [M//x]N''
+| box_LF N' => box_LF [M//x]N'
+| unbox_LF N' => unbox_LF [M//x]N'
+| here_LF N' => here_LF [M//x]N'
+| letdia_LF N' N'' => letdia_LF [M//x]N' [M//shift_vte x]N''
+end
+where " [ M // x ] N " := (subst_t_LF M x N).
+
+Definition open_LF (M: te_LF) (t: te_LF) := subst_t_LF t (bte 0) M.
+Notation " M '^t^' t " := (open_LF M t) (at level 67).
+
+Lemma closed_subst_t_free_LF:
+forall M v0 N
+  (H_lc: v0 \notin used_vars_te_LF N),
+  [M // fte v0] N = N.
+induction N; intros; simpl in *;
+repeat case_if;
+try (rewrite IHN || (rewrite IHN1; try rewrite IHN2); auto);
+[ rewrite notin_singleton in H_lc; elim H_lc |
+  destruct v]; auto.
+Qed.
+
+Lemma closed_subst_t_bound_LF:
+forall N M v0 n
+  (H_lc: lc_t_n_LF n N),
+  v0 >= n -> [M // bte v0] N = N.
+induction N; intros; simpl in *;
+repeat case_if; inversion H_lc; subst;
+try (erewrite IHN || (erewrite IHN1; try erewrite IHN2)); eauto.
+assert (~(n = v0)) by omega;
+apply gt_asym in H2; elim H2; omega.
+omega. omega.
+Qed.
+
+Lemma subst_t_comm_LF:
+forall M v v' n N
+  (Lc: lc_t_LF N),
+  v <> v' ->
+  [ N // fte v] ([ hyp_LF (fte v') // bte n] M) =
+  [hyp_LF (fte v') // bte n] ([N // fte v] M).
+induction M; intros; simpl;
+[ repeat (case_if; simpl); auto;
+  erewrite closed_subst_t_bound_LF; eauto; omega | | | | | |];
+try (rewrite IHM; auto);
+try (rewrite IHM1; try rewrite IHM2; auto);
+repeat (case_if; simpl); subst; simpl;
+auto;
+erewrite closed_subst_t_bound;
+eauto;
+replace n with (0+n) by omega;
+apply closed_t_addition; auto.
+Qed.
+
+Lemma subst_t_neutral_free_LF:
+forall M v n N
+  (HT: v \notin used_vars_te_LF M),
+  [ N // bte n] M = [N // fte v] [hyp_LF (fte v) // bte n] M.
+induction M; intros; simpl in *;
+try (erewrite IHM || (erewrite IHM1; try erewrite IHM2); eauto);
+repeat (case_if; simpl); subst; auto;
+assert (v0 <> v0) as Neq by eauto; elim Neq; auto.
+Qed.
